Fundamental Lemma!

theories/Fundamental.v
@@ -1,10 +1,10 @@
 (** * LogRel.Fundamental: declarative typing implies the logical relation for any generic instance. *)
 From LogRel.AutoSubst Require Import core unscoped Ast Extra.
-From LogRel Require Import Utils BasicAst Notations Context NormalForms Weakening
-  DeclarativeTyping DeclarativeInstance GenericTyping LogicalRelation Validity.
-From LogRel.LogicalRelation Require Import Escape Irrelevance Reflexivity Transitivity Universe Weakening Neutral Induction NormalRed.
-From LogRel.Substitution Require Import Irrelevance Properties Conversion Reflexivity SingleSubst Escape.
-From LogRel.Substitution.Introductions Require Import Application Universe Pi Lambda Var Nat Empty SimpleArr.
+From LogRel Require Import Utils BasicAst Notations LContexts Context NormalForms Weakening
+  DeclarativeTyping DeclarativeInstance GenericTyping Monad LogicalRelation Validity.
+From LogRel.LogicalRelation Require Import Escape Irrelevance Reflexivity Transitivity Universe Monotonicity Split Weakening Neutral Induction NormalRed.
+From LogRel.Substitution Require Import Irrelevance Properties Conversion Reflexivity SingleSubst Escape Monotonicity Split.
+From LogRel.Substitution.Introductions Require Import Application Universe Pi Lambda Var Nat Bool Empty SimpleArr Sigma Id.
 
 Set Primitive Projections.
 Set Universe Polymorphism.
@@ -21,84 +21,83 @@ later validity relations depends on earlier ones, and makes using the fundamenta
 easier, because we can simply invoke it to get all the validity properties we need. *)
 
 Definition FundCon `{GenericTypingProperties}
-  (Γ : context) : Type := [||-v Γ ].
+  (wl : wfLCon) (Γ : context) : Type := [||-v Γ ]< wl >.
 
 Module FundTy.
-  Record FundTy `{GenericTypingProperties} {Γ : context} {A : term}
+  Record FundTy `{GenericTypingProperties} {wl : wfLCon} {Γ : context} {A : term}
   : Type := {
-    VΓ : [||-v Γ ];
-    VA : [ Γ ||-v< one > A | VΓ ]
+    VΓ : [||-v Γ ]< wl >;
+    VA : [ Γ ||-v< one > A | VΓ ]< wl >
   }.
-
-  Arguments FundTy {_ _ _ _ _ _ _ _ _ _ _ _ _ _ _ _}.
+  Arguments FundTy {_ _ _ _ _ _ _ _ _ _ _ _}.
 End FundTy.
 
 Export FundTy(FundTy,Build_FundTy).
 
 Module FundTyEq.
   Record FundTyEq `{GenericTypingProperties}
-    {Γ : context} {A B : term}
+    {wl : wfLCon} {Γ : context} {A B : term}
   : Type := {
-    VΓ : [||-v Γ ];
-    VA : [ Γ ||-v< one > A | VΓ ];
-    VB : [ Γ ||-v< one > B | VΓ ];
-    VAB : [ Γ ||-v< one > A ≅ B | VΓ | VA ]
+    VΓ : [||-v Γ ]< wl >;
+    VA : [ Γ ||-v< one > A | VΓ ]< wl >;
+    VB : [ Γ ||-v< one > B | VΓ ]< wl >;
+    VAB : [ Γ ||-v< one > A ≅ B | VΓ | VA ]< wl >
   }.
-  Arguments FundTyEq {_ _ _ _ _ _ _ _ _ _ _ _ _ _ _ _}.
+  Arguments FundTyEq {_ _ _ _ _ _ _ _ _ _ _ _}.
 End FundTyEq.
 
 Export FundTyEq(FundTyEq,Build_FundTyEq).
 
 Module FundTm.
   Record FundTm `{GenericTypingProperties}
-    {Γ : context} {A t : term}
+    {wl : wfLCon} {Γ : context} {A t : term}
   : Type := {
-    VΓ : [||-v Γ ];
-    VA : [ Γ ||-v< one > A | VΓ ];
-    Vt : [ Γ ||-v< one > t : A | VΓ | VA ];
+    VΓ : [||-v Γ ]< wl >;
+    VA : [ Γ ||-v< one > A | VΓ ]< wl >;
+    Vt : [ Γ ||-v< one > t : A | VΓ | VA ]< wl >;
   }.
-  Arguments FundTm {_ _ _ _ _ _ _ _ _ _ _ _ _ _ _ _}.
+  Arguments FundTm {_ _ _ _ _ _ _ _ _ _ _ _}.
 End FundTm.
 
 Export FundTm(FundTm,Build_FundTm).
 
 Module FundTmEq.
   Record FundTmEq `{GenericTypingProperties}
-    {Γ : context} {A t u : term}
+    {wl : wfLCon} {Γ : context} {A t u : term}
   : Type := {
-    VΓ : [||-v Γ ];
-    VA : [ Γ ||-v< one > A | VΓ ];
-    Vt : [ Γ ||-v< one > t : A | VΓ | VA ];
-    Vu : [ Γ ||-v< one > u : A | VΓ | VA ];
-    Vtu : [ Γ ||-v< one > t ≅ u : A | VΓ | VA ];
+    VΓ : [||-v Γ ]< wl >;
+    VA : [ Γ ||-v< one > A | VΓ ]< wl >;
+    Vt : [ Γ ||-v< one > t : A | VΓ | VA ]< wl >;
+    Vu : [ Γ ||-v< one > u : A | VΓ | VA ]< wl >;
+    Vtu : [ Γ ||-v< one > t ≅ u : A | VΓ | VA ]< wl >;
   }.
-  Arguments FundTmEq {_ _ _ _ _ _ _ _ _ _ _ _ _ _ _ _}.
+  Arguments FundTmEq {_ _ _ _ _ _ _ _ _ _ _ _}.
 End FundTmEq.
 
 Export FundTmEq(FundTmEq,Build_FundTmEq).
 
 Module FundSubst.
   Record FundSubst `{GenericTypingProperties}
-    {Γ Δ : context} {wfΓ : [|- Γ]} {σ : nat -> term}
+    {wl wl' : wfLCon} {Γ Δ : context} {σ : nat -> term} {f: wl' ≤ε wl}  {wfΓ : [|- Γ]< wl' >}
   : Type := {
-    VΔ : [||-v Δ ] ;
-    Vσ : [VΔ | Γ ||-v σ : Δ | wfΓ] ;
+    VΔ : [||-v Δ ]< wl > ;
+    Vσ : [VΔ | Γ ||-v σ : Δ | wfΓ | f]< wl > ;
   }.
-  Arguments FundSubst {_ _ _ _ _ _ _ _ _ _ _ _ _ _ _ _}.
+  Arguments FundSubst {_ _ _ _ _ _ _ _ _ _ _ _}.
 End FundSubst.
 
 Export FundSubst(FundSubst,Build_FundSubst).
 
 Module FundSubstConv.
   Record FundSubstConv `{GenericTypingProperties}
-    {Γ Δ : context} {wfΓ : [|- Γ]} {σ σ' : nat -> term}
+    {wl wl' : wfLCon} {Γ Δ : context}  {σ σ' : nat -> term} {f: wl' ≤ε wl} {wfΓ : [|- Γ]< wl' >}
   : Type := {
-    VΔ : [||-v Δ ] ;
-    Vσ : [VΔ | Γ ||-v σ : Δ | wfΓ] ;
-    Vσ' : [VΔ | Γ ||-v σ' : Δ | wfΓ ] ;
-    Veq : [VΔ | Γ ||-v σ ≅ σ' : Δ | wfΓ | Vσ] ;
+    VΔ : [||-v Δ ]< wl > ;
+    Vσ : [VΔ | Γ ||-v σ : Δ | wfΓ | f]< wl > ;
+    Vσ' : [VΔ | Γ ||-v σ' : Δ | wfΓ | f]< wl > ;
+    Veq : [VΔ | Γ ||-v σ ≅ σ' : Δ | wfΓ | Vσ | f]< wl > ;
   }.
-  Arguments FundSubstConv {_ _ _ _ _ _ _ _ _ _ _ _ _ _ _ _}.
+  Arguments FundSubstConv {_ _ _ _ _ _ _ _ _ _ _ _ _ _}.
 End FundSubstConv.
 
 Export FundSubstConv(FundSubstConv,Build_FundSubstConv).
@@ -114,80 +113,90 @@ Section Fundamental.
   Context `{GenericTypingProperties}.
   Import DeclarativeTypingData.
 
-  Lemma FundConNil : FundCon ε.
+  Lemma FundConNil {wl} : FundCon wl ε.
   Proof.
   unshelve econstructor.
-  + unshelve econstructor.
-    - intros; exact unit.
-    - intros; exact unit.
-  + constructor.
+  - unshelve econstructor.
+    + intros; exact unit.
+    + intros; exact unit.
+  - cbn.
+    constructor.
+    all: now auto.
   Qed.
 
-  Lemma FundConCons (Γ : context) (A : term)
-  (wfΓ : [ |-[ de ] Γ]) (fΓ : FundCon Γ) (tA : [Γ |-[ de ] A]) (fA : FundTy Γ A) : FundCon (Γ,, A).
+  Lemma FundConCons (wl : wfLCon) (Γ : context) (A : term)
+  (fΓ : FundCon wl Γ) (fA : FundTy wl Γ A) : FundCon wl (Γ,, A).
   Proof.
     destruct fA as [ VΓ VA ].
-    eapply validSnoc. exact VA.
+    eapply validSnoc'. exact VA.
   Qed.
 
-  Lemma FundTyU (Γ : context) (tΓ : [ |-[ de ] Γ]) (fΓ : FundCon Γ) : FundTy Γ U.
+  Lemma FundTyU (wl : wfLCon) (Γ : context) (fΓ : FundCon wl Γ) : FundTy wl Γ U.
   Proof.
     unshelve econstructor.
     - assumption.
     - unshelve econstructor.
-      + intros * _. apply LRU_.  
-        econstructor; tea; [constructor|]. 
-        cbn; eapply redtywf_refl; gen_typing.
-      + intros * _ _. simpl. constructor.
-        cbn; eapply redtywf_refl; gen_typing.
+      + intros * _.
+        econstructor ; intros wl'' Ho.
+        pose (f' := over_tree_le Ho).
+        apply LRU_.  
+        econstructor; tea  ; [constructor| now eapply wfc_Ltrans | ]. 
+        cbn; eapply redtywf_refl.
+        eapply wft_Ltrans ; [eassumption | gen_typing].
+      + intros * _ _. simpl.
+        econstructor ; intros wl'' Ho Ho'.
+        pose (f' := over_tree_le Ho).
+        constructor.
+        cbn; eapply redtywf_refl.
+        eapply wft_Ltrans ; [eassumption | gen_typing].
+        Unshelve. all: now constructor.
   Qed.
 
-  Lemma FundTyPi (Γ : context) (F G : term)
-    (tF : [Γ |-[ de ] F]) (fF : FundTy Γ F)
-    (tG : [Γ,, F |-[ de ] G]) (fG : FundTy (Γ,, F) G)
-    : FundTy Γ (tProd F G).
+  Lemma FundTyPi (wl : wfLCon) (Γ : context) (F G : term)
+    (fF : FundTy wl Γ F)
+    (fG : FundTy wl (Γ,, F) G)
+    : FundTy wl Γ (tProd F G).
   Proof.
     destruct fF as [ VΓ VF ]. destruct fG as [ VΓF VG ].
     econstructor.
     unshelve eapply (PiValid VΓ).
     - assumption.
-    - now eapply irrelevanceValidity.
+    - now eapply irrelevanceTy.
   Qed.
 
-  Lemma FundTyUniv (Γ : context) (A : term)
-    (tA : [Γ |-[ de ] A : U]) (fA : FundTm Γ U A)
-    : FundTy Γ A.
+  Lemma FundTyUniv (wl : wfLCon) (Γ : context) (A : term)
+    (fA : FundTm wl Γ U A)
+    : FundTy wl Γ A.
   Proof.
     destruct fA as [ VΓ VU [ RA RAext ] ]. econstructor.
     unshelve econstructor.
     - intros * vσ.
-      eapply UnivEq. exact (RA _ _ wfΔ vσ).
+      eapply WUnivEq. exact (RA _ _ _ _ wfΔ vσ).
     - intros * vσ' vσσ'.
-      eapply UnivEqEq. exact (RAext _ _ _ wfΔ vσ vσ' vσσ').
+      eapply WUnivEqEq. exact (RAext _ _ _ _ _ wfΔ vσ vσ' vσσ').
   Qed.
 
-  Lemma FundTmVar : forall (Γ : context) (n : nat) decl,
-    [ |-[ de ] Γ] -> FundCon Γ ->
-    in_ctx Γ n decl -> FundTm Γ decl (tRel n).
+  Lemma FundTmVar : forall (wl : wfLCon) (Γ : context) (n : nat) decl,
+      FundCon wl Γ ->
+      in_ctx Γ n decl -> FundTm wl Γ decl (tRel n).
   Proof.
-    intros Γ n d wfΓ FΓ hin; induction hin;
-      destruct (invValiditySnoc FΓ) as [l [VΓ [VA _]]]; clear FΓ.
+    intros wl Γ n d FΓ hin.
+    induction hin ; destruct (invValidity FΓ) as [l [VΓ [VA [Hsub [Hext ]]]]] ; subst.
     - renToWk; rewrite <- (wk1_ren_on Γ d d).
       eexists _ _; unshelve eapply var0Valid; tea.
       now eapply embValidTyOne.
     - renToWk; rewrite <- (wk1_ren_on Γ d' d).
-      destruct (IHhin (boundary_ctx_ctx wfΓ) VΓ); cbn in *.
+      destruct (IHhin VΓ); cbn in *.
       econstructor. set (ρ := wk1 _).
       replace (tRel _) with (tRel n)⟨ρ⟩ by (unfold ρ; now bsimpl).
-      unshelve eapply wk1ValidTm; cycle 1; tea; now eapply irrelevanceValidity.
+      unshelve eapply wk1ValidTm; cycle 1; tea; now eapply irrelevanceTy.
   Qed.
 
-  Lemma FundTmProd : forall (Γ : context) (A B : term),
-    [Γ |-[ de ] A : U] -> FundTm Γ U A ->
-    [Γ,, A |-[ de ] B : U] ->
-    FundTm (Γ,, A) U B -> FundTm Γ U (tProd A B).
+  Lemma FundTmProd : forall (wl : wfLCon) (Γ : context) (A B : term),
+    FundTm wl Γ U A ->
+    FundTm wl (Γ,, A) U B -> FundTm wl Γ U (tProd A B).
   Proof.
-    intros * ? [] ? []; econstructor.
+    intros * [] []; econstructor.
     eapply PiValidU; irrValid.
     Unshelve. 
     3: eapply UValid. 
@@ -195,140 +204,131 @@ Section Fundamental.
     all:tea.
   Qed.
 
-  Lemma FundTmLambda : forall (Γ : context) (A B t : term),
-    [Γ |-[ de ] A] ->
-    FundTy Γ A ->
-    [Γ,, A |-[ de ] t : B] ->
-    FundTm (Γ,, A) B t -> FundTm Γ (tProd A B) (tLambda A t).
+  Lemma FundTmLambda : forall (wl : wfLCon) (Γ : context) (A B t : term),
+    FundTy wl Γ A ->
+    FundTm wl (Γ,, A) B t -> FundTm wl Γ (tProd A B) (tLambda A t).
   Proof.
-    intros * ?[]?[]; econstructor.
+    intros * [] []; econstructor.
     eapply lamValid; irrValid.
     Unshelve. all: irrValid.
   Qed.
 
-  Lemma FundTmApp : forall (Γ : context) (f a A B : term),
-    [Γ |-[ de ] f : tProd A B] ->
-    FundTm Γ (tProd A B) f ->
-    [Γ |-[ de ] a : A] -> FundTm Γ A a -> FundTm Γ B[a..] (tApp f a).
+  Lemma FundTmApp : forall (wl : wfLCon) (Γ : context) (f a A B : term),
+    FundTm wl Γ (tProd A B) f ->
+    FundTm wl Γ A a -> FundTm wl Γ B[a..] (tApp f a).
   Proof.
-    intros * ?[]?[]; econstructor.
+    intros * [] []; econstructor.
     now eapply appValid.
     Unshelve. all: irrValid.
   Qed.
 
-  Lemma FundTmConv : forall (Γ : context) (t A B : term),
-    [Γ |-[ de ] t : A] -> FundTm Γ A t ->
-    [Γ |-[ de ] A ≅ B] -> FundTyEq Γ A B -> FundTm Γ B t.
+  Lemma FundTmConv : forall (wl : wfLCon) (Γ : context) (t A B : term),
+      FundTm wl Γ A t ->
+      FundTyEq wl Γ A B -> FundTm wl Γ B t.
   Proof.
-    intros * ?[]?[]; econstructor. 
+    intros * [] []; econstructor. 
     eapply conv; irrValid.
     Unshelve. all: tea.
   Qed.
 
-  Lemma FundTyEqPiCong : forall (Γ : context) (A B C D : term),
-    [Γ |-[ de ] A ] ->
-    FundTy Γ A ->
-    [Γ |-[ de ] A ≅ B] ->
-    FundTyEq Γ A B ->
-    [Γ,, A |-[ de ] C ≅ D] ->
-    FundTyEq (Γ,, A) C D -> FundTyEq Γ (tProd A C) (tProd B D).
+  Lemma FundTyEqPiCong : forall (wl : wfLCon) (Γ : context) (A B C D : term),
+    FundTy wl Γ A ->
+    FundTyEq wl Γ A B ->
+    FundTyEq wl (Γ,, A) C D ->
+    FundTyEq wl Γ (tProd A C) (tProd B D).
   Proof.
-    intros * ?[]?[]?[]; econstructor.
+    intros * [] [] []; econstructor.
     - eapply PiValid. eapply irrelevanceLift; tea; irrValid.
     - eapply PiCong. 1: eapply irrelevanceLift; tea.
       all: irrValid.
     Unshelve. all: tea; irrValid.
   Qed.
 
-  Lemma FundTyEqRefl : forall (Γ : context) (A : term),
-    [Γ |-[ de ] A] -> FundTy Γ A -> FundTyEq Γ A A.
+  Lemma FundTyEqRefl : forall (wl : wfLCon) (Γ : context) (A : term),
+      FundTy wl Γ A -> FundTyEq wl Γ A A.
   Proof.
-    intros * ?[]; unshelve econstructor; tea; now eapply reflValidTy.
+    intros * []; unshelve econstructor; tea; now eapply reflValidTy.
   Qed.
 
-  Lemma FundTyEqSym : forall (Γ : context) (A B : term),
-    [Γ |-[ de ] A ≅ B] -> FundTyEq Γ A B -> FundTyEq Γ B A.
+  Lemma FundTyEqSym : forall (wl : wfLCon) (Γ : context) (A B : term),
+      FundTyEq wl Γ A B -> FundTyEq wl Γ B A.
   Proof.
-    intros * ? [];  unshelve econstructor; tea.
-    now eapply symValidEq.
+    intros * [];  unshelve econstructor; tea.
+    now eapply symValidTyEq.
   Qed.
 
-  Lemma FundTyEqTrans : forall (Γ : context) (A B C : term),
-    [Γ |-[ de ] A ≅ B] -> FundTyEq Γ A B ->
-    [Γ |-[ de ] B ≅ C] -> FundTyEq Γ B C ->
-    FundTyEq Γ A C.
+  Lemma FundTyEqTrans : forall (wl : wfLCon) (Γ : context) (A B C : term),
+      FundTyEq wl Γ A B ->
+      FundTyEq wl Γ B C ->
+      FundTyEq wl Γ A C.
   Proof.
-    intros * ?[]?[]; unshelve econstructor; tea. 1:irrValid.
-    eapply transValidEq; irrValid.
+    intros *  [] []; unshelve econstructor; tea. 1:irrValid.
+    eapply transValidTyEq; irrValid.
     Unshelve. tea.
   Qed.
 
-  Lemma FundTyEqUniv : forall (Γ : context) (A B : term),
-    [Γ |-[ de ] A ≅ B : U] -> FundTmEq Γ U A B -> FundTyEq Γ A B.
+  Lemma FundTyEqUniv : forall (wl : wfLCon) (Γ : context) (A B : term),
+      FundTmEq wl Γ U A B -> FundTyEq wl Γ A B.
   Proof.
-    intros * ?[]; unshelve econstructor; tea.
+    intros * []; unshelve econstructor; tea.
     1,2: now eapply univValid.
     now eapply univEqValid.
   Qed.
 
-  Lemma FundTmEqBRed : forall (Γ : context) (a t A B : term),
-    [Γ |-[ de ] A] ->
-    FundTy Γ A ->
-    [Γ,, A |-[ de ] t : B] ->
-    FundTm (Γ,, A) B t ->
-    [Γ |-[ de ] a : A] ->
-    FundTm Γ A a -> FundTmEq Γ B[a..] (tApp (tLambda A t) a) t[a..].
+  Lemma FundTmEqBRed : forall (wl : wfLCon) (Γ : context) (a t A B : term),
+    FundTy wl Γ A ->
+    FundTm wl (Γ,, A) B t ->
+    FundTm wl Γ A a -> FundTmEq wl Γ B[a..] (tApp (tLambda A t) a) t[a..].
   Proof.
-    intros * ?[]?[]?[]; econstructor.
+    intros *  [] [] []; econstructor.
     - eapply appValid. eapply lamValid. irrValid.
     - unshelve epose (substSTm _ _).
       8-12: irrValid.
-      tea.
+      cbn in *.
+      irrValid.
     - unshelve epose (betaValid VA _ _ _). 2,5-7:irrValid.
       Unshelve. all: tea; try irrValid.
   Qed.
 
-  Lemma FundTmEqPiCong : forall (Γ : context) (A B C D : term),
-    [Γ |-[ de ] A : U] -> FundTm Γ U A ->
-    [Γ |-[ de ] A ≅ B : U] -> FundTmEq Γ U A B ->
-    [Γ,, A |-[ de ] C ≅ D : U] -> FundTmEq (Γ,, A) U C D ->
-    FundTmEq Γ U (tProd A C) (tProd B D).
+
+  Lemma FundTmEqPiCong : forall (wl : wfLCon) (Γ : context) (A B C D : term),
+    FundTm wl Γ U A ->
+    FundTmEq wl Γ U A B ->
+    FundTmEq wl (Γ,, A) U C D ->
+    FundTmEq wl Γ U (tProd A C) (tProd B D).
   Proof.
-    intros * ?[]?[]?[].
-    assert (VA' : [Γ ||-v<one> A | VΓ]) by now eapply univValid.
-    assert [Γ ||-v<one> A ≅ B | VΓ | VA'] by (eapply univEqValid; irrValid).
+    intros * [] [] [].
+    assert (VA' : [Γ ||-v<one> A | VΓ]< wl >) by now eapply univValid.
+    assert [Γ ||-v<one> A ≅ B | VΓ | VA']< wl > by (eapply univEqValid; irrValid).
     opector; tea.
-    - edestruct FundTmProd. 5: irrValid.
-      1,3: eapply ty_sound; now eapply escapeTm.
+    - now eapply UValid.
+    - edestruct FundTmProd. 3: irrValid.
+      2: eauto.
       all: unshelve econstructor; irrValid.
-    - edestruct FundTmProd. 5: irrValid.
-      1,3: eapply ty_sound; eapply escapeTm; tea.
-      1: eapply irrelevanceTmLift; tea; irrValid.
+    - edestruct FundTmProd. 3: irrValid.
       1: unshelve econstructor; irrValid.
-      opector.
-      + eapply validSnoc; now eapply univValid.
-      + eapply irrelevanceLift; irrValid.
+      unshelve econstructor.
+      + eapply validSnoc'; now eapply univValid.
+      + eapply UValid.
       + eapply irrelevanceTmLift; irrValid.
     - unshelve epose (PiCongTm _ _ _ _ _ _ _ _ _ _ _).
-      16: irrValid.
-      2: tea.
-      2,3,8: irrValid.
+      17: irrValid.
+      3: tea.
+      3,4,9: irrValid.
       all: try irrValid.
-      + now eapply univValid.
+      + eapply univValid; irrValid.
       + eapply irrelevanceLift; irrValid.
       + eapply irrelevanceTmLift; irrValid.
       Unshelve.
       all: try irrValid.
-      1: unshelve eapply irrelevanceLift; cycle 3; try irrValid.
-      unshelve eapply univValid; cycle 1; try irrValid.
   Qed.
 
-  Lemma FundTmEqAppCong : forall (Γ : context) (a b f g A B : term),
-    [Γ |-[ de ] f ≅ g : tProd A B] -> FundTmEq Γ (tProd A B) f g ->
-    [Γ |-[ de ] a ≅ b : A] -> FundTmEq Γ A a b ->
-    FundTmEq Γ B[a..] (tApp f a) (tApp g b).
+  Lemma FundTmEqAppCong : forall (wl : wfLCon) (Γ : context) (a b f g A B : term),
+      FundTmEq wl Γ (tProd A B) f g ->
+      FundTmEq wl Γ A a b ->
+    FundTmEq wl Γ B[a..] (tApp f a) (tApp g b).
   Proof.
-    intros * ?[]?[]; econstructor.
+    intros *  [] []; econstructor.
     - eapply appValid; irrValid.
     - eapply conv. 2: eapply appValid; irrValid.
       eapply substSΠeq; try irrValid.
@@ -337,20 +337,181 @@ Section Fundamental.
     - eapply appcongValid; irrValid.
     Unshelve. all: irrValid.
   Qed.
-
-  Lemma FundTmEqFunExt : forall (Γ : context) (f g A B : term),
-    [Γ |-[ de ] A] -> FundTy Γ A ->
-    [Γ |-[ de ] f : tProd A B] -> FundTm Γ (tProd A B) f ->
-    [Γ |-[ de ] g : tProd A B] -> FundTm Γ (tProd A B) g ->
-    [Γ,, A |-[ de ] tApp (f⟨↑⟩) (tRel 0) ≅ tApp (g⟨↑⟩) (tRel 0) : B] -> FundTmEq (Γ,, A) B (tApp (f⟨↑⟩) (tRel 0)) (tApp (g⟨↑⟩) (tRel 0)) ->
-    FundTmEq Γ (tProd A B) f g.
+  
+  Lemma FundTmEqLambdaCong : forall (wl : wfLCon) (Γ : context) (t u A A' A'' B : term),
+    FundTy wl Γ A ->
+    FundTyEq wl Γ A A' ->
+    FundTyEq wl Γ A A'' ->
+    FundTmEq wl (Γ,, A) B t u ->
+    FundTmEq wl Γ (tProd A B) (tLambda A' t) (tLambda A'' u).
   Proof.
-    intros * ?[]?[VΓ0 VA0]?[]?[].
-    assert [Γ ||-v< one > g : tProd A B | VΓ0 | VA0].
+    intros * [VΓ] [? ? VA'] [? ? VA''] [].
+    assert (VΠAB : [Γ ||-v< one > tProd A B | VΓ]< wl >).
+    { unshelve eapply PiValid; irrValid. }
+    assert (VB' : [Γ,, A' ||-v< one > B | validSnoc' _ VA']< wl >).
+    { eapply irrelevanceLift; [tea|]; irrValid. }
+    assert (VB'' : [Γ,, A'' ||-v< one > B | validSnoc' _ VA'']< wl >).
+    { eapply irrelevanceLift; [tea|]; irrValid. }
+    assert (Vλt : [Γ ||-v< one > tLambda A' t : tProd A B | VΓ | VΠAB ]< wl >).
+    { eapply conv; [|eapply lamValid].
+      + eapply symValidTyEq, PiCong; tea; try irrValid.
+        eapply reflValidTy.
+      + eapply irrelevanceTmLift; irrValid.
+    }
+    assert (Vλu : [Γ ||-v< one > tLambda A'' u : tProd A B | VΓ | VΠAB ]< wl >).
+    { eapply conv; [|eapply lamValid].
+      + eapply symValidTyEq, PiCong; tea; try irrValid.
+        eapply reflValidTy.
+      + eapply irrelevanceTmLift; irrValid.
+    }
+    Unshelve. all: try irrValid.
+    assert [Γ,, A ||-v< one > A⟨@wk1 Γ A⟩ | validSnoc' VΓ VA]< wl >.
+    { apply wk1ValidTy; irrValid. }
+    assert (VΓAA' : [Γ,, A ||-v< one > A'⟨@wk1 Γ A⟩ | validSnoc' VΓ VA]< wl >).
+    { apply wk1ValidTy; irrValid. }
+    assert (VΓAA'' : [Γ,, A ||-v< one > A''⟨@wk1 Γ A⟩ | validSnoc' VΓ VA]< wl >).
+    { apply wk1ValidTy; irrValid. }
+    assert (VAdequate (ta := ta) wl (Γ,, A) VR).
+    { now eapply validSnoc'. }
+    assert (VAdequate (ta := ta) wl (Γ,, A,, A'⟨@wk1 Γ A⟩) VR).
+    { unshelve eapply validSnoc'; tea; try irrValid. }
+    assert (VAdequate (ta := ta) wl (Γ,, A,, A''⟨@wk1 Γ A⟩) VR).
+    { unshelve eapply validSnoc'; tea; try irrValid. }
+    assert (eq0 : forall t, t⟨upRen_term_term ↑⟩[(tRel 0)..] = t).
+    { clear; intros; bsimpl; apply idSubst_term; intros []; reflexivity. }
+    econstructor; tea.
+    eapply irrelevanceTmEq, etaeqValid; try irrValid.
+    eapply transValidTmEq; [|eapply transValidTmEq]; [|eapply irrelevanceTmEq; tea|].
+    + eapply irrelevanceTmEq'; [eapply eq0|].
+      eapply transValidTmEq; [eapply betaValid|]; refold.
+      - eapply irrelevanceTm'.
+        2: eapply (wkValidTm  (A := B)) with (ρ := wk_up A' (@wk1 Γ A)).
+        * now bsimpl.
+        * eapply irrelevanceTmLift; irrValid.
+      - eapply irrelevanceTmEq'; [symmetry; eapply eq0|].
+        match goal with |- [_ ||-v< _ > ?t ≅ ?u : _ | _ | _ ]< wl > => assert (Hrw : t = u) end.
+        { bsimpl; apply idSubst_term; intros []; reflexivity. }
+        set (t' := t) at 2; rewrite Hrw.
+        apply reflValidTm; tea.
+    + apply symValidTmEq; eapply irrelevanceTmEq'; [eapply eq0|].
+      eapply transValidTmEq; [eapply betaValid|]; refold.
+      - eapply irrelevanceTm'.
+        2: eapply (wkValidTm  (A := B)) with (ρ := wk_up A'' (@wk1 Γ A)).
+        * now bsimpl.
+        * eapply irrelevanceTmLift; irrValid.
+      - eapply irrelevanceTmEq'; [symmetry; eapply eq0|].
+        match goal with |- [_ ||-v< _ > ?t ≅ ?u : _ | _ | _ ]< wl > => assert (Hrw : t = u) end.
+        { bsimpl; apply idSubst_term; intros []; reflexivity. }
+        set (u' := u) at 2; rewrite Hrw.
+        apply reflValidTm; tea.
+    Unshelve.
+    all: refold; try irrValid.
+    * unshelve eapply irrelevanceTy; tea.
+      rewrite <- (wk_up_wk1_ren_on Γ A' A).
+      eapply wkValidTy, irrelevanceLift; irrValid.
+    * eapply conv; [now eapply irrelevanceTyEq, wk1ValidTyEq|].
+      eapply irrelevanceTm'; [symmetry; eapply wk1_ren_on|].
+      eapply var0Valid'.
+    * eapply irrelevanceTy.
+      rewrite <- (wk_up_wk1_ren_on Γ A'' A).
+      eapply wkValidTy, irrelevanceLift; irrValid.
+    * eapply conv; [now eapply irrelevanceTyEq, wk1ValidTyEq|].
+      eapply irrelevanceTm'; [symmetry; eapply wk1_ren_on|].
+      eapply var0Valid'.
+  Unshelve.
+  all: try irrValid.
+  2,4: rewrite <- (wk1_ren_on Γ A); irrValid.
+  Qed.
+
+
+  Lemma FundTmEqFunEta : forall (wl : wfLCon) (Γ : context) (f A B : term),
+    FundTm wl Γ (tProd A B) f -> FundTmEq wl Γ (tProd A B) (tLambda A (tApp f⟨↑⟩ (tRel 0))) f.
+  Proof.
+  intros * [VΓ VΠ Vf].
+  assert (eq0 : forall t, t⟨upRen_term_term ↑⟩[(tRel 0)..] = t).
+  { clear; intros; bsimpl; apply idSubst_term; intros []; reflexivity. }
+  assert (VA : [Γ ||-v< one > A | VΓ]< wl >).
+  { now eapply PiValidDom. }
+  assert (VΓA := validSnoc' VΓ VA).
+  assert (VΓAA : [Γ,, A ||-v< one > A⟨@wk1 Γ A⟩ | VΓA]< wl >).
+  { now eapply irrelevanceTy, wk1ValidTy. }
+  assert (VΓAA0 : VAdequate (ta := ta) wl (Γ,, A,, A⟨@wk1 Γ A⟩) VR).
+  { now eapply validSnoc'. }
+  assert (VΓAA' : [Γ,, A ||-v< one > A⟨↑⟩ | VΓA]< wl >).
+  { now rewrite wk1_ren_on in VΓAA. }
+  assert [Γ,, A ||-v< one > B | VΓA]< wl >.
+  { eapply irrelevanceTy, PiValidCod. }
+  assert ([Γ,, A ||-v< one > tProd A⟨@wk1 Γ A⟩ B⟨upRen_term_term ↑⟩ | VΓA]< wl >).
+  { rewrite <- (wk_up_wk1_ren_on Γ A A).
+    now eapply irrelevanceTy, (wk1ValidTy (A := tProd A B)). }
+  assert ([Γ,, A ||-v< one > tRel 0 : A⟨wk1 A⟩ | VΓA | VΓAA]< wl >).
+  { eapply irrelevanceTm'; [rewrite wk1_ren_on; reflexivity|].
+    unshelve apply var0Valid'. }
+  assert ([(Γ,, A),, A⟨wk1 A⟩ ||-v< one > tProd A⟨↑⟩⟨↑⟩ B⟨upRen_term_term ↑⟩⟨upRen_term_term ↑⟩ | VΓAA0]< wl >).
+  { assert (eq1 : (tProd A B)⟨@wk1 Γ A⟩⟨@wk1 (Γ,, A) A⟨@wk1 Γ A⟩⟩ = tProd (A⟨↑⟩⟨↑⟩) (B⟨upRen_term_term ↑⟩⟨upRen_term_term ↑⟩)).
+    { rewrite wk1_ren_on, wk1_ren_on; reflexivity. }
+    eapply irrelevanceTy'; [|eapply eq1|reflexivity].
+    now eapply wkValidTy, wkValidTy. }
+  assert ([Γ ||-v< one > tLambda A (tApp f⟨↑⟩ (tRel 0)) : tProd A B | VΓ | VΠ]< wl >).
+  { eapply irrelevanceTm, lamValid.
+    eapply irrelevanceTm'; [apply eq0|eapply (appValid (F := A⟨@wk1 Γ A⟩))].
+    rewrite <- (wk1_ren_on Γ A).
+    eapply irrelevanceTm'; [|now eapply wkValidTm].
+    rewrite <- (wk_up_wk1_ren_on Γ A A).
+    reflexivity. }
+  Unshelve. all: try irrValid.
+  econstructor; tea.
+  eapply irrelevanceTmEq, etaeqValid; try irrValid.
+  eapply transValidTmEq; refold.
+  + eapply irrelevanceTmEq'; [eapply eq0|].
+    eapply betaValid; refold.
+    eapply irrelevanceTm'; [apply eq0|].
+    eapply appValid.
+    rewrite <- shift_upRen.
+    assert (eq1 : (tProd A B)⟨@wk1 Γ A⟩⟨@wk1 (Γ,, A) A⟨@wk1 Γ A⟩⟩ = tProd (A⟨↑⟩⟨↑⟩) (B⟨upRen_term_term ↑⟩⟨upRen_term_term ↑⟩)).
+    { rewrite wk1_ren_on, wk1_ren_on; reflexivity. }
+    eapply irrelevanceTm'; [eapply eq1|].
+    rewrite <- (wk1_ren_on (Γ,, A)  A⟨@wk1 Γ A⟩).
+    now eapply wkValidTm, wkValidTm.
+  + refold.
+    match goal with |- [_ ||-v< _ > ?t ≅ ?u : _ | _ | _ ]< wl > => assert (Hrw : t = u) end.
+    { rewrite <- eq0; now bsimpl. }
+    rewrite Hrw.
+    apply reflValidTm; tea.
+    eapply irrelevanceTm'; [apply eq0|].
+    eapply (appValid (F := A⟨@wk1 Γ A⟩)).
+    eapply irrelevanceTm'; [|now eapply wk1ValidTm].
+    now rewrite <- (wk_up_wk1_ren_on Γ A A).
+  Unshelve.
+  all: refold; try irrValid.
+  { unshelve eapply irrelevanceTy; [tea|].
+    rewrite <- (wk_up_wk1_ren_on Γ A A).
+    now eapply wkValidTy. }
+  { eapply (irrelevanceTy' (A := A⟨↑⟩⟨@wk1 (Γ,, A) A⟨@wk1 Γ A⟩⟩)); [|now rewrite wk1_ren_on|reflexivity].
+    now eapply wkValidTy. }
+  { eapply (irrelevanceTm' (A := A⟨@wk1 Γ A⟩⟨↑⟩)); [now rewrite wk1_ren_on|].
+    apply var0Valid'. }
+  Unshelve.
+  all: try irrValid.
+  { shelve. }
+  { rewrite <- (wk1_ren_on (Γ,, A)  A⟨@wk1 Γ A⟩).
+    now eapply wkValidTy. }
+  Qed.
+
+
+  Lemma FundTmEqFunExt : forall (wl : wfLCon) (Γ : context) (f g A B : term),
+      FundTy wl Γ A ->
+      FundTm wl Γ (tProd A B) f ->
+      FundTm wl Γ (tProd A B) g ->
+     FundTmEq wl (Γ,, A) B (tApp (f⟨↑⟩) (tRel 0)) (tApp (g⟨↑⟩) (tRel 0)) ->
+     FundTmEq wl Γ (tProd A B) f g.
+  Proof.
+    intros *  [] [VΓ0 VA0] [] [].
+    assert [Γ ||-v< one > g : tProd A B | VΓ0 | VA0]< wl >.
     1:{
       eapply conv. 
       2: irrValid.
-      eapply symValidEq. eapply PiCong.
+      eapply symValidTyEq. eapply PiCong.
       eapply irrelevanceLift. 
       1,3,4: eapply reflValidTy.
       irrValid.
@@ -361,136 +522,173 @@ Section Fundamental.
     Unshelve. all: irrValid.
   Qed.
 
-  Lemma FundTmEqRefl : forall (Γ : context) (t A : term),
-    [Γ |-[ de ] t : A] -> FundTm Γ A t ->
-    FundTmEq Γ A t t.
+  Lemma FundTmEqRefl : forall (wl : wfLCon) (Γ : context) (t A : term),
+      FundTm wl Γ A t ->
+      FundTmEq wl Γ A t t.
   Proof.
-    intros * ?[]; econstructor; tea; now eapply reflValidTm.
+    intros * []; econstructor; tea; now eapply reflValidTm.
   Qed.
 
-  Lemma FundTmEqSym : forall (Γ : context) (t t' A : term),
-    [Γ |-[ de ] t ≅ t' : A] -> FundTmEq Γ A t t' ->
-    FundTmEq Γ A t' t.
+  Lemma FundTmEqSym : forall (wl : wfLCon) (Γ : context) (t t' A : term),
+      FundTmEq wl Γ A t t' ->
+      FundTmEq wl Γ A t' t.
   Proof.
-    intros * ?[]; econstructor; tea; now eapply symValidTmEq.
+    intros * []; econstructor; tea; now eapply symValidTmEq.
   Qed.
 
-  Lemma FundTmEqTrans : forall (Γ : context) (t t' t'' A : term),
-    [Γ |-[ de ] t ≅ t' : A] -> FundTmEq Γ A t t' ->
-    [Γ |-[ de ] t' ≅ t'' : A] -> FundTmEq Γ A t' t'' ->
-    FundTmEq Γ A t t''.
+  Lemma FundTmEqTrans : forall (wl : wfLCon) (Γ : context) (t t' t'' A : term),
+      FundTmEq wl Γ A t t' ->
+      FundTmEq wl Γ A t' t'' ->
+    FundTmEq wl Γ A t t''.
   Proof.
-    intros * ?[]?[]; econstructor; tea.
+    intros *  [] []; econstructor; tea.
     1: irrValid.
     eapply transValidTmEq; irrValid.
   Qed.
 
-  Lemma FundTmEqConv : forall (Γ : context) (t t' A B : term),
-    [Γ |-[ de ] t ≅ t' : A] -> FundTmEq Γ A t t' ->
-    [Γ |-[ de ] A ≅ B] -> FundTyEq Γ A B ->
-    FundTmEq Γ B t t'.
+  Lemma FundTmEqConv : forall (wl : wfLCon) (Γ : context) (t t' A B : term),
+      FundTmEq wl Γ A t t' ->
+      FundTyEq wl Γ A B ->
+    FundTmEq wl Γ B t t'.
   Proof.
-    intros * ?[]?[]; econstructor.
+    intros *  [] []; econstructor.
     1,2: eapply conv; irrValid.
     eapply convEq; irrValid.
     Unshelve. all: irrValid.
   Qed.
 
-  Lemma FundTyNat : forall Γ : context, [ |-[ de ] Γ] -> FundCon Γ -> FundTy Γ tNat.
+  Lemma FundTyNat : forall (wl : wfLCon) (Γ : context),
+      FundCon wl Γ -> FundTy wl Γ tNat.
   Proof.
     intros ???; unshelve econstructor; tea;  eapply natValid.
   Qed.
 
-  Lemma FundTmNat : forall Γ : context, [ |-[ de ] Γ] -> FundCon Γ -> FundTm Γ U tNat.
+  Lemma FundTmNat : forall (wl : wfLCon) (Γ : context),
+      FundCon wl Γ -> FundTm wl Γ U tNat.
   Proof.
     intros ???; unshelve econstructor; tea.
     2: eapply natTermValid.
   Qed.
 
-  Lemma FundTmZero : forall Γ : context, [ |-[ de ] Γ] -> FundCon Γ -> FundTm Γ tNat tZero.
+  Lemma FundTmZero : forall (wl : wfLCon) (Γ : context), FundCon wl Γ -> FundTm wl Γ tNat tZero.
   Proof.
     intros; unshelve econstructor; tea. 
     2:eapply zeroValid.
   Qed.
 
-  Lemma FundTmSucc : forall (Γ : context) (n : term),
-    [Γ |-[ de ] n : tNat] -> FundTm Γ tNat n -> FundTm Γ tNat (tSucc n).
+  Lemma FundTmSucc : forall (wl : wfLCon) (Γ : context) (n : term),
+      FundTm wl Γ tNat n -> FundTm wl Γ tNat (tSucc n).
   Proof.
-    intros * ?[]; unshelve econstructor; tea.
+    intros * []; unshelve econstructor; tea.
     eapply irrelevanceTm; eapply succValid; irrValid.
     Unshelve. tea.
   Qed.
 
-  Lemma FundTmNatElim : forall (Γ : context) (P hz hs n : term),
-    [Γ,, tNat |-[ de ] P] ->
-    FundTy (Γ,, tNat) P ->
-    [Γ |-[ de ] hz : P[tZero..]] ->
-    FundTm Γ P[tZero..] hz ->
-    [Γ |-[ de ] hs : elimSuccHypTy P] ->
-    FundTm Γ (elimSuccHypTy P) hs ->
-    [Γ |-[ de ] n : tNat] ->
-    FundTm Γ tNat n -> FundTm Γ P[n..] (tNatElim P hz hs n).
+  Lemma FundTmNatElim : forall (wl : wfLCon) (Γ : context) (P hz hs n : term),
+    FundTy wl (Γ,, tNat) P ->
+    FundTm wl Γ P[tZero..] hz ->
+    FundTm wl Γ (elimSuccHypTy P) hs ->
+    FundTm wl Γ tNat n -> FundTm wl Γ P[n..] (tNatElim P hz hs n).
   Proof.
-    intros * ?[]?[]?[]?[]; unshelve econstructor; tea.
+    intros *  [] [] [] []; unshelve econstructor; tea.
     2: eapply natElimValid; irrValid.
     Unshelve. all: irrValid.
   Qed.
 
-  Lemma FundTyEmpty : forall Γ : context, [ |-[ de ] Γ] -> FundCon Γ -> FundTy Γ tEmpty.
+  Lemma FundTyBool : forall (wl : wfLCon) (Γ : context),
+      FundCon wl Γ -> FundTy wl Γ tBool.
+  Proof.
+    intros ???; unshelve econstructor; tea;  eapply boolValid.
+  Qed.
+
+  Lemma FundTmBool : forall (wl : wfLCon) (Γ : context),
+      FundCon wl Γ -> FundTm wl Γ U tBool.
+  Proof.
+    intros ???; unshelve econstructor; tea.
+    2: eapply boolTermValid.
+  Qed.
+
+  Lemma FundTmTrue : forall (wl : wfLCon) (Γ : context), FundCon wl Γ -> FundTm wl Γ tBool tTrue.
+  Proof.
+    intros; unshelve econstructor; tea. 
+    2:eapply trueValid.
+  Qed.
+
+  Lemma FundTmFalse : forall (wl : wfLCon) (Γ : context), FundCon wl Γ -> FundTm wl Γ tBool tFalse.
+  Proof.
+    intros; unshelve econstructor; tea. 
+    2:eapply falseValid.
+  Qed.
+
+  Lemma FundTmAlpha : forall (wl : wfLCon) (Γ : context) (n : term),
+      FundTm wl Γ tNat n -> FundTm wl Γ tBool (tAlpha n).
+  Proof.
+    intros * []; unshelve econstructor; tea.
+    1: now eapply boolValid.
+    eapply irrelevanceTm; eapply alphaValid; irrValid.
+    Unshelve. tea.
+  Qed.
+
+  Lemma FundTmBoolElim : forall (wl : wfLCon) (Γ : context) (P ht hf n : term),
+    FundTy wl (Γ,, tBool) P ->
+    FundTm wl Γ P[tTrue..] ht ->
+    FundTm wl Γ P[tFalse..] hf ->
+    FundTm wl Γ tBool n ->
+    FundTm wl Γ P[n..] (tBoolElim P ht hf n).
+  Proof.
+    intros *  [] [] [] []; unshelve econstructor; tea.
+    2: eapply boolElimValid; irrValid.
+    Unshelve. all: irrValid.
+  Qed.
+  
+  Lemma FundTyEmpty : forall (wl : wfLCon) (Γ : context), FundCon wl Γ -> FundTy wl Γ tEmpty.
   Proof.
     intros ???; unshelve econstructor; tea;  eapply emptyValid.
   Qed.
 
-  Lemma FundTmEmpty : forall Γ : context, [ |-[ de ] Γ] -> FundCon Γ -> FundTm Γ U tEmpty.
+  Lemma FundTmEmpty : forall (wl : wfLCon) (Γ : context), [ |-[ de ] Γ]< wl > -> FundCon wl Γ -> FundTm wl Γ U tEmpty.
   Proof.
     intros ???; unshelve econstructor; tea.
     2: eapply emptyTermValid.
   Qed.
 
-  Lemma FundTmEmptyElim : forall (Γ : context) (P n : term),
-    [Γ,, tEmpty |-[ de ] P] ->
-    FundTy (Γ,, tEmpty) P ->
-    [Γ |-[ de ] n : tEmpty] ->
-    FundTm Γ tEmpty n -> FundTm Γ P[n..] (tEmptyElim P n).
+  Lemma FundTmEmptyElim : forall (wl : wfLCon) (Γ : context) (P n : term),
+    FundTy wl (Γ,, tEmpty) P ->
+    FundTm wl Γ tEmpty n -> FundTm wl Γ P[n..] (tEmptyElim P n).
   Proof.
-    intros * ?[]?[]; unshelve econstructor; tea.
+    intros *  [] []; unshelve econstructor; tea.
     2: eapply emptyElimValid; irrValid.
     Unshelve. 1,2: irrValid. 
   Qed.
 
-  Lemma FundTmEqSuccCong : forall (Γ : context) (n n' : term),
-    [Γ |-[ de ] n ≅ n' : tNat] ->
-    FundTmEq Γ tNat n n' -> FundTmEq Γ tNat (tSucc n) (tSucc n').
+  Lemma FundTmEqSuccCong : forall (wl : wfLCon) (Γ : context) (n n' : term),
+      FundTmEq wl Γ tNat n n' -> FundTmEq wl Γ tNat (tSucc n) (tSucc n').
   Proof.
-    intros * ?[]; unshelve econstructor; tea.
+    intros * []; unshelve econstructor; tea.
     1,2: eapply irrelevanceTm; eapply succValid; irrValid.
     eapply irrelevanceTmEq; eapply succcongValid; irrValid.
     Unshelve. all: tea.
   Qed.
 
-  Lemma FundTmEqNatElimCong : forall (Γ : context)
+  Lemma FundTmEqNatElimCong : forall (wl : wfLCon) (Γ : context)
       (P P' hz hz' hs hs' n n' : term),
-    [Γ,, tNat |-[ de ] P ≅ P'] ->
-    FundTyEq (Γ,, tNat) P P' ->
-    [Γ |-[ de ] hz ≅ hz' : P[tZero..]] ->
-    FundTmEq Γ P[tZero..] hz hz' ->
-    [Γ |-[ de ] hs ≅ hs' : elimSuccHypTy P] ->
-    FundTmEq Γ (elimSuccHypTy P) hs hs' ->
-    [Γ |-[ de ] n ≅ n' : tNat] ->
-    FundTmEq Γ tNat n n' ->
-    FundTmEq Γ P[n..] (tNatElim P hz hs n) (tNatElim P' hz' hs' n').
+    FundTyEq wl (Γ,, tNat) P P' ->
+    FundTmEq wl Γ P[tZero..] hz hz' ->
+    FundTmEq wl Γ (elimSuccHypTy P) hs hs' ->
+    FundTmEq wl Γ tNat n n' ->
+    FundTmEq wl Γ P[n..] (tNatElim P hz hs n) (tNatElim P' hz' hs' n').
   Proof.
-    intros * ?[? VP0 VP0']?[VΓ0]?[]?[].
+    intros * [? VP0 VP0'] [VΓ0] [] [].
     pose (VN := natValid (l:=one) VΓ0).
-    assert (VP' : [ _ ||-v<one> P' | validSnoc VΓ0 VN]) by irrValid. 
-    assert [Γ ||-v< one > hz' : P'[tZero..] | VΓ0 | substS VP' (zeroValid VΓ0)]. 1:{
+    assert (VP' : [ _ ||-v<one> P' | validSnoc' VΓ0 VN]< wl >) by irrValid. 
+    assert [Γ ||-v< one > hz' : P'[tZero..] | VΓ0 | substS VP' (zeroValid VΓ0)]< wl >. 1:{
       eapply conv. 2: irrValid.
       eapply substSEq. 2,3: irrValid.
       1: eapply reflValidTy.
       2: eapply reflValidTm.
       all: eapply zeroValid.
     }
-    assert [Γ ||-v< one > hs' : elimSuccHypTy P' | VΓ0 | elimSuccHypTyValid VΓ0 VP']. 1:{
+    assert [Γ ||-v< one > hs' : elimSuccHypTy P' | VΓ0 | elimSuccHypTyValid VΓ0 VP']< wl >. 1:{
       eapply conv. 2: irrValid.
       eapply elimSuccHypTyCongValid; irrValid.
     } 
@@ -498,7 +696,7 @@ Section Fundamental.
     2: eapply natElimValid; irrValid.
     + eapply conv.
       2: eapply irrelevanceTm; now eapply natElimValid.
-      eapply symValidEq. 
+      eapply symValidTyEq. 
       eapply substSEq; tea. 
       2,3: irrValid.
       eapply reflValidTy.
@@ -508,35 +706,28 @@ Section Fundamental.
     1: unshelve eapply substS; try irrValid.
   Qed.
 
-  Lemma FundTmEqNatElimZero : forall (Γ : context) (P hz hs : term),
-    [Γ,, tNat |-[ de ] P] ->
-    FundTy (Γ,, tNat) P ->
-    [Γ |-[ de ] hz : P[tZero..]] ->
-    FundTm Γ P[tZero..] hz ->
-    [Γ |-[ de ] hs : elimSuccHypTy P] ->
-    FundTm Γ (elimSuccHypTy P) hs ->
-    FundTmEq Γ P[tZero..] (tNatElim P hz hs tZero) hz.
+  Lemma FundTmEqNatElimZero : forall (wl : wfLCon) (Γ : context) (P hz hs : term),
+    FundTy wl (Γ,, tNat) P ->
+    FundTm wl Γ P[tZero..] hz ->
+    FundTm wl Γ (elimSuccHypTy P) hs ->
+    FundTmEq wl Γ P[tZero..] (tNatElim P hz hs tZero) hz.
   Proof.
-    intros * ?[]?[]?[]; unshelve econstructor; tea.
+    intros * [] [] []; unshelve econstructor; tea.
     3: irrValid.
     3: eapply natElimZeroValid; irrValid.
     eapply natElimValid; irrValid.
     Unshelve. irrValid.
   Qed.
 
-  Lemma FundTmEqNatElimSucc : forall (Γ : context) (P hz hs n : term),
-    [Γ,, tNat |-[ de ] P] ->
-    FundTy (Γ,, tNat) P ->
-    [Γ |-[ de ] hz : P[tZero..]] ->
-    FundTm Γ P[tZero..] hz ->
-    [Γ |-[ de ] hs : elimSuccHypTy P] ->
-    FundTm Γ (elimSuccHypTy P) hs ->
-    [Γ |-[ de ] n : tNat] ->
-    FundTm Γ tNat n ->
-    FundTmEq Γ P[(tSucc n)..] (tNatElim P hz hs (tSucc n))
+  Lemma FundTmEqNatElimSucc : forall (wl : wfLCon) (Γ : context) (P hz hs n : term),
+    FundTy wl (Γ,, tNat) P ->
+    FundTm wl Γ P[tZero..] hz ->
+    FundTm wl Γ (elimSuccHypTy P) hs ->
+    FundTm wl Γ tNat n ->
+    FundTmEq wl Γ P[(tSucc n)..] (tNatElim P hz hs (tSucc n))
       (tApp (tApp hs n) (tNatElim P hz hs n)).
   Proof.
-    intros * ?[]?[]?[]?[]; unshelve econstructor; tea.
+    intros *  [] [] [] []; unshelve econstructor; tea.
     4: eapply natElimSuccValid; irrValid.
     1: eapply natElimValid; irrValid.
     eapply simple_appValid.
@@ -550,22 +741,115 @@ Section Fundamental.
     eapply succValid; irrValid.
   Qed.
 
-  Lemma FundTmEqEmptyElimCong : forall (Γ : context)
-      (P P' n n' : term),
-    [Γ,, tEmpty |-[ de ] P ≅ P'] ->
-    FundTyEq (Γ,, tEmpty) P P' ->
-    [Γ |-[ de ] n ≅ n' : tEmpty] ->
-    FundTmEq Γ tEmpty n n' ->
-    FundTmEq Γ P[n..] (tEmptyElim P n) (tEmptyElim P' n').
+  Lemma FundTmEqBoolElimCong : forall (wl : wfLCon) (Γ : context)
+      (P P' ht ht' hf hf' n n' : term),
+    FundTyEq wl (Γ,, tBool) P P' ->
+    FundTmEq wl Γ P[tTrue..] ht ht' ->
+    FundTmEq wl Γ P[tFalse..] hf hf' ->
+    FundTmEq wl Γ tBool n n' ->
+    FundTmEq wl Γ P[n..] (tBoolElim P ht hf n) (tBoolElim P' ht' hf' n').
   Proof.
-    intros * ?[? VP0 VP0']?[VΓ0].
+    intros * [? VP0 VP0'] [VΓ0] [] [].
+    pose (VN := boolValid (l:=one) VΓ0).
+    assert (VP' : [ _ ||-v<one> P' | validSnoc' VΓ0 VN]< wl >) by irrValid. 
+    assert [Γ ||-v< one > ht' : P'[tTrue..] | VΓ0 | substS VP' (trueValid VΓ0)]< wl >. 1:{
+      eapply conv. 2: irrValid.
+      eapply substSEq. 2,3: irrValid.
+      1: eapply reflValidTy.
+      2: eapply reflValidTm.
+      all: eapply trueValid.
+    }
+    assert [Γ ||-v< one > hf' : P'[tFalse..] | VΓ0 | substS VP' (falseValid VΓ0)]< wl >. 1:{
+      eapply conv. 2: irrValid.
+      eapply substSEq. 2,3: irrValid.
+      1: eapply reflValidTy.
+      2: eapply reflValidTm.
+      all: eapply falseValid.
+    }
+    unshelve econstructor; tea.
+    2: eapply boolElimValid; irrValid.
+    + eapply conv.
+      2: eapply irrelevanceTm; now eapply boolElimValid.
+      eapply symValidTyEq. 
+      eapply substSEq; tea. 
+      2,3: irrValid.
+      eapply reflValidTy.
+    + eapply boolElimCongValid; tea; try irrValid.
+    Unshelve. all: try irrValid.
+    1: eapply trueValid.
+    1: eapply falseValid.
+    1: unshelve eapply substS; try irrValid.
+  Qed.
+
+  Lemma FundTmEqBoolElimTrue : forall (wl : wfLCon) (Γ : context) (P ht hf : term),
+    FundTy wl (Γ,, tBool) P ->
+    FundTm wl Γ P[tTrue..] ht ->
+    FundTm wl Γ P[tFalse..] hf ->
+    FundTmEq wl Γ P[tTrue..] (tBoolElim P ht hf tTrue) ht.
+  Proof.
+    intros * [] [] []; unshelve econstructor; tea.
+    3: irrValid.
+    3: eapply boolElimTrueValid; irrValid.
+    eapply boolElimValid; irrValid.
+    Unshelve. irrValid.
+  Qed.
+
+  Lemma FundTmEqBoolElimFalse : forall (wl : wfLCon) (Γ : context) (P ht hf : term),
+    FundTy wl (Γ,, tBool) P ->
+    FundTm wl Γ P[tTrue..] ht ->
+    FundTm wl Γ P[tFalse..] hf ->
+    FundTmEq wl Γ P[tFalse..] (tBoolElim P ht hf tFalse) hf.
+  Proof.
+    intros * [] [] []; unshelve econstructor.
+    1: tea.
+    3: irrValid.
+    3: eapply boolElimFalseValid; irrValid.
+    eapply boolElimValid; irrValid.
+    Unshelve. irrValid.
+  Qed.
+
+  Lemma FundTmEqAlphaCong : forall (wl : wfLCon) (Γ : context) (n n' : term),
+      FundTmEq wl Γ tNat n n' -> FundTmEq wl Γ tBool (tAlpha n) (tAlpha n').
+  Proof.
+    intros * []; unshelve econstructor; tea.
+    1: now eapply boolValid.
+    1,2: eapply irrelevanceTm; eapply alphaValid; irrValid.
+    eapply irrelevanceTmEq; eapply alphacongValid; irrValid.
+    Unshelve. all: tea.
+  Qed.
+
+  Lemma FundTmEqAlpha : forall (wl : wfLCon) (Γ : context) (n : nat) (b : bool),
+      FundCon wl Γ -> in_LCon wl n b ->
+      FundTmEq wl Γ tBool (tAlpha (nat_to_term n)) (bool_to_term b).
+  Proof.
+    intros * wfG Hin.
+    unshelve econstructor.
+    - eassumption.
+    - now eapply boolValid.
+    - eapply alphaValid.
+      clear Hin ; induction n.
+      + now eapply zeroValid.
+      + cbn ; now eapply succValid.
+    - destruct b.
+      + now eapply trueValid.
+      + now eapply falseValid.
+    - now eapply alphacongValidSubst.
+  Qed.
+  
+  Lemma FundTmEqEmptyElimCong : forall (wl : wfLCon) (Γ : context)
+      (P P' n n' : term),
+    FundTyEq wl (Γ,, tEmpty) P P' ->
+    FundTmEq wl Γ tEmpty n n' ->
+    FundTmEq wl Γ P[n..] (tEmptyElim P n) (tEmptyElim P' n').
+  Proof.
+    intros * [? VP0 VP0'] [VΓ0].
     pose (VN := emptyValid (l:=one) VΓ0).
-    assert (VP' : [ _ ||-v<one> P' | validSnoc VΓ0 VN]) by irrValid.
+    assert (VP' : [ _ ||-v<one> P' | validSnoc' VΓ0 VN]< wl >) by irrValid.
     unshelve econstructor; tea.
     2: eapply emptyElimValid; irrValid.
     + eapply conv.
       2: eapply irrelevanceTm; now eapply emptyElimValid.
-      eapply symValidEq.
+      eapply symValidTyEq.
       eapply substSEq; tea.
       2,3: irrValid.
       eapply reflValidTy.
@@ -574,61 +858,626 @@ Section Fundamental.
     1: unshelve eapply substS; try irrValid.
   Qed.
 
-Lemma Fundamental : (forall Γ : context, [ |-[ de ] Γ ] -> FundCon (ta := ta) Γ)
-    × (forall (Γ : context) (A : term), [Γ |-[ de ] A] -> FundTy (ta := ta) Γ A)
-    × (forall (Γ : context) (A t : term), [Γ |-[ de ] t : A] -> FundTm (ta := ta) Γ A t)
-    × (forall (Γ : context) (A B : term), [Γ |-[ de ] A ≅ B] -> FundTyEq (ta := ta) Γ A B)
-    × (forall (Γ : context) (A t u : term), [Γ |-[ de ] t ≅ u : A] -> FundTmEq (ta := ta) Γ A t u).
+
+  Lemma FundTySig : forall wl (Γ : context) (A B : term),
+  FundTy wl Γ A -> FundTy wl (Γ,, A) B -> FundTy wl Γ (tSig A B).
   Proof.
-  apply WfDeclInduction.
-  + apply FundConNil.
-  + apply FundConCons.
-  + apply FundTyU.
-  + apply FundTyPi.
-  + apply FundTyNat.
-  + apply FundTyEmpty.
-  + apply FundTyUniv.
-  + apply FundTmVar.
-  + apply FundTmProd.
-  + apply FundTmLambda.
-  + apply FundTmApp.
-  + apply FundTmNat.
-  + apply FundTmZero.
-  + apply FundTmSucc.
-  + apply FundTmNatElim.
-  + apply FundTmEmpty.
-  + apply FundTmEmptyElim.
-  + apply FundTmConv.
-  + apply FundTyEqPiCong.
-  + apply FundTyEqRefl.
-  + apply FundTyEqUniv.
-  + apply FundTyEqSym.
-  + apply FundTyEqTrans.
-  + apply FundTmEqBRed.
-  + apply FundTmEqPiCong.
-  + apply FundTmEqAppCong.
-  + apply FundTmEqFunExt.
-  + apply FundTmEqSuccCong.
-  + apply FundTmEqNatElimCong.
-  + apply FundTmEqNatElimZero.
-  + apply FundTmEqNatElimSucc.
-  + apply FundTmEqEmptyElimCong.
-  + apply FundTmEqRefl.
-  + apply FundTmEqConv.
-  + apply FundTmEqSym.
-  + apply FundTmEqTrans.
+    intros * [] []; unshelve econstructor; tea.
+    unshelve eapply SigValid; tea; irrValid.
+  Qed.
+
+  Lemma FundTmSig : forall wl (Γ : context) (A B : term),
+    FundTm wl Γ U A ->
+    FundTm wl (Γ,, A) U B -> FundTm wl Γ U (tSig A B).
+  Proof.
+    intros * [] []; unshelve econstructor.
+    3: unshelve eapply SigValidU.
+    3-5: irrValid.
+    1: tea.
+    unshelve eapply univValid; tea.
+  Qed.
+
+  Lemma FundTmPair : forall wl (Γ : context) (A B a b : term),
+    FundTy wl Γ A ->
+    FundTy wl (Γ,, A) B ->
+    FundTm wl Γ A a ->
+    FundTm wl Γ B[a..] b -> FundTm wl Γ (tSig A B) (tPair A B a b).
+  Proof.
+    intros * [] [] [] []; unshelve econstructor.
+    3: unshelve eapply pairValid; irrValid.
+    tea.
+  Qed.
+
+  Lemma FundTmFst : forall wl (Γ : context) (A B p : term),
+    FundTm wl Γ (tSig A B) p -> FundTm wl Γ A (tFst p).
+  Proof.
+    intros * []; unshelve econstructor.
+    3: unshelve eapply fstValid.
+    5: irrValid.
+    2: now eapply domSigValid.
+    now eapply codSigValid.
+  Qed.
+
+  Lemma FundTmSnd : forall wl (Γ : context) (A B p : term),
+    FundTm wl Γ (tSig A B) p -> FundTm wl Γ B[(tFst p)..] (tSnd p).
+  Proof.
+    intros * []; unshelve econstructor.
+    3: unshelve eapply sndValid.
+    5: irrValid.
+    2: now eapply domSigValid.
+    now eapply codSigValid.
+  Qed.
+
+  Lemma FundTyEqSigCong : forall wl (Γ : context) (A B C D : term),
+    FundTy wl Γ A ->
+    FundTyEq wl Γ A B ->
+    FundTyEq wl (Γ,, A) C D -> FundTyEq wl Γ (tSig A C) (tSig B D).
+  Proof.
+    intros * [] [] [].
+    unshelve econstructor.
+    4: eapply SigCong; tea; try irrValid.
+    2: eapply irrelevanceLift; irrValid.
+    eapply SigValid; eapply irrelevanceLift; irrValid.
+    Unshelve. all: irrValid.
+  Qed.
+
+  Lemma FundTmEqSigCong :forall wl (Γ : context) (A A' B B' : term),
+    FundTm wl Γ U A ->
+    FundTmEq wl Γ U A A' ->
+    FundTmEq wl (Γ,, A) U B B' -> FundTmEq wl Γ U (tSig A B) (tSig A' B').
+  Proof.
+    intros * [] [] []; unshelve econstructor.
+    5: eapply SigCongTm; tea; try irrValid.
+    4: eapply irrelevanceTmLift ; try irrValid; now eapply univEqValid.
+    1,2: unshelve eapply SigValidU; try irrValid.
+    1,2: now eapply univValid.
+    1: eapply UValid.
+    eapply irrelevanceTmLift ; try irrValid; now eapply univEqValid.
+    Unshelve. all: solve [ eapply UValid | now eapply univValid | irrValid].
+  Qed.
+
+  Lemma FundTmEqPairCong : forall wl (Γ : context) (A A' A'' B B' B'' a a' b b' : term),
+    FundTy wl Γ A ->
+    FundTyEq wl Γ A A' ->
+    FundTyEq wl Γ A A'' ->
+    FundTyEq wl (Γ,, A) B B' ->
+    FundTyEq wl (Γ,, A) B B'' ->
+    FundTmEq wl Γ A a a' ->
+    FundTmEq wl Γ B[a..] b b' -> FundTmEq wl Γ (tSig A B) (tPair A' B' a b) (tPair A'' B'' a' b').
+  Proof.
+    intros * [VΓ VA] [] [] [] [] [] [].
+    assert (VΣ : [Γ ||-v< one > tSig A B | VΓ]< wl >).
+    { unshelve eapply SigValid; irrValid. }
+    assert (VA' : [Γ ||-v< one > A' | VΓ]< wl >) by irrValid.
+    assert (VA'' : [Γ ||-v< one > A'' | VΓ]< wl >) by irrValid.
+    assert ([Γ ||-v< one > a : A' | VΓ | VA']< wl >).
+    { eapply conv; [|irrValid]; irrValid. Unshelve. tea. }
+    assert ([Γ ||-v< one > a : A'' | VΓ | VA'']< wl >).
+    { eapply conv; [irrValid|]; irrValid. Unshelve. tea. }
+    assert ([Γ ||-v< one > a' : A'' | VΓ | VA'']< wl >).
+    { eapply conv; [irrValid|]; irrValid. Unshelve. tea. }
+    assert (VΓA' : VAdequate (ta := ta) wl (Γ,, A') VR) by now eapply validSnoc'.
+    assert (VΓA'' : VAdequate (ta := ta) wl (Γ,, A'') VR) by now eapply validSnoc'.
+    assert (VA'B : [Γ,, A' ||-v< one > B | VΓA']< wl >).
+    { eapply irrelevanceTy, irrelevanceLift; irrValid.
+      Unshelve. all: irrValid. }
+    assert (VA''B : [Γ,, A'' ||-v< one > B | VΓA'']< wl >).
+    { eapply irrelevanceTy, irrelevanceLift; irrValid.
+      Unshelve. all: irrValid. }
+    assert (VA'B' : [Γ,, A' ||-v< one > B' | VΓA']< wl >).
+    { eapply irrelevanceTy, irrelevanceLift; try irrValid.
+      Unshelve. all: irrValid. }
+    assert (VA''B' : [Γ,, A'' ||-v< one > B' | VΓA'']< wl >).
+    { eapply irrelevanceTy, irrelevanceLift; try irrValid.
+      Unshelve. all: irrValid. }
+    assert (VA''B'' : [Γ,, A'' ||-v< one > B'' | VΓA'']< wl >).
+    { eapply irrelevanceTy, irrelevanceLift; try irrValid.
+      Unshelve. all: irrValid. }
+    assert (VBa : [Γ ||-v< one > B[a..] | VΓ]< wl >).
+    { irrValid. }
+    assert (VB'a : [Γ ||-v< one > B'[a..] | VΓ]< wl >).
+    { eapply substS; irrValid. Unshelve. all: irrValid. }
+    assert (VB''a : [Γ ||-v< one > B''[a..] | VΓ]< wl >).
+    { eapply substS; irrValid. Unshelve. all: irrValid. }
+    assert (VB''a' : [Γ ||-v< one > B''[a'..] | VΓ]< wl >).
+    { eapply substS; irrValid. Unshelve. all: irrValid. }
+    assert [Γ ||-v< one > B[a..] ≅ B'[a..] | VΓ | VBa]< wl >.
+    { eapply irrelevanceTyEq, substSEq; try irrValid.
+      apply reflValidTm. irrValid. Unshelve. all: irrValid. }
+    assert [Γ ||-v< one > B[a..] ≅ B''[a'..] | VΓ | VBa]< wl >.
+    { eapply irrelevanceTyEq, substSEq; [..|irrValid|irrValid].
+      all: irrValid. Unshelve. all: irrValid. }
+    assert (VΣA'B' : [Γ ||-v< one > tSig A' B' | VΓ]< wl >).
+    { unshelve eapply SigValid; try irrValid. }
+    assert (VΣA''B'' : [Γ ||-v< one > tSig A'' B'' | VΓ]< wl >).
+    { unshelve eapply SigValid; try irrValid. }
+    assert ([Γ ||-v< one > tSig A B ≅ tSig A' B' | VΓ | VΣ]< wl >).
+    { unshelve eapply irrelevanceTyEq, SigCong; try irrValid. }
+    assert ([Γ ||-v< one > tSig A B ≅ tSig A'' B'' | VΓ | VΣ]< wl >).
+    { unshelve eapply irrelevanceTyEq, SigCong; try irrValid. }
+    assert [Γ ||-v< one > tPair A' B' a b : tSig A B | _ | VΣ ]< wl >.
+    { eapply conv; [|unshelve eapply pairValid]; try irrValid.
+      - unshelve eapply symValidTyEq; irrValid.
+      - eapply conv; irrValid. Unshelve. all: irrValid. }
+    assert [Γ ||-v< one > tPair A'' B'' a' b' : tSig A B | _ | VΣ ]< wl >.
+    { eapply conv; [|unshelve eapply pairValid]; try irrValid.
+      - unshelve eapply symValidTyEq; irrValid.
+      - eapply conv; irrValid.
+        Unshelve. all: irrValid. }
+    assert [Γ ||-v< one > b : B'[a..] | VΓ | VB'a]< wl >.
+    { eapply conv; irrValid. Unshelve. all: irrValid. }
+    assert [Γ ||-v< one > b' : B''[a'..] | VΓ | VB''a']< wl >.
+    { eapply conv; irrValid. Unshelve. all: irrValid. }
+    assert ([Γ ||-v< one > tFst (tPair A' B' a b) ≅ a : A | VΓ | VA]< wl >).
+    { eapply (convEq (A := A')); [eapply symValidTyEq; irrValid|].
+      eapply pairFstValid. Unshelve. all: try irrValid. }
+    assert ([Γ ||-v< one > tFst (tPair A'' B'' a' b') ≅ a' : A | VΓ | VA]< wl >).
+    { eapply (convEq (A := A'')); [eapply symValidTyEq; irrValid|].
+      eapply pairFstValid. Unshelve. all: irrValid. }
+    assert ([Γ ||-v< one > tFst (tPair A' B' a b) ≅ tFst (tPair A'' B'' a' b') : A | VΓ | VA]< wl >).
+    { eapply transValidTmEq; [irrValid|].
+      eapply transValidTmEq; [irrValid|].
+      eapply symValidTmEq; irrValid. }
+    assert ([Γ ||-v< one > tFst (tPair A' B' a b) : A | VΓ | VA]< wl >).
+    { eapply fstValid. Unshelve. all: try irrValid. }
+    assert ([Γ ||-v< one > tFst (tPair A'' B'' a' b') : A | VΓ | VA]< wl >).
+    { eapply fstValid. Unshelve. all: try irrValid. }
+    assert (VBfst : [Γ ||-v< one > B[(tFst (tPair A' B' a b))..] | VΓ]< wl >).
+    { eapply (substS (F := A)). Unshelve. all: try  irrValid. }
+    assert (VB'fst : [Γ ||-v< one > B'[(tFst (tPair A' B' a b))..] | VΓ]< wl >).
+    { eapply (substS (F := A)). Unshelve. all: try  irrValid. }
+    assert (VB''fst' : [Γ ||-v< one > B''[(tFst (tPair A'' B'' a' b'))..] | VΓ]< wl >).
+    { eapply (substS (F := A)). Unshelve. all: try irrValid. }
+    assert ([Γ ||-v< one > B[(tFst (tPair A' B' a b))..] ≅ B[a..] | VΓ | VBfst]< wl >).
+    { eapply irrelevanceTyEq, substSEq; [..|irrValid|irrValid].
+      Unshelve. all: try irrValid. eapply reflValidTy. }
+    assert ([Γ ||-v< one > B'[(tFst (tPair A' B' a b))..] ≅ B[a..] | VΓ | VB'fst]< wl >).
+    { eapply irrelevanceTyEq, substSEq; [..|irrValid|irrValid].
+      Unshelve. all: try irrValid.
+      eapply symValidTyEq; irrValid. Unshelve. all: try irrValid. }
+    assert ([Γ ||-v< one > B''[(tFst (tPair A'' B'' a' b'))..] ≅ B[a'..] | VΓ | VB''fst']< wl >).
+    { eapply irrelevanceTyEq, substSEq; [..|irrValid|].
+      Unshelve. all: try irrValid.
+      eapply symValidTyEq; irrValid. Unshelve. all: try irrValid. }
+    assert ([Γ ||-v< one > B''[(tFst (tPair A'' B'' a' b'))..] ≅ B[a..] | VΓ | VB''fst']< wl >).
+    { eapply irrelevanceTyEq, substSEq; [..|irrValid|].
+      Unshelve. all: try irrValid.
+      eapply symValidTyEq; irrValid. Unshelve. all: try irrValid.
+      eapply transValidTmEq; [irrValid|].
+      eapply symValidTmEq; irrValid.
+    }
+    assert ([Γ ||-v< one > tSnd (tPair A' B' a b) ≅ b : B[(tFst (tPair A' B' a b))..] | VΓ | VBfst]< wl >).
+    { eapply (convEq (A := B'[(tFst (tPair A' B' a b))..])).
+      shelve. eapply pairSndValid.
+      Unshelve. all: try irrValid.
+      eapply irrelevanceTyEq, substSEq; [..|irrValid|apply reflValidTm; irrValid].
+      all: try irrValid.
+      - unshelve apply reflValidTy.
+      - unshelve eapply symValidTyEq; irrValid. }
+    assert ([Γ ||-v< one > tSnd (tPair A'' B'' a' b') ≅ b' : B[a..] | VΓ | VBa]< wl >).
+    { eapply (convEq (A := B''[(tFst (tPair A'' B'' a' b'))..])).
+      shelve. eapply pairSndValid.
+      Unshelve. all: try irrValid. }
+    unshelve econstructor. 1-4: irrValid.
+    eapply irrelevanceTmEq, sigEtaValid; try irrValid.
+    eapply transValidTmEq; [irrValid|].
+    eapply transValidTmEq.
+    - eapply convEq; [|irrValid].
+      eapply symValidTyEq; try irrValid.
+    - eapply symValidTmEq; try irrValid.
+      eapply convEq; [|irrValid].
+      eapply symValidTyEq; try irrValid.
+  Unshelve. all: try irrValid.
+  Qed.
+
+  Lemma FundTmEqSigEta : forall wl (Γ : context) (A B p : term),
+    FundTm wl Γ (tSig A B) p -> FundTmEq wl Γ (tSig A B) (tPair A B (tFst p) (tSnd p)) p.
+  Proof.
+  intros * [VΓ VΣ Vp].
+  assert (VA := domSigValid _ VΣ).
+  assert (VB := codSigValid _ VΣ).
+  assert (Vfst : [Γ ||-v< one > tFst p : A | _ | VA]< wl >).
+  { unshelve eapply irrelevanceTm, fstValid; try irrValid. }
+  assert (VBfst : [Γ ||-v< one > B[(tFst p)..] | VΓ]< wl >).
+  { unshelve eapply substS; try irrValid. }
+  assert (Vsnd : [Γ ||-v< one > tSnd p : B[(tFst p)..] | _ | VBfst]< wl >).
+  { unshelve eapply irrelevanceTm, sndValid.
+    5: irrValid. all: irrValid. }
+  assert (Vηp : [Γ ||-v< one > tPair A B (tFst p) (tSnd p) : tSig A B | VΓ | VΣ]< wl >).
+  { unshelve eapply irrelevanceTm, pairValid; try irrValid. }
+  unshelve econstructor; try irrValid.
+  eapply irrelevanceTmEq, sigEtaValid; try irrValid.
+  - eapply transValidTmEq; [eapply pairFstValid|eapply reflValidTm].
+    Unshelve. all: try irrValid.
+  - eapply transValidTmEq; [unshelve eapply irrelevanceTmEq, pairSndValid|unshelve eapply reflValidTm]; try irrValid.
+    unshelve eapply conv; try irrValid.
+    eapply irrelevanceTyEq, substSEq; try irrValid.
+    1,2: unshelve apply reflValidTy.
+    { unshelve eapply fstValid; try irrValid. }
+    { unshelve eapply symValidTmEq, pairFstValid; try irrValid. }
+    Unshelve. all: try irrValid.
+  Qed.
+
+  Lemma FundTmEqFstCong : forall wl (Γ : context) (A B p p' : term),
+    FundTmEq wl Γ (tSig A B) p p' -> FundTmEq wl Γ A (tFst p) (tFst p').
+  Proof.
+    intros * []; unshelve econstructor.
+    5: eapply fstCongValid; irrValid.
+    2: now eapply domSigValid.
+    1,2: eapply fstValid; irrValid.
+    Unshelve. all: now eapply codSigValid.
+  Qed.
+
+  Lemma FundTmEqFstBeta : forall wl (Γ : context) (A B a b : term),
+    FundTy wl Γ A ->
+    FundTy wl (Γ,, A) B ->
+    FundTm wl Γ A a ->
+    FundTm wl Γ B[a..] b -> FundTmEq wl Γ A (tFst (tPair A B a b)) a.
+  Proof.
+    intros * [] [] [] [].
+    unshelve econstructor.
+    3,5: eapply pairFstValid; irrValid.
+    2,3: irrValid. 
+    tea.
+    Unshelve. all: irrValid.
+  Qed.
+
+  Lemma FundTmEqSndCong : forall wl (Γ : context) (A B p p' : term),
+    FundTmEq wl Γ (tSig A B) p p' -> FundTmEq wl Γ B[(tFst p)..] (tSnd p) (tSnd p').
+  Proof.
+    intros * []; unshelve econstructor.
+    5: eapply sndCongValid; irrValid.
+    1: tea.
+    1: eapply sndValid.
+    eapply conv; [| eapply sndValid].
+    eapply substSEq.
+    5: eapply fstCongValid.
+    4: eapply fstValid.
+    4-6: irrValid.
+    + eapply reflValidTy.
+    + eapply codSigValid.
+    + eapply reflValidTy.
+    + eapply symValidTmEq; irrValid.
+    Unshelve. all: try solve [now eapply domSigValid| now eapply codSigValid| irrValid].
+  Qed.
+
+  Lemma FundTmEqSndBeta : forall wl (Γ : context) (A B a b : term),
+    FundTy wl Γ A ->
+    FundTy wl (Γ,, A) B ->
+    FundTm wl Γ A a ->
+    FundTm wl Γ B[a..] b ->
+    FundTmEq wl Γ B[(tFst (tPair A B a b))..] (tSnd (tPair A B a b)) b.
+  Proof.
+    intros * [] [] [] []; unshelve econstructor.
+    3,5: unshelve eapply pairSndValid; irrValid.
+    + tea.
+    + eapply conv; tea.
+      eapply irrelevanceTyEq.
+      eapply substSEq.
+      1,3: eapply reflValidTy.
+      1: irrValid.
+      2: eapply symValidTmEq.
+      1,2: eapply pairFstValid; irrValid.
+    Unshelve. all: irrValid.
+  Qed.
+
+  Lemma FundTyId : forall wl (Γ : context) (A x y : term),
+    FundTy wl Γ A -> FundTm wl Γ A x -> FundTm wl Γ A y -> FundTy wl Γ (tId A x y).
+  Proof.
+    intros * [] [] [].
+    unshelve econstructor; tea.
+    unshelve eapply IdValid; irrValid.
+  Qed.
+
+
+  Lemma FundTmId : forall wl (Γ : context) (A x y : term),
+    FundTm wl Γ U A -> FundTm wl Γ A x -> FundTm wl Γ A y -> FundTm wl Γ U (tId A x y).
+  Proof.
+      intros * [] [] [].
+      unshelve econstructor; tea.
+      1: eapply UValid.
+      unshelve eapply IdTmValid; cycle 1; try irrValid; tea.
+  Qed.
+
+  Lemma FundTmRefl : forall wl (Γ : context) (A x : term),
+    FundTy wl Γ A -> FundTm wl Γ A x -> FundTm wl Γ (tId A x x) (tRefl A x).
+  Proof.
+    intros * [] []; unshelve econstructor.
+    3: now eapply reflValid.
+    now eapply IdValid.
+  Qed.
+
+  Lemma FundTmIdElim : forall wl (Γ : context) (A x P hr y e : term),
+    FundTy wl Γ A ->
+    FundTm wl Γ A x ->
+    FundTy wl ((Γ,, A),, tId A⟨@wk1 Γ A⟩ x⟨@wk1 Γ A⟩ (tRel 0)) P ->
+    FundTm wl Γ P[tRefl A x .: x..] hr ->
+    FundTm wl Γ A y -> FundTm wl Γ (tId A x y) e -> FundTm wl Γ P[e .: y..] (tIdElim A x P hr y e).
+  Proof.
+    intros * [] [] [] [] [] []; unshelve econstructor.
+    3: unshelve eapply IdElimValid; try irrValid.
+    tea.
+  Qed.
+
+  Lemma FundTyEqId : forall wl (Γ : context) (A A' x x' y y' : term),
+    FundTyEq wl Γ A A' ->
+    FundTmEq wl Γ A x x' -> FundTmEq wl Γ A y y' -> FundTyEq wl Γ (tId A x y) (tId A' x' y').
+  Proof.
+    intros * [] [] [].
+    unshelve econstructor; tea.
+    3: eapply IdCongValid; irrValid.
+    1,2: eapply IdValid; try irrValid.
+    1,2: eapply conv; irrValid.
+    Unshelve. all: irrValid.
+  Qed.
+
+  Lemma FundTmEqIdCong : forall wl (Γ : context) (A A' x x' y y' : term),
+    FundTmEq wl Γ U A A' ->
+    FundTmEq wl Γ A x x' -> FundTmEq wl Γ A y y' -> FundTmEq wl Γ U (tId A x y) (tId A' x' y').
+  Proof.
+    intros * [] [] []; unshelve econstructor.
+    5: eapply IdTmCongValid; try irrValid; tea.
+    2,3: eapply IdTmValid; try irrValid; tea.
+    1: tea.
+    1,2: eapply conv; try irrValid; eapply univEqValid; irrValid.
+    Unshelve. all: first [eapply UValid| irrValid | tea].
+  Qed.
+
+  Lemma FundTmEqReflCong : forall wl (Γ : context) (A A' x x' : term),
+    FundTyEq wl Γ A A' -> FundTmEq wl Γ A x x' -> FundTmEq wl Γ (tId A x x) (tRefl A x) (tRefl A' x').
+  Proof.
+    intros * [] []; unshelve econstructor.
+    5: eapply reflCongValid; tea; irrValid.
+    3: eapply conv.
+    2,4: eapply reflValid; try irrValid.
+    2: eapply conv; irrValid.
+    2: eapply symValidTyEq; eapply IdCongValid; tea; try irrValid.
+    eapply IdValid; irrValid.
+    Unshelve. all: try eapply IdValid; try irrValid; eapply conv; irrValid.
+    Unshelve. all: irrValid.
+  Qed.
+
+  Lemma FundTmEqIdElimCong : forall wl (Γ : context) (A A' x x' P P' hr hr' y y' e e' : term),
+    FundTy wl Γ A ->
+    FundTm wl Γ A x ->
+    FundTyEq wl Γ A A' ->
+    FundTmEq wl Γ A x x' ->
+    FundTyEq wl ((Γ,, A),, tId A⟨@wk1 Γ A⟩ x⟨@wk1 Γ A⟩ (tRel 0)) P P' ->
+    FundTmEq wl Γ P[tRefl A x .: x..] hr hr' ->
+    FundTmEq wl Γ A y y' ->
+    FundTmEq wl Γ (tId A x y) e e' -> FundTmEq wl Γ P[e .: y..] (tIdElim A x P hr y e) (tIdElim A' x' P' hr' y' e').
+  Proof.
+    intros * [] [] [] [] [] [] [] [].
+    assert [_ ||-v<one> x' : _ | _ | VB]< wl > by (eapply conv; irrValid).
+    assert [_ ||-v<one> y' : _ | _ | VB]< wl > by (eapply conv; irrValid).
+    assert (VId' : [_ ||-v<one> tId A' x' y' | VΓ]< wl >) by (eapply IdValid; irrValid).
+    assert [_ ||-v<one> _ ≅ tId A' x' y' | _ | VA6]< wl > by (eapply IdCongValid; irrValid).
+    assert [_ ||-v<one> e' : _ | _ | VId']< wl > by (eapply conv; irrValid).
+    unshelve econstructor.
+    5: eapply IdElimCongValid; tea; irrValid.
+    1: eapply IdElimValid; irrValid.
+    eapply convsym.
+    2: eapply IdElimValid; eapply conv; [|irrValid].
+    1:{
+      eapply substEqIdElimMotive. 7: tea. 2,3,5-12: tea; try irrValid. 1,2: irrValid.
+    } 
+   eapply substEqIdElimMotive. 7: tea. 2,3,5-9: tea; try irrValid.
+    1,2: irrValid.
+    2: eapply convsym. 
+    1,3: eapply reflValid; first [irrValid| eapply conv; irrValid].
+    1:eapply IdCongValid; irrValid.
+    eapply reflCongValid; irrValid.
+    Unshelve. all: tea; try irrValid.
+    3,4: eapply IdValid; irrValid.
+    1: eapply validSnoc'; now eapply idElimMotiveCtxIdValid.
+    eapply convCtx2'; tea.
+    1: eapply convCtx1; tea; [eapply symValidTyEq; irrValid| ].
+    1,3: now eapply idElimMotiveCtxIdValid.
+    eapply idElimMotiveCtxIdCongValid; tea; irrValid.
+    Unshelve.
+    3: eapply idElimMotiveCtxIdValid. all: irrValid.
+  Qed.
+
+  Lemma FundTmEqIdElimRefl : forall wl (Γ : context) (A x P hr y A' z : term),
+    FundTy wl Γ A ->
+    FundTm wl Γ A x ->
+    FundTy wl ((Γ,, A),, tId A⟨@wk1 Γ A⟩ x⟨@wk1 Γ A ⟩ (tRel 0)) P ->
+    FundTm wl Γ P[tRefl A x .: x..] hr ->
+    FundTm wl Γ A y ->
+    FundTy wl Γ A' ->
+    FundTm wl Γ A z ->
+    FundTyEq wl Γ A A' ->
+    FundTmEq wl Γ A x y ->
+    FundTmEq wl Γ A x z -> FundTmEq wl Γ P[tRefl A' z .: y..] (tIdElim A x P hr y (tRefl A' z)) hr.
+  Proof.
+    intros * [] [] [] [] [] [] [] [] [] [].
+    assert (VId : [_ ||-v<one> tId A x y | VΓ]< wl >) by (unshelve eapply IdValid; irrValid).
+    assert [Γ ||-v< one > tRefl A' z : tId A x y | _ | VId]< wl >.
+    1:{
+      eapply convsym ; [| eapply reflValid; try irrValid].
+      2: eapply conv; irrValid.
+      eapply IdCongValid; try irrValid.
+      eapply transValidTmEq; [eapply symValidTmEq|]; irrValid.
+      Unshelve.
+       1: unshelve eapply IdValid; try eapply conv. 
+       all: try irrValid.
+       Unshelve. all: irrValid.
+    } 
+    unshelve econstructor.
+    5: eapply IdElimReflValid; tea; try irrValid.
+    3: eapply conv; irrValid.
+    2:{
+      eapply conv; [|irrValid].
+      eapply substExtIdElimMotive; cycle 1; tea.
+      + eapply reflValid; irrValid.
+      + irrValid.
+      + eapply reflCongValid; tea; irrValid.
+    }
+    eapply IdElimValid; irrValid.
+    Unshelve. all: tea; try irrValid.
+      unshelve eapply IdValid; irrValid.
+  Qed.
+
+Lemma FundTySplit : forall (wl : wfLCon)
+  (Γ : context)
+  (A : term)
+  (n : nat)
+  (ne : not_in_LCon wl n),
+  FundTy (wl,,l (ne, true)) Γ A ->
+  FundTy (wl,,l (ne, false)) Γ A ->
+  FundTy wl Γ A.
+Proof.
+  intros ????? [] [].
+  unshelve econstructor.
+  2: now unshelve eapply validTySplit.
+  now eapply WfCSplit.
+Qed.
+
+Lemma FundTmSplit : forall (wl : wfLCon)
+  (Γ : context)
+  (A t : term)
+  (n : nat)
+  (ne : not_in_LCon wl n),
+  FundTm (wl,,l (ne, true)) Γ A t ->
+  FundTm (wl,,l (ne, false)) Γ A t ->
+  FundTm wl Γ A t.
+Proof.
+  intros ?????? [] [].
+  unshelve econstructor.
+  - now eapply WfCSplit.
+  - now eapply validTySplit.
+  - unshelve eapply validTmSplit' ; eassumption.
+Qed.
+
+Lemma FundTyEqSplit : forall (wl : wfLCon)
+  (Γ : context)
+  (A B : term)
+  (n : nat)
+  (ne : not_in_LCon wl n),
+  FundTyEq (wl,,l (ne, true)) Γ A B ->
+  FundTyEq (wl,,l (ne, false)) Γ A B ->
+  FundTyEq wl Γ A B.
+Proof.
+  intros ?????? [] [].
+  unshelve econstructor.
+  - now eapply WfCSplit.
+  - now eapply validTySplit.
+  - now eapply validTySplit.
+  - now unshelve eapply validEqTySplit'.
+Qed.
+
+Lemma FundTmEqSplit : forall (wl : wfLCon)
+  (Γ : context)
+  (t u A : term)
+  (n : nat)
+  (ne : not_in_LCon wl n),
+  FundTmEq (wl,,l (ne, true)) Γ A t u ->
+  FundTmEq (wl,,l (ne, false)) Γ A t u ->
+  FundTmEq wl Γ A t u.
+Proof.
+  intros ??????? [] [].
+  unshelve econstructor.
+  - now eapply WfCSplit.
+  - now eapply validTySplit.
+  - now eapply validTmSplit'.
+  - now eapply validTmSplit'.
+  - now eapply validEqTmSplit'.
+Qed.  
+  
+  Lemma Fundamental (wl : wfLCon) :
+    (forall (Γ : context), [ |-[ de ] Γ ]< wl > -> FundCon wl (ta := ta) Γ)
+    × (forall (Γ : context) (A : term), [Γ |-[ de ] A]< wl > -> FundTy wl (ta := ta) Γ A)
+    × (forall (Γ : context) (A t : term), [Γ |-[ de ] t : A]< wl > -> FundTm wl (ta := ta) Γ A t)
+    × (forall (Γ : context) (A B : term), [Γ |-[ de ] A ≅ B]< wl > -> FundTyEq wl (ta := ta) Γ A B)
+    × (forall (Γ : context) (A t u : term), [Γ |-[ de ] t ≅ u : A]< wl > -> FundTmEq wl (ta := ta) Γ A t u).
+  Proof.
+  apply WfDeclInduction ; intros.
+  + intros; now apply FundConNil.
+  + intros; now apply FundConCons.
+  + intros; now apply FundTyU.
+  + intros; now apply FundTyPi.
+  + intros; now apply FundTyNat.
+  + intros; now apply FundTyEmpty.
+  + intros; now apply FundTyBool.
+  + intros; now apply FundTySig.
+  + intros; now apply FundTyId.
+  + intros; now apply FundTyUniv.
+  + intros; now eapply FundTySplit. 
+  + intros; now apply FundTmVar.
+  + intros; now apply FundTmProd.
+  + intros; now apply FundTmLambda.
+  + intros; now eapply FundTmApp.
+  + intros; now apply FundTmNat.
+  + intros; now apply FundTmBool.
+  + intros; now apply FundTmZero.
+  + intros; now apply FundTmSucc.
+  + intros; now apply FundTmNatElim.
+  + intros; now apply FundTmEmpty.
+  + intros; now apply FundTmEmptyElim.
+  + intros; now apply FundTmTrue.
+  + intros; now apply FundTmFalse.
+  + intros ; now apply FundTmAlpha. 
+  + intros; now apply FundTmBoolElim.
+  + intros; now apply FundTmSig.
+  + intros; now apply FundTmPair.
+  + intros; now eapply FundTmFst.
+  + intros; now eapply FundTmSnd.
+  + intros; now eapply FundTmId.
+  + intros; now eapply FundTmRefl.
+  + intros; now eapply FundTmIdElim.
+  + intros; now eapply FundTmConv.
+  + intros; now eapply FundTmSplit.
+  + intros; now apply FundTyEqPiCong.
+  + intros; now apply FundTyEqSigCong.
+  + intros; now eapply FundTyEqId.
+  + intros; now apply FundTyEqRefl.
+  + intros; now apply FundTyEqUniv.
+  + intros; now apply FundTyEqSym.
+  + intros; now eapply FundTyEqTrans.
+  + intros; now eapply FundTyEqSplit. 
+  + intros; now apply FundTmEqBRed.
+  + intros; now apply FundTmEqPiCong.
+  + intros; now eapply FundTmEqAppCong.
+  + intros; now apply FundTmEqLambdaCong.
+  + intros; now apply FundTmEqFunEta.
+  + intros; now apply FundTmEqSuccCong.
+  + intros; now apply FundTmEqNatElimCong.
+  + intros; now apply FundTmEqNatElimZero.
+  + intros; now apply FundTmEqNatElimSucc.
+  + intros; now apply FundTmEqEmptyElimCong.
+  + intros; now apply FundTmEqBoolElimCong.
+  + intros; now apply FundTmEqBoolElimTrue. 
+  + intros; now apply FundTmEqBoolElimFalse. 
+  + intros; now apply FundTmEqAlphaCong. 
+  + intros; now apply FundTmEqAlpha.
+  + intros; now apply FundTmEqSigCong.
+  + intros; now apply FundTmEqPairCong.
+  + intros; now apply FundTmEqSigEta.
+  + intros; now eapply FundTmEqFstCong.
+  + intros; now apply FundTmEqFstBeta.
+  + intros; now eapply FundTmEqSndCong.
+  + intros; now apply FundTmEqSndBeta.
+  + intros; now apply FundTmEqIdCong.
+  + intros; now apply FundTmEqReflCong.
+  + intros; now apply FundTmEqIdElimCong.
+  + intros; now apply FundTmEqIdElimRefl.
+  + intros; now apply FundTmEqRefl.
+  + intros; now eapply FundTmEqConv.
+  + intros; now apply FundTmEqSym.
+  + intros; now eapply FundTmEqTrans.
+  + intros; now eapply FundTmEqSplit. 
   Qed.
 
 (** ** Well-typed substitutions are also valid *)
 
-  Corollary Fundamental_subst Γ Δ σ (wfΓ : [|-[ta] Γ ]) :
-    [|-[de] Δ] ->
-    [Γ |-[de]s σ : Δ] ->
-    FundSubst Γ Δ wfΓ σ.
+  Corollary Fundamental_subst wl wl' Γ Δ σ f (wfΓ : [|-[ta] Γ ]< wl' >) :
+    [|-[de] Δ]< wl > ->
+    [Γ |-[de]s σ : Δ]< wl' > ->
+    FundSubst wl wl' Γ Δ σ f wfΓ .
   Proof.
     intros HΔ.
     induction 1 as [|σ Δ A Hσ IH Hσ0].
-    - exists validEmpty.
+    - exists validEmpty'.
       now constructor.
     - inversion HΔ as [|?? HΔ' HA] ; subst ; clear HΔ ; refold.
       destruct IH ; tea.
@@ -637,51 +1486,50 @@ Lemma Fundamental : (forall Γ : context, [ |-[ de ] Γ ] -> FundCon (ta := ta) 
       eapply reducibleTm in Hσ0.
       eapply Fundamental in HA as [].
       unshelve econstructor.
-      1: now eapply validSnoc.
+      1: now eapply validSnoc'.
       unshelve econstructor.
       + now eapply irrelevanceSubst.
-      + cbn; irrelevance0.
+      + cbn; Wirrelevance0.
         2: eassumption.
         reflexivity.
   Qed.
 
-  Corollary Fundamental_subst_conv Γ Δ σ σ' (wfΓ : [|-[ta] Γ ]) :
-    [|-[de] Δ] ->
-    [Γ |-[de]s σ ≅ σ' : Δ] ->
-    FundSubstConv Γ Δ wfΓ σ σ'.
+  Corollary Fundamental_subst_conv wl wl' Γ Δ σ σ' (f : wl' ≤ε wl) (wfΓ : [|-[ta] Γ ]< wl' >) :
+    [|-[de] Δ]< wl > ->
+    [Γ |-[de]s σ ≅ σ' : Δ]< wl' > ->
+    FundSubstConv Γ Δ σ σ' f wfΓ .
   Proof.
     intros HΔ.
     induction 1 as [|σ τ Δ A Hσ IH Hσ0].
     - unshelve econstructor.
-      1: eapply validEmpty.
+      1: eapply validEmpty'.
       all: now econstructor.
     - inversion HΔ as [|?? HΔ' HA] ; subst ; clear HΔ ; refold.
       destruct IH ; tea.
       apply Fundamental in Hσ0 as [?? Hσ0 Hτ0 Ηστ] ; cbn in *.
       eapply Fundamental in HA as [? HA].
       unshelve econstructor.
-      + now eapply validSnoc.
+      + now eapply validSnoc'.
       + unshelve econstructor.
         1: now irrValid.
-        cbn.
-        irrelevanceRefl.
+        cbn ; Wirrelevance0 ; [reflexivity | ].
         now eapply reducibleTm.
       + unshelve econstructor.
         1: now eapply irrelevanceSubst.
         cbn.
-        unshelve irrelevanceRefl.
+        unshelve (Wirrelevance0 ; [reflexivity | ]).
         2: now unshelve eapply HA ; tea ; irrValid.
         cbn.
-        unshelve eapply LRTmRedConv.
+        unshelve eapply WLRTmRedConv.
         3: now eapply reducibleTy.
-        * irrelevanceRefl.
+        * cbn ; Wirrelevance0 ; [reflexivity | ].
           unshelve eapply HA ; tea.
           all: now irrValid.
-        * irrelevanceRefl.
+        * cbn ; Wirrelevance0 ; [reflexivity | ].
           now eapply reducibleTm.
       + unshelve econstructor ; cbn in *.
         * now irrValid.
-        * irrelevanceRefl.
+        * cbn ; Wirrelevance0 ; [reflexivity | ].
           now eapply reducibleTmEq.
   Qed.
 
