theories/Substitution/Introductions/Id.v
@@ -1,7 +1,7 @@
 From LogRel.AutoSubst Require Import core unscoped Ast Extra.
-From LogRel Require Import Utils BasicAst Notations Context NormalForms Weakening GenericTyping LogicalRelation Validity.
-From LogRel.LogicalRelation Require Import Induction Irrelevance Escape Reflexivity Weakening Neutral Transitivity Reduction Application Universe Id.
-From LogRel.Substitution Require Import Irrelevance Properties Conversion SingleSubst Reflexivity Reduction.
+From LogRel Require Import Utils BasicAst Notations LContexts Context NormalForms Weakening GenericTyping Monad LogicalRelation Validity.
+From LogRel.LogicalRelation Require Import Induction Irrelevance Escape Reflexivity Monotonicity Split Weakening Neutral Transitivity Reduction Application Universe Id.
+From LogRel.Substitution Require Import Irrelevance Properties Monotonicity Conversion SingleSubst Reflexivity Reduction.
 From LogRel.Substitution.Introductions Require Import Universe Var.
 
 Set Universe Polymorphism.
@@ -9,111 +9,109 @@ Set Universe Polymorphism.
 Section Id.
 Context `{GenericTypingProperties}.
 
-  Lemma IdValid {Γ l A x y} 
-    (VΓ : [||-v Γ]) 
-    (VA : [_ ||-v<l> A | VΓ]) 
-    (Vx : [_ ||-v<l> x : _ | _ | VA])
-    (Vy : [_ ||-v<l> y : _ | _ | VA]) :
-    [_ ||-v<l> tId A x y | VΓ].
+  Lemma IdValid {wl Γ l A x y} 
+    (VΓ : [||-v Γ]< wl >) 
+    (VA : [_ ||-v<l> A | VΓ]< wl >) 
+    (Vx : [_ ||-v<l> x : _ | _ | VA]< wl >)
+    (Vy : [_ ||-v<l> y : _ | _ | VA]< wl >) :
+    [_ ||-v<l> tId A x y | VΓ]< wl >.
   Proof.
     unshelve econstructor; intros.
-    - instValid vσ; cbn; now eapply IdRed.
-    - instAllValid vσ vσ' vσσ'; eapply IdCongRed; refold; tea.
-      eapply wft_Id; now escape.
+    - instValid vσ; cbn ; now eapply WIdRed.
+    - instAllValid vσ vσ' vσσ'; eapply WIdCongRed; refold; tea.
+      eapply wft_Id; now Wescape.
   Qed.
 
-  Lemma IdCongValid {Γ l A A' x x' y y'}
-    (VΓ : [||-v Γ]) 
-    (VA : [_ ||-v<l> A | VΓ]) 
-    (VA' : [_ ||-v<l> A' | VΓ]) 
-    (VAA' : [_ ||-v<l> A ≅ A' | VΓ | VA]) 
-    (Vx : [_ ||-v<l> x : _ | _ | VA])
-    (Vx' : [_ ||-v<l> x' : _ | _ | VA])
-    (Vxx' : [_ ||-v<l> x ≅ x' : _ | _ | VA])
-    (Vy : [_ ||-v<l> y : _ | _ | VA]) 
-    (Vy' : [_ ||-v<l> y' : _ | _ | VA]) 
-    (Vyy' : [_ ||-v<l> y ≅ y' : _ | _ | VA]) 
-    (VId : [_ ||-v<l> tId A x y | VΓ]) :
-    [_ ||-v<l> tId A x y ≅ tId A' x' y' | VΓ | VId].
+  Lemma IdCongValid {wl Γ l A A' x x' y y'}
+    (VΓ : [||-v Γ]< wl >) 
+    (VA : [_ ||-v<l> A | VΓ]< wl >) 
+    (VA' : [_ ||-v<l> A' | VΓ]< wl >) 
+    (VAA' : [_ ||-v<l> A ≅ A' | VΓ | VA]< wl >) 
+    (Vx : [_ ||-v<l> x : _ | _ | VA]< wl >)
+    (Vx' : [_ ||-v<l> x' : _ | _ | VA]< wl >)
+    (Vxx' : [_ ||-v<l> x ≅ x' : _ | _ | VA]< wl >)
+    (Vy : [_ ||-v<l> y : _ | _ | VA]< wl >) 
+    (Vy' : [_ ||-v<l> y' : _ | _ | VA]< wl >) 
+    (Vyy' : [_ ||-v<l> y ≅ y' : _ | _ | VA]< wl >) 
+    (VId : [_ ||-v<l> tId A x y | VΓ]< wl >) :
+    [_ ||-v<l> tId A x y ≅ tId A' x' y' | VΓ | VId]< wl >.
   Proof.
     constructor; intros.
-    instValid Vσ; eapply IdCongRed; refold; tea.
+    instValid Vσ; eapply WIdCongRed; refold; tea.
     eapply wft_Id. 
     2,3: eapply ty_conv.
-    all: now escape.
+    all: now Wescape.
   Qed.
 
 
-  Lemma IdTmValid {Γ l A x y} 
-    (VΓ : [||-v Γ]) 
+  Lemma IdTmValid {wl Γ l A x y} 
+    (VΓ : [||-v Γ]< wl >) 
     (VU := UValid VΓ)
-    (VAU : [_ ||-v<one> A : U | VΓ | VU]) 
+    (VAU : [_ ||-v<one> A : U | VΓ | VU]< wl >) 
     (VA := univValid VΓ VU VAU)
-    (Vx : [_ ||-v<l> x : _ | _ | VA])
-    (Vy : [_ ||-v<l> y : _ | _ | VA]) :
-    [_ ||-v<one> tId A x y : _ | VΓ | VU].
+    (Vx : [_ ||-v<l> x : _ | _ | VA]< wl >)
+    (Vy : [_ ||-v<l> y : _ | _ | VA]< wl >) :
+    [_ ||-v<one> tId A x y : _ | VΓ | VU]< wl >.
   Proof. 
     unshelve econstructor; intros.
-    - instValid Vσ. 
-      unshelve eapply IdRedU; refold; tea.
-      1: now eapply univValid.
-      all: irrelevance.
+    - instValid Vσ.
+      unshelve econstructor ; [ shelve | ].
+      intros wl'' Ho Ho'.
+      pose (f' := over_tree_le Ho').
+      unshelve eapply WIdRedU; refold ; tea.
     - instAllValid Vσ Vσ' Vσσ'.
-      unshelve eapply IdCongRedU; refold; tea.
-      1,2: now eapply univValid.
-      all: irrelevance.
+      unshelve eapply WIdCongRedU; refold; tea.
   Qed.
     
-  Lemma IdTmCongValid {Γ l A A' x x' y y'}
-    (VΓ : [||-v Γ]) 
+  Lemma IdTmCongValid {wl Γ l A A' x x' y y'}
+    (VΓ : [||-v Γ]< wl >) 
     (VU := UValid VΓ)
-    (VAU : [_ ||-v<one> A : _ | VΓ | VU]) 
+    (VAU : [_ ||-v<one> A : _ | VΓ | VU]< wl >) 
     (VA := univValid VΓ VU VAU)
-    (VAU' : [_ ||-v<one> A' : _ | VΓ | VU]) 
-    (VAAU' : [_ ||-v<one> A ≅ A' : _ | VΓ | VU]) 
-    (Vx : [_ ||-v<l> x : _ | _ | VA])
-    (Vx' : [_ ||-v<l> x' : _ | _ | VA])
-    (Vxx' : [_ ||-v<l> x ≅ x' : _ | _ | VA])
-    (Vy : [_ ||-v<l> y : _ | _ | VA]) 
-    (Vy' : [_ ||-v<l> y' : _ | _ | VA]) 
-    (Vyy' : [_ ||-v<l> y ≅ y' : _ | _ | VA]) :
-    [_ ||-v<one> tId A x y ≅ tId A' x' y' : _ | VΓ | VU].
+    (VAU' : [_ ||-v<one> A' : _ | VΓ | VU]< wl >) 
+    (VAAU' : [_ ||-v<one> A ≅ A' : _ | VΓ | VU]< wl >) 
+    (Vx : [_ ||-v<l> x : _ | _ | VA]< wl >)
+    (Vx' : [_ ||-v<l> x' : _ | _ | VA]< wl >)
+    (Vxx' : [_ ||-v<l> x ≅ x' : _ | _ | VA]< wl >)
+    (Vy : [_ ||-v<l> y : _ | _ | VA]< wl >) 
+    (Vy' : [_ ||-v<l> y' : _ | _ | VA]< wl >) 
+    (Vyy' : [_ ||-v<l> y ≅ y' : _ | _ | VA]< wl >) :
+    [_ ||-v<one> tId A x y ≅ tId A' x' y' : _ | VΓ | VU]< wl >.
   Proof.
     constructor; intros; instValid Vσ.
-    unshelve eapply IdCongRedU; refold; tea.
-    1,2: now eapply univValid.
-    2,5: eapply LRTmRedConv; [eapply univEqValid; irrValid|].
-    all: irrelevance.
-    Unshelve. 3,9: now eapply univValid.
-    all: tea.
-  Qed.
+    unshelve eapply WIdCongRedU; refold; tea.
+    1: now eapply univValid.
+    all: eapply WLRTmRedConv ; [ eapply univEqValid; irrValid | ].
+    all: Wirrelevance0 ; [ reflexivity | eassumption].
+    Unshelve.
+    all: eassumption.
+Qed.    
 
-
-  Lemma reflValid {Γ l A x} 
-    (VΓ : [||-v Γ]) 
-    (VA : [_ ||-v<l> A | VΓ]) 
-    (Vx : [_ ||-v<l> x : _ | _ | VA])
-    (VId : [_ ||-v<l> tId A x x | VΓ]) :
-    [_ ||-v<l> tRefl A x : _ | _ | VId].
+  Lemma reflValid {wl Γ l A x} 
+    (VΓ : [||-v Γ]< wl >) 
+    (VA : [_ ||-v<l> A | VΓ]< wl >) 
+    (Vx : [_ ||-v<l> x : _ | _ | VA]< wl >)
+    (VId : [_ ||-v<l> tId A x x | VΓ]< wl >) :
+    [_ ||-v<l> tRefl A x : _ | _ | VId]< wl >.
   Proof.
     unshelve econstructor; intros.
-    - instValid Vσ; now unshelve eapply reflRed.
-    - instAllValid Vσ Vσ' Vσσ'; escape; now unshelve eapply reflCongRed.
+    - instValid Vσ; now unshelve eapply WreflRed.
+    - instAllValid Vσ Vσ' Vσσ'; Wescape; now unshelve eapply WreflCongRed.
   Qed.
 
-  Lemma reflCongValid {Γ l A A' x x'}
-    (VΓ : [||-v Γ]) 
-    (VA : [_ ||-v<l> A | VΓ]) 
-    (VA' : [_ ||-v<l> A' | VΓ]) 
-    (VAA' : [_ ||-v<l> A ≅ A' | VΓ | VA]) 
-    (Vx : [_ ||-v<l> x : _ | _ | VA])
-    (Vx' : [_ ||-v<l> x' : _ | _ | VA])
-    (Vxx' : [_ ||-v<l> x ≅ x' : _ | _ | VA])
-    (VId : [_ ||-v<l> tId A x x | VΓ]) :
-    [_ ||-v<l> tRefl A x ≅ tRefl A' x' : _ | _ | VId].
+  Lemma reflCongValid {wl Γ l A A' x x'}
+    (VΓ : [||-v Γ]< wl >) 
+    (VA : [_ ||-v<l> A | VΓ]< wl >) 
+    (VA' : [_ ||-v<l> A' | VΓ]< wl >) 
+    (VAA' : [_ ||-v<l> A ≅ A' | VΓ | VA]< wl >) 
+    (Vx : [_ ||-v<l> x : _ | _ | VA]< wl >)
+    (Vx' : [_ ||-v<l> x' : _ | _ | VA]< wl >)
+    (Vxx' : [_ ||-v<l> x ≅ x' : _ | _ | VA]< wl >)
+    (VId : [_ ||-v<l> tId A x x | VΓ]< wl >) :
+    [_ ||-v<l> tRefl A x ≅ tRefl A' x' : _ | _ | VId]< wl >.
   Proof.
     constructor; intros; instValid Vσ.
-    escape; unshelve eapply reflCongRed; refold; tea.
+    Wescape; unshelve eapply WreflCongRed; refold; tea.
     now eapply ty_conv.
   Qed.
 
@@ -123,42 +121,41 @@ Context `{GenericTypingProperties}.
   Lemma subst_upup_scons2 (P e y : term) (σ : nat -> term) : P[up_term_term (up_term_term σ)][e .: y..] = P [e .: (y .: σ)].
   Proof. now asimpl. Qed.
 
-  Lemma consSubstS' {Γ σ t l A Δ} 
-    (VΓ : [||-v Γ])
-    (VΓA : [||-v Γ ,, A])
-    (wfΔ : [|- Δ])
-    (Vσ : [Δ ||-v σ : Γ | VΓ | wfΔ])
-    (VA : [Γ ||-v<l> A | VΓ])
-    (Vt : [ Δ ||-<l> t : A[σ] | validTy VA wfΔ Vσ]) :
-    [Δ ||-v (t .: σ) : Γ ,, A | VΓA | wfΔ].
-  Proof. 
-    pose proof (invValiditySnoc VΓA) as [? [? [? ->]]].
-    unshelve eapply consSubstS; [ irrValid| irrelevance].
+  Lemma consSubstS' {wl Γ σ t l A Δ wl' f} 
+    (VΓ : [||-v Γ]< wl >)
+    (VΓA : [||-v Γ ,, A]< wl >)
+    (wfΔ : [|- Δ]< wl' >)
+    (Vσ : [Δ ||-v σ : Γ | VΓ | wfΔ | f]< wl >)
+    (VA : [Γ ||-v<l> A | VΓ]< wl >)
+    (Vt : W[ Δ ||-<l> t : A[σ] | validTy VA f wfΔ Vσ]< wl' >) :
+    [Δ ||-v (t .: σ) : Γ ,, A | VΓA | wfΔ | f]< wl >.
+  Proof.
+    pose proof (consSubstS VΓ wfΔ Vσ VA Vt).
+    irrValid.
   Qed.
 
-  Lemma consSubstSEq'' {Γ σ σ' t u l A Δ} 
-    (VΓ : [||-v Γ])
-    (VΓA : [||-v Γ ,, A])
-    (wfΔ : [|- Δ])
-    (Vσ : [Δ ||-v σ : Γ | VΓ | wfΔ])
-    (Vσσ' : [Δ ||-v σ ≅ σ' : Γ | VΓ | wfΔ | Vσ])
-    (VA : [Γ ||-v<l> A | VΓ])
-    (Vt : [Δ ||-<l> t : A[σ] | validTy VA wfΔ Vσ])
-    (Vtu : [Δ ||-<l> t ≅ u : A[σ] | validTy VA wfΔ Vσ])
-    (Vσt : [_ ||-v (t .: σ) : _ | VΓA | wfΔ]) :
-    [Δ ||-v (t .: σ) ≅  (u .: σ') : Γ ,, A | VΓA | wfΔ | Vσt].
+  Lemma consSubstSEq'' {wl Γ σ σ' t u l A Δ wl' f} 
+    (VΓ : [||-v Γ]< wl >)
+    (VΓA : [||-v Γ ,, A]< wl >)
+    (wfΔ : [|- Δ]< wl' >)
+    (Vσ : [Δ ||-v σ : Γ | VΓ | wfΔ | f]< wl >)
+    (Vσσ' : [Δ ||-v σ ≅ σ' : Γ | VΓ | wfΔ | Vσ | f]< wl >)
+    (VA : [Γ ||-v<l> A | VΓ]< wl >)
+    (Vt : W[Δ ||-<l> t : A[σ] | validTy VA f wfΔ Vσ]< wl' >)
+    (Vtu : W[Δ ||-<l> t ≅ u : A[σ] | validTy VA f wfΔ Vσ]< wl' >)
+    (Vσt : [_ ||-v (t .: σ) : _ | VΓA | wfΔ | f]< wl >) :
+    [Δ ||-v (t .: σ) ≅  (u .: σ') : Γ ,, A | VΓA | wfΔ | Vσt | f]< wl >.
   Proof.
-    pose proof (invValiditySnoc VΓA) as [? [? [? ->]]].
     pose proof (consSubstSEq' VΓ wfΔ Vσ Vσσ' VA Vt Vtu).
     irrValid.
   Qed.  
 
 
-  Lemma idElimMotiveCtxIdValid {Γ l A x}
-    (VΓ : [||-v Γ]) 
-    (VA : [_ ||-v<l> A | VΓ]) 
-    (Vx : [_ ||-v<l> x : _ | _ | VA]) :
-    [Γ,, A ||-v< l > tId A⟨@wk1 Γ A⟩ x⟨@wk1 Γ A⟩ (tRel 0) | validSnoc VΓ VA].
+  Lemma idElimMotiveCtxIdValid {wl Γ l A x}
+    (VΓ : [||-v Γ]< wl >) 
+    (VA : [_ ||-v<l> A | VΓ]< wl >) 
+    (Vx : [_ ||-v<l> x : _ | _ | VA]< wl >) :
+    [Γ,, A ||-v< l > tId A⟨@wk1 Γ A⟩ x⟨@wk1 Γ A⟩ (tRel 0) | validSnoc' VΓ VA]< wl >.
   Proof.
     unshelve eapply IdValid.
     - now eapply wk1ValidTy.
@@ -166,16 +163,16 @@ Context `{GenericTypingProperties}.
     - exact (var0Valid VΓ VA).
   Qed.
   
-  Lemma idElimMotiveCtxIdCongValid {Γ l A A' x x'}
-    (VΓ : [||-v Γ]) 
-    (VA : [_ ||-v<l> A | VΓ]) 
-    (VA' : [_ ||-v<l> A' | VΓ]) 
-    (VAA' : [_ ||-v<l> A ≅ A' | VΓ | VA])
-    (Vx : [_ ||-v<l> x : _ | _ | VA]) 
-    (Vx' : [_ ||-v<l> x' : _ | _ | VA]) 
-    (Vxx' : [_ ||-v<l> x ≅ x' : _ | _ | VA]) 
-    (VId : [Γ,, A ||-v< l > tId A⟨@wk1 Γ A⟩ x⟨@wk1 Γ A⟩ (tRel 0) | validSnoc VΓ VA]) :
-    [_ ||-v<l> _ ≅ tId A'⟨@wk1 Γ A'⟩ x'⟨@wk1 Γ A'⟩ (tRel 0) | validSnoc VΓ VA | VId].
+  Lemma idElimMotiveCtxIdCongValid {wl Γ l A A' x x'}
+    (VΓ : [||-v Γ]< wl >) 
+    (VA : [_ ||-v<l> A | VΓ]< wl >) 
+    (VA' : [_ ||-v<l> A' | VΓ]< wl >) 
+    (VAA' : [_ ||-v<l> A ≅ A' | VΓ | VA]< wl >)
+    (Vx : [_ ||-v<l> x : _ | _ | VA]< wl >) 
+    (Vx' : [_ ||-v<l> x' : _ | _ | VA]< wl >) 
+    (Vxx' : [_ ||-v<l> x ≅ x' : _ | _ | VA]< wl >) 
+    (VId : [Γ,, A ||-v< l > tId A⟨@wk1 Γ A⟩ x⟨@wk1 Γ A⟩ (tRel 0) | validSnoc' VΓ VA]< wl >) :
+    [_ ||-v<l> _ ≅ tId A'⟨@wk1 Γ A'⟩ x'⟨@wk1 Γ A'⟩ (tRel 0) | validSnoc' VΓ VA | VId]< wl >.
   Proof.
     assert (h : forall t, t⟨@wk1 Γ A'⟩ = t⟨@wk1 Γ A⟩) by reflexivity.
     unshelve eapply IdCongValid.
@@ -191,73 +188,74 @@ Context `{GenericTypingProperties}.
   Qed.
   
   
-  Lemma idElimMotiveScons2Valid {Γ l A x y e}
-    (VΓ : [||-v Γ]) 
-    (VA : [_ ||-v<l> A | VΓ]) 
-    (Vx : [_ ||-v<l> x : _ | _ | VA])
-    (Vy : [Γ ||-v<l> y : _ | _ | VA])
-    (VId : [Γ ||-v<l> tId A x y | VΓ])
-    (Ve : [_ ||-v<l> e : _ | _ | VId]) 
-    (VΓext : [||-v (Γ ,, A) ,, tId A⟨@wk1 Γ A⟩ x⟨@wk1 Γ A⟩ (tRel 0)])
-    Δ σ (wfΔ: [ |-[ ta ] Δ]) (vσ: [VΓ | Δ ||-v σ : _ | wfΔ]) :
-      [VΓext | Δ ||-v (e[σ] .: (y[σ] .: σ)) : _ | wfΔ].
+  Lemma idElimMotiveScons2Valid {wl Γ l A x y e}
+    (VΓ : [||-v Γ]< wl >) 
+    (VA : [_ ||-v<l> A | VΓ]< wl >) 
+    (Vx : [_ ||-v<l> x : _ | _ | VA]< wl >)
+    (Vy : [Γ ||-v<l> y : _ | _ | VA]< wl >)
+    (VId : [Γ ||-v<l> tId A x y | VΓ]< wl >)
+    (Ve : [_ ||-v<l> e : _ | _ | VId]< wl >) 
+    (VΓext : [||-v (Γ ,, A) ,, tId A⟨@wk1 Γ A⟩ x⟨@wk1 Γ A⟩ (tRel 0)]< wl >)
+    Δ σ wl' f (wfΔ: [ |-[ ta ] Δ]< wl' >) (vσ: [VΓ | Δ ||-v σ : _ | wfΔ | f]< wl >) :
+      [VΓext | Δ ||-v (e[σ] .: (y[σ] .: σ)) : _ | wfΔ| f]< wl >.
   Proof.
     intros; unshelve eapply consSubstS'; tea.
     2: now eapply consSubstSvalid.
     1: now eapply idElimMotiveCtxIdValid.
-    instValid vσ; irrelevance.
+    instValid vσ; Wirrelevance.
   Qed.
   
-  Lemma substIdElimMotive {Γ l A x P y e}
-    (VΓ : [||-v Γ]) 
-    (VA : [_ ||-v<l> A | VΓ]) 
-    (Vx : [_ ||-v<l> x : _ | _ | VA])
-    (VΓext : [||-v (Γ ,, A) ,, tId A⟨@wk1 Γ A⟩ x⟨@wk1 Γ A⟩ (tRel 0)])
-    (VP : [_ ||-v<l> P | VΓext])
-    (Vy : [Γ ||-v<l> y : _ | _ | VA])
-    (VId : [Γ ||-v<l> tId A x y | VΓ])
-    (Ve : [_ ||-v<l> e : _ | _ | VId]) : 
-    [_ ||-v<l> P[e .: y ..] | VΓ].
+  Lemma substIdElimMotive {wl Γ l A x P y e}
+    (VΓ : [||-v Γ]< wl >) 
+    (VA : [_ ||-v<l> A | VΓ]< wl >) 
+    (Vx : [_ ||-v<l> x : _ | _ | VA]< wl >)
+    (VΓext : [||-v (Γ ,, A) ,, tId A⟨@wk1 Γ A⟩ x⟨@wk1 Γ A⟩ (tRel 0)]< wl >)
+    (VP : [_ ||-v<l> P | VΓext]< wl >)
+    (Vy : [Γ ||-v<l> y : _ | _ | VA]< wl >)
+    (VId : [Γ ||-v<l> tId A x y | VΓ]< wl >)
+    (Ve : [_ ||-v<l> e : _ | _ | VId]< wl >) : 
+    [_ ||-v<l> P[e .: y ..] | VΓ]< wl >.
   Proof.
     opector; intros.
     - rewrite subst_scons2; eapply validTy; tea; now eapply idElimMotiveScons2Valid.
-    - irrelevance0 ; rewrite subst_scons2;[reflexivity|].
+    - Wirrelevance0 ; rewrite subst_scons2;[reflexivity|].
       unshelve eapply validTyExt.
-      5,6: eapply idElimMotiveScons2Valid; cycle 1; tea.
+      7,8: eapply idElimMotiveScons2Valid; cycle 1; tea.
       1: tea.
       eapply consSubstSEq''.
       + now unshelve eapply consSubstSEqvalid.
-      + instValid vσ; irrelevance.
-      + instAllValid vσ vσ' vσσ'; irrelevance.
+      + instValid vσ; Wirrelevance.
+      + instAllValid vσ vσ' vσσ'; Wirrelevance.
       Unshelve. 2: now eapply idElimMotiveCtxIdValid.
   Qed.
   
 
-  Lemma subst_idElimMotive_substupup {Γ Δ l A x P y e σ}
-    (VΓ : [||-v Γ]) 
-    (wfΔ : [|- Δ])
-    (Vσ : [_ ||-v σ : _ | VΓ | wfΔ])
-    (VA : [_ ||-v<l> A | VΓ]) 
-    (RVA := validTy VA wfΔ Vσ)
-    (Vx : [_ ||-v<l> x : _ | _ | VA])
-    (VΓext : [||-v (Γ ,, A) ,, tId A⟨@wk1 Γ A⟩ x⟨@wk1 Γ A⟩ (tRel 0)])
-    (VP : [_ ||-v<l> P | VΓext])
-    (Ry : [ RVA |  _ ||- y : _])
-    (RId : [Δ ||-<l> tId A[σ] x[σ] y])
-    (Re : [RId | _ ||- e : _]) :
-    [Δ ||-<l> P[up_term_term (up_term_term σ)][e .: y ..]].
+  Lemma subst_idElimMotive_substupup {wl Γ Δ l A x P y e σ wl' f}
+    (VΓ : [||-v Γ]< wl >) 
+    (wfΔ : [|- Δ]< wl' >)
+    (Vσ : [_ ||-v σ : _ | VΓ | wfΔ | f]< wl >)
+    (VA : [_ ||-v<l> A | VΓ]< wl >) 
+    (RVA := validTy VA f wfΔ Vσ)
+    (Vx : [_ ||-v<l> x : _ | _ | VA]< wl >)
+    (VΓext : [||-v (Γ ,, A) ,, tId A⟨@wk1 Γ A⟩ x⟨@wk1 Γ A⟩ (tRel 0)]< wl >)
+    (VP : [_ ||-v<l> P | VΓext]< wl >)
+    (Ry : W[ _ ||-< l > y : _ | RVA]< wl' >)
+    (RId : W[Δ ||-<l> tId A[σ] x[σ] y]< wl' >)
+    (Re : W[ _ ||-< l > e : _ | RId]< wl' >) :
+    W[Δ ||-<l> P[up_term_term (up_term_term σ)][e .: y ..]]< wl' >.
   Proof.
-    pose (VΓA := validSnoc VΓ VA). 
+    pose (VΓA := validSnoc' VΓ VA). 
     rewrite subst_upup_scons2.
-    unshelve eapply validTy; cycle 2; tea.
+    unshelve eapply validTy; cycle 4 ; tea.
     unshelve eapply consSubstS'; tea.
     + now eapply consSubstS.
     + now eapply idElimMotiveCtxIdValid.
-    + irrelevance.
+    + Wirrelevance.
   Qed.
   
-  Lemma irrelevanceSubst' {Γ} (VΓ VΓ' : [||-v Γ]) {σ Δ Δ'} (wfΔ : [|- Δ]) (wfΔ' : [|- Δ']) : Δ = Δ' ->
-    [Δ ||-v σ : Γ | VΓ | wfΔ] -> [Δ' ||-v σ : Γ | VΓ' | wfΔ'].
+  Lemma irrelevanceSubst' {wl Γ} (VΓ VΓ' : [||-v Γ]< wl >) {σ Δ Δ' wl' f}
+    (wfΔ : [|- Δ]< wl' >) (wfΔ' : [|- Δ']< wl' >) : Δ = Δ' ->
+    [Δ ||-v σ : Γ | VΓ | wfΔ | f]< wl > -> [Δ' ||-v σ : Γ | VΓ' | wfΔ' |f]< wl >.
   Proof.
     intros ->; eapply irrelevanceSubst.
   Qed.
@@ -266,21 +264,21 @@ Context `{GenericTypingProperties}.
     tId A[σ]⟨@wk1 Δ A[σ]⟩ x[σ]⟨@wk1 Δ A[σ]⟩ (tRel 0) = (tId A⟨@wk1 Γ A⟩ x⟨@wk1 Γ A⟩ (tRel 0))[up_term_term σ].
   Proof. now bsimpl. Qed.
   
-  Lemma red_idElimMotive_substupup {Γ Δ l A x P σ}
-    (VΓ : [||-v Γ]) 
-    (wfΔ : [|- Δ])
-    (Vσ : [_ ||-v σ : _ | VΓ | wfΔ])
-    (VA : [_ ||-v<l> A | VΓ]) 
-    (Vx : [_ ||-v<l> x : _ | _ | VA])
-    (VΓext : [||-v (Γ ,, A) ,, tId A⟨@wk1 Γ A⟩ x⟨@wk1 Γ A⟩ (tRel 0)])
-    (VP : [_ ||-v<l> P | VΓext]) :
-    [(Δ ,, A[σ]),, tId A[σ]⟨@wk1 Δ A[σ]⟩ x[σ]⟨@wk1 Δ A[σ]⟩ (tRel 0) ||-<l> P[up_term_term (up_term_term σ)]].
+  Lemma red_idElimMotive_substupup {wl Γ Δ l A x P σ wl' f}
+    (VΓ : [||-v Γ]< wl >) 
+    (wfΔ : [|- Δ]< wl' >)
+    (Vσ : [_ ||-v σ : _ | VΓ | wfΔ | f]< wl >)
+    (VA : [_ ||-v<l> A | VΓ]< wl >) 
+    (Vx : [_ ||-v<l> x : _ | _ | VA]< wl >)
+    (VΓext : [||-v (Γ ,, A) ,, tId A⟨@wk1 Γ A⟩ x⟨@wk1 Γ A⟩ (tRel 0)]< wl >)
+    (VP : [_ ||-v<l> P | VΓext]< wl >) :
+   W[(Δ ,, A[σ]),, tId A[σ]⟨@wk1 Δ A[σ]⟩ x[σ]⟨@wk1 Δ A[σ]⟩ (tRel 0) ||-<l> P[up_term_term (up_term_term σ)]]< wl' >.
   Proof.
-    pose (VΓA := validSnoc VΓ VA). 
+    pose (VΓA := validSnoc' VΓ VA). 
     instValid Vσ.
-    unshelve eapply validTy; cycle 2; tea.
-    * escape. 
-      assert [|- Δ,, A[σ]] by now eapply wfc_cons.
+    unshelve eapply validTy; cycle 4; tea.
+    * Wescape. 
+      assert [|- Δ,, A[σ]]< wl' > by now eapply wfc_cons.
       eapply wfc_cons; tea.
       eapply wft_Id.
       1: now eapply wft_wk.
@@ -294,32 +292,33 @@ Context `{GenericTypingProperties}.
       Unshelve. 2: now eapply idElimMotiveCtxIdValid.
   Qed.
 
-  Lemma irrelevanceSubstEq' {Γ} (VΓ VΓ' : [||-v Γ]) {σ σ' Δ Δ'} (wfΔ : [|- Δ]) (wfΔ' : [|- Δ'])
-    (Vσ : [Δ ||-v σ : Γ | VΓ | wfΔ]) (Vσ' : [Δ' ||-v σ : Γ | VΓ' | wfΔ']) :
+  Lemma irrelevanceSubstEq' {wl Γ} (VΓ VΓ' : [||-v Γ]< wl >) {σ σ' Δ Δ' wl' f}
+    (wfΔ : [|- Δ]< wl' >) (wfΔ' : [|- Δ']< wl' >)
+    (Vσ : [Δ ||-v σ : Γ | VΓ | wfΔ | f]< wl >) (Vσ' : [Δ' ||-v σ : Γ | VΓ' | wfΔ' | f]< wl >) :
     Δ = Δ' ->
-    [Δ ||-v σ ≅ σ' : Γ | VΓ | wfΔ | Vσ] -> [Δ' ||-v σ ≅ σ' : Γ | VΓ' | wfΔ' | Vσ'].
+    [Δ ||-v σ ≅ σ' : Γ | VΓ | wfΔ | Vσ | f]< wl > -> [Δ' ||-v σ ≅ σ' : Γ | VΓ' | wfΔ' | Vσ' | f]< wl >.
   Proof.
     intros ->; eapply irrelevanceSubstEq.
   Qed.
   
-  Lemma red_idElimMotive_substupup_cong {Γ Δ l A x P σ σ'}
-    (VΓ : [||-v Γ]) 
-    (wfΔ : [|- Δ])
-    (Vσ : [_ ||-v σ : _ | VΓ | wfΔ])
-    (Vσ' : [_ ||-v σ' : _ | VΓ | wfΔ])
-    (Vσσ' : [_ ||-v σ ≅ σ' : _ | VΓ | wfΔ | Vσ])
-    (VA : [_ ||-v<l> A | VΓ]) 
-    (Vx : [_ ||-v<l> x : _ | _ | VA])
-    (VΓext : [||-v (Γ ,, A) ,, tId A⟨@wk1 Γ A⟩ x⟨@wk1 Γ A⟩ (tRel 0)])
-    (VP : [_ ||-v<l> P | VΓext]) 
-    (RPσ : [(Δ ,, A[σ]),, tId A[σ]⟨@wk1 Δ A[σ]⟩ x[σ]⟨@wk1 Δ A[σ]⟩ (tRel 0) ||-<l> P[up_term_term (up_term_term σ)]]) :
-    [RPσ | _ ||- _ ≅ P[up_term_term (up_term_term σ')]].
+  Lemma red_idElimMotive_substupup_cong {wl Γ Δ l A x P σ σ' wl' f}
+    (VΓ : [||-v Γ]< wl >) 
+    (wfΔ : [|- Δ]< wl' >)
+    (Vσ : [_ ||-v σ : _ | VΓ | wfΔ | f]< wl >)
+    (Vσ' : [_ ||-v σ' : _ | VΓ | wfΔ | f]< wl >)
+    (Vσσ' : [_ ||-v σ ≅ σ' : _ | VΓ | wfΔ | Vσ| f]< wl >)
+    (VA : [_ ||-v<l> A | VΓ]< wl >) 
+    (Vx : [_ ||-v<l> x : _ | _ | VA]< wl >)
+    (VΓext : [||-v (Γ ,, A) ,, tId A⟨@wk1 Γ A⟩ x⟨@wk1 Γ A⟩ (tRel 0)]< wl >)
+    (VP : [_ ||-v<l> P | VΓext]< wl >) 
+    (RPσ : W[(Δ ,, A[σ]),, tId A[σ]⟨@wk1 Δ A[σ]⟩ x[σ]⟨@wk1 Δ A[σ]⟩ (tRel 0) ||-<l> P[up_term_term (up_term_term σ)]]< wl' >) :
+    W[_ ||-< l > _ ≅ P[up_term_term (up_term_term σ')]| RPσ]< wl' >.
   Proof.
-    pose (VΓA := validSnoc VΓ VA). 
+    pose (VΓA := validSnoc' VΓ VA). 
     instAllValid Vσ Vσ' Vσσ'.
-    irrelevanceRefl; unshelve eapply validTyExt; cycle 2; tea.
-    * escape. 
-      assert [|- Δ,, A[σ]] by now eapply wfc_cons.
+    Wirrelevance0 ; [reflexivity | ] ; unshelve eapply validTyExt; cycle 3 ; tea.
+    * Wescape. 
+      assert [|- Δ,, A[σ]]< wl' > by now eapply wfc_cons.
       eapply wfc_cons; tea.
       eapply wft_Id.
       1: now eapply wft_wk.
@@ -346,28 +345,28 @@ Context `{GenericTypingProperties}.
       2: now eapply idElimMotiveCtxIdValid.
   Qed.
 
-  Lemma redEq_idElimMotive_substupup {Γ Δ l A A' x x' P P' σ}
-    (VΓ : [||-v Γ]) 
-    (wfΔ : [|- Δ])
-    (Vσ : [_ ||-v σ : _ | VΓ | wfΔ])
-    (VA : [_ ||-v<l> A | VΓ]) 
-    (VA' : [_ ||-v<l> A' | VΓ]) 
-    (VAA' : [_ ||-v<l> A ≅ A' | _ | VA])
-    (Vx : [_ ||-v<l> x : _ | _ | VA])
-    (Vx' : [_ ||-v<l> x' : _ | _ | VA])
-    (Vxx' : [_ ||-v<l> x ≅ x' : _ | _ | VA])
-    (VΓext : [||-v (Γ ,, A) ,, tId A⟨@wk1 Γ A⟩ x⟨@wk1 Γ A⟩ (tRel 0)])
-    (VP : [_ ||-v<l> P | VΓext])
-    (VP' : [_ ||-v<l> P' | VΓext])
-    (VPP' : [_ ||-v<l> P ≅ P' | _ | VP]) 
-    (VPsubstupup : [(Δ ,, A[σ]),, tId A[σ]⟨@wk1 Δ A[σ]⟩ x[σ]⟨@wk1 Δ A[σ]⟩ (tRel 0) ||-<l> P[up_term_term (up_term_term σ)]]) :
-    [_ ||-<l> _ ≅ P'[up_term_term (up_term_term σ)] | VPsubstupup].
+  Lemma redEq_idElimMotive_substupup {wl Γ Δ l A A' x x' P P' σ wl' f}
+    (VΓ : [||-v Γ]< wl >) 
+    (wfΔ : [|- Δ]< wl' >)
+    (Vσ : [_ ||-v σ : _ | VΓ | wfΔ | f]< wl >)
+    (VA : [_ ||-v<l> A | VΓ]< wl >) 
+    (VA' : [_ ||-v<l> A' | VΓ]< wl >) 
+    (VAA' : [_ ||-v<l> A ≅ A' | _ | VA]< wl >)
+    (Vx : [_ ||-v<l> x : _ | _ | VA]< wl >)
+    (Vx' : [_ ||-v<l> x' : _ | _ | VA]< wl >)
+    (Vxx' : [_ ||-v<l> x ≅ x' : _ | _ | VA]< wl >)
+    (VΓext : [||-v (Γ ,, A) ,, tId A⟨@wk1 Γ A⟩ x⟨@wk1 Γ A⟩ (tRel 0)]< wl >)
+    (VP : [_ ||-v<l> P | VΓext]< wl >)
+    (VP' : [_ ||-v<l> P' | VΓext]< wl >)
+    (VPP' : [_ ||-v<l> P ≅ P' | _ | VP]< wl >) 
+    (VPsubstupup : W[(Δ ,, A[σ]),, tId A[σ]⟨@wk1 Δ A[σ]⟩ x[σ]⟨@wk1 Δ A[σ]⟩ (tRel 0) ||-<l> P[up_term_term (up_term_term σ)]]< wl' >) :
+    W[_ ||-<l> _ ≅ P'[up_term_term (up_term_term σ)] | VPsubstupup]< wl' >.
   Proof.
-    pose (VΓA := validSnoc VΓ VA). 
+    pose (VΓA := validSnoc' VΓ VA). 
     instValid Vσ.
-    irrelevanceRefl; unshelve eapply validTyEq; cycle 2; tea.
-    * escape. 
-      assert [|- Δ,, A[σ]] by now eapply wfc_cons.
+    Wirrelevance0 ; [reflexivity | ] ; unshelve eapply validTyEq; cycle 4; tea.
+    * Wescape. 
+      assert [|- Δ,, A[σ]]< wl' > by now eapply wfc_cons.
       eapply wfc_cons; tea.
       eapply wft_Id.
       1: now eapply wft_wk.
@@ -382,165 +381,165 @@ Context `{GenericTypingProperties}.
   Qed.
 
 
-  Lemma substEq_idElimMotive_substupupEq {Γ Δ l A x P y y' e e' σ σ'}
-    (VΓ : [||-v Γ]) 
-    (wfΔ : [|- Δ])
-    (Vσ : [_ ||-v σ : _ | VΓ | wfΔ])
-    (Vσ' : [_ ||-v σ' : _ | VΓ | wfΔ])
-    (Vσσ' : [_ ||-v σ ≅ σ' : _ | VΓ | wfΔ | Vσ])
-    (VA : [_ ||-v<l> A | VΓ]) 
-    (RVA := validTy VA wfΔ Vσ)
-    (RVA' := validTy VA wfΔ Vσ')
-    (Vx : [_ ||-v<l> x : _ | _ | VA])
-    (VΓext : [||-v (Γ ,, A) ,, tId A⟨@wk1 Γ A⟩ x⟨@wk1 Γ A⟩ (tRel 0)])
-    (VP : [_ ||-v<l> P | VΓext])
-    (Ry : [ RVA |  _ ||- y : _])
-    (Ry' : [ RVA' |  _ ||- y' : _])
-    (Ryy' : [ RVA |  _ ||- y ≅ y' : _])
-    (RId : [Δ ||-<l> tId A[σ] x[σ] y])
-    (RId' : [Δ ||-<l> tId A[σ'] x[σ'] y'])
-    (Re : [RId | _ ||- e : _])
-    (Re' : [RId' | _ ||- e' : _])
-    (Ree' : [RId | _ ||- e ≅ e' : _])
-    (RPsubst : [Δ ||-<l> P[up_term_term (up_term_term σ)][e .: y ..]]) :
-    [RPsubst | Δ ||- P[up_term_term (up_term_term σ)][e .: y ..] ≅ P[up_term_term (up_term_term σ')][e' .: y' ..]].
+  Lemma substEq_idElimMotive_substupupEq {wl Γ Δ l A x P y y' e e' σ σ' wl' f}
+    (VΓ : [||-v Γ]< wl >) 
+    (wfΔ : [|- Δ]< wl' >)
+    (Vσ : [_ ||-v σ : _ | VΓ | wfΔ | f]< wl >)
+    (Vσ' : [_ ||-v σ' : _ | VΓ | wfΔ | f]< wl >)
+    (Vσσ' : [_ ||-v σ ≅ σ' : _ | VΓ | wfΔ | Vσ | f]< wl >)
+    (VA : [_ ||-v<l> A | VΓ]< wl >) 
+    (RVA := validTy VA f wfΔ Vσ)
+    (RVA' := validTy VA f wfΔ Vσ')
+    (Vx : [_ ||-v<l> x : _ | _ | VA]< wl >)
+    (VΓext : [||-v (Γ ,, A) ,, tId A⟨@wk1 Γ A⟩ x⟨@wk1 Γ A⟩ (tRel 0)]< wl >)
+    (VP : [_ ||-v<l> P | VΓext]< wl >)
+    (Ry : W[  _ ||-< l > y : _ | RVA]< wl' >)
+    (Ry' : W[  _ ||-< l > y' : _ | RVA']< wl' >)
+    (Ryy' : W[  _ ||-< l > y ≅ y' : _ | RVA]< wl' >)
+    (RId : W[Δ ||-<l> tId A[σ] x[σ] y]< wl' >)
+    (RId' : W[Δ ||-<l> tId A[σ'] x[σ'] y']< wl' >)
+    (Re : W[ _ ||-< l > e : _ | RId]< wl' >)
+    (Re' : W[ _ ||-< l > e' : _ | RId']< wl' >)
+    (Ree' : W[ _ ||-< l > e ≅ e' : _ | RId]< wl' >)
+    (RPsubst : W[Δ ||-<l> P[up_term_term (up_term_term σ)][e .: y ..]]< wl' >) :
+    W[Δ ||-< l > P[up_term_term (up_term_term σ)][e .: y ..] ≅ P[up_term_term (up_term_term σ')][e' .: y' ..] | RPsubst]< wl' >.
   Proof.
-    pose (VΓA := validSnoc VΓ VA). 
-    irrelevance0; rewrite subst_upup_scons2; [reflexivity|].
-    unshelve eapply validTyExt; cycle 2; tea.
+    pose (VΓA := validSnoc' VΓ VA). 
+    Wirrelevance0; rewrite subst_upup_scons2; [reflexivity|].
+    unshelve eapply validTyExt; cycle 3; tea.
     - unshelve eapply consSubstS'; tea.
       + now eapply consSubstS.
       + now eapply idElimMotiveCtxIdValid.
-      + irrelevance.
+      + Wirrelevance.
     - unshelve eapply consSubstS'; tea.
       + now eapply consSubstS.
       + now eapply idElimMotiveCtxIdValid.
-      + irrelevance.
+      + Wirrelevance.
     - unshelve eapply consSubstSEq''; tea.
-      4,5: irrelevance.
+      4,5: Wirrelevance.
       2: now eapply idElimMotiveCtxIdValid.
       2: unshelve eapply consSubstSEq'; tea.
   Qed.
 
-  Lemma substEq_idElimMotive_substupup {Γ Δ l A x P y y' e e' σ}
-    (VΓ : [||-v Γ]) 
-    (wfΔ : [|- Δ])
-    (Vσ : [_ ||-v σ : _ | VΓ | wfΔ])
-    (VA : [_ ||-v<l> A | VΓ]) 
-    (RVA := validTy VA wfΔ Vσ)
-    (Vx : [_ ||-v<l> x : _ | _ | VA])
-    (VΓext : [||-v (Γ ,, A) ,, tId A⟨@wk1 Γ A⟩ x⟨@wk1 Γ A⟩ (tRel 0)])
-    (VP : [_ ||-v<l> P | VΓext])
-    (Ry : [ RVA |  _ ||- y : _])
-    (Ry' : [ RVA |  _ ||- y' : _])
-    (Ryy' : [ RVA |  _ ||- y ≅ y' : _])
-    (RId : [Δ ||-<l> tId A[σ] x[σ] y])
-    (RId' : [Δ ||-<l> tId A[σ] x[σ] y'])
-    (Re : [RId | _ ||- e : _])
-    (Re' : [RId' | _ ||- e' : _])
-    (Ree' : [RId | _ ||- e ≅ e' : _])
-    (RPsubst : [Δ ||-<l> P[up_term_term (up_term_term σ)][e .: y ..]]) :
-    [RPsubst | Δ ||- P[up_term_term (up_term_term σ)][e .: y ..] ≅ P[up_term_term (up_term_term σ)][e' .: y' ..]].
+  Lemma substEq_idElimMotive_substupup {wl Γ Δ l A x P y y' e e' σ wl' f}
+    (VΓ : [||-v Γ]< wl >) 
+    (wfΔ : [|- Δ]< wl' >)
+    (Vσ : [_ ||-v σ : _ | VΓ | wfΔ| f]< wl >)
+    (VA : [_ ||-v<l> A | VΓ]< wl >) 
+    (RVA := validTy VA f wfΔ Vσ)
+    (Vx : [_ ||-v<l> x : _ | _ | VA]< wl >)
+    (VΓext : [||-v (Γ ,, A) ,, tId A⟨@wk1 Γ A⟩ x⟨@wk1 Γ A⟩ (tRel 0)]< wl >)
+    (VP : [_ ||-v<l> P | VΓext]< wl >)
+    (Ry : W[  _ ||-< l > y : _ | RVA]< wl' >)
+    (Ry' : W[  _ ||-< l > y' : _ | RVA]< wl' >)
+    (Ryy' : W[  _ ||-< l > y ≅ y' : _ | RVA]< wl' >)
+    (RId : W[Δ ||-<l> tId A[σ] x[σ] y]< wl' >)
+    (RId' : W[Δ ||-<l> tId A[σ] x[σ] y']< wl' >)
+    (Re : W[ _ ||-< l > e : _ | RId]< wl' >)
+    (Re' : W[ _ ||-< l > e' : _ | RId']< wl' >)
+    (Ree' : W[ _ ||-< l > e ≅ e' : _ | RId]< wl' >)
+    (RPsubst : W[Δ ||-<l> P[up_term_term (up_term_term σ)][e .: y ..]]< wl' >) :
+    W[Δ ||-< l > P[up_term_term (up_term_term σ)][e .: y ..] ≅ P[up_term_term (up_term_term σ)][e' .: y' ..] | RPsubst]< wl' >.
   Proof.
     eapply substEq_idElimMotive_substupupEq; tea; eapply reflSubst.
   Qed.
 
   Set Printing Primitive Projection Parameters.
 
-  Lemma substExt_idElimMotive_substupup {Γ Δ l A A' x x' P P' y y' e e' σ}
-    (VΓ : [||-v Γ]) 
-    (wfΔ : [|- Δ])
-    (Vσ : [_ ||-v σ : _ | VΓ | wfΔ])
-    (VA : [_ ||-v<l> A | VΓ]) 
-    (VA' : [_ ||-v<l> A' | VΓ]) 
-    (VAA' : [_ ||-v<l> A ≅ A' | _ | VA])
-    (RVA := validTy VA wfΔ Vσ)
-    (Vx : [_ ||-v<l> x : _ | _ | VA])
-    (Vx' : [_ ||-v<l> x' : _ | _ | VA])
-    (Vxx' : [_ ||-v<l> x ≅ x' : _ | _ | VA])
-    (VΓext : [||-v (Γ ,, A) ,, tId A⟨@wk1 Γ A⟩ x⟨@wk1 Γ A⟩ (tRel 0)])
-    (VP : [_ ||-v<l> P | VΓext])
-    (VP' : [_ ||-v<l> P' | VΓext])
-    (VPP' : [_ ||-v<l> P ≅ P' | _ | VP]) 
-    (Ry : [ RVA |  _ ||- y : _])
-    (Ry' : [ RVA |  _ ||- y' : _])
-    (Ryy' : [ RVA |  _ ||- y ≅ y' : _])
-    (RId : [Δ ||-<l> tId A[σ] x[σ] y])
-    (RId' : [Δ ||-<l> tId A[σ] x[σ] y'])
-    (Re : [RId | _ ||- e : _])
-    (Re' : [RId' | _ ||- e' : _])
-    (Ree' : [RId | _ ||- e ≅ e' : _])
-    (RPsubst : [Δ ||-<l> P[up_term_term (up_term_term σ)][e .: y ..]]) :
-    [RPsubst | Δ ||- P[up_term_term (up_term_term σ)][e .: y ..] ≅ P'[up_term_term (up_term_term σ)][e' .: y' ..]].
+  Lemma substExt_idElimMotive_substupup {wl Γ Δ l A A' x x' P P' y y' e e' σ wl' f}
+    (VΓ : [||-v Γ]< wl >) 
+    (wfΔ : [|- Δ]< wl' >)
+    (Vσ : [_ ||-v σ : _ | VΓ | wfΔ | f]< wl >)
+    (VA : [_ ||-v<l> A | VΓ]< wl >) 
+    (VA' : [_ ||-v<l> A' | VΓ]< wl >) 
+    (VAA' : [_ ||-v<l> A ≅ A' | _ | VA]< wl >)
+    (RVA := validTy VA f wfΔ Vσ)
+    (Vx : [_ ||-v<l> x : _ | _ | VA]< wl >)
+    (Vx' : [_ ||-v<l> x' : _ | _ | VA]< wl >)
+    (Vxx' : [_ ||-v<l> x ≅ x' : _ | _ | VA]< wl >)
+    (VΓext : [||-v (Γ ,, A) ,, tId A⟨@wk1 Γ A⟩ x⟨@wk1 Γ A⟩ (tRel 0)]< wl >)
+    (VP : [_ ||-v<l> P | VΓext]< wl >)
+    (VP' : [_ ||-v<l> P' | VΓext]< wl >)
+    (VPP' : [_ ||-v<l> P ≅ P' | _ | VP]< wl >) 
+    (Ry : W[  _ ||-< l > y : _ | RVA]< wl' >)
+    (Ry' : W[  _ ||-< l > y' : _ | RVA]< wl' >)
+    (Ryy' : W[  _ ||-< l > y ≅ y' : _ | RVA]< wl' >)
+    (RId : W[Δ ||-<l> tId A[σ] x[σ] y]< wl' >)
+    (RId' : W[Δ ||-<l> tId A[σ] x[σ] y']< wl' >)
+    (Re : W[ _ ||-< l > e : _ | RId]< wl' >)
+    (Re' : W[ _ ||-< l > e' : _ | RId']< wl' >)
+    (Ree' : W[ _ ||-< l > e ≅ e' : _ | RId]< wl' >)
+    (RPsubst : W[Δ ||-<l> P[up_term_term (up_term_term σ)][e .: y ..]]< wl' >) :
+    W[ Δ ||-< l > P[up_term_term (up_term_term σ)][e .: y ..] ≅ P'[up_term_term (up_term_term σ)][e' .: y' ..] | RPsubst]< wl' >.
   Proof.
-    pose (VΓA := validSnoc VΓ VA). 
-    eapply LRTransEq.
+    pose (VΓA := validSnoc' VΓ VA). 
+    eapply WLRTransEq.
     eapply substEq_idElimMotive_substupup.
     2,4,8: tea. all:tea.
-    irrelevance0; rewrite subst_upup_scons2; [reflexivity|].
-    unshelve eapply validTyEq; cycle 2; tea.
+    Wirrelevance0; rewrite subst_upup_scons2; [reflexivity|].
+    unshelve eapply validTyEq; cycle 4; tea.
     eapply irrelevanceSubst.
     unshelve eapply consSubstS.
     3: now eapply idElimMotiveCtxIdValid.
     1: now eapply consSubstS.
-    irrelevance.
+    Wirrelevance.
     Unshelve. 2: eapply subst_idElimMotive_substupup; cycle 1; tea.
   Qed.
 
 
-  Lemma substExtIdElimMotive {Γ l A x P y y' e e'}
-    (VΓ : [||-v Γ]) 
-    (VA : [_ ||-v<l> A | VΓ]) 
-    (Vx : [_ ||-v<l> x : _ | _ | VA])
-    (VΓext : [||-v (Γ ,, A) ,, tId A⟨@wk1 Γ A⟩ x⟨@wk1 Γ A⟩ (tRel 0)])
-    (VP : [_ ||-v<l> P | VΓext])
-    (Vy : [Γ ||-v<l> y : _ | _ | VA])
-    (Vy' : [Γ ||-v<l> y' : _ | _ | VA])
-    (Vyy' : [Γ ||-v<l> y ≅ y' : _ | _ | VA])
-    (VId : [Γ ||-v<l> tId A x y | VΓ])
-    (VId' : [Γ ||-v<l> tId A x y' | VΓ])
-    (Ve : [_ ||-v<l> e : _ | _ | VId]) 
-    (Ve' : [_ ||-v<l> e' : _ | _ | VId']) 
-    (Vee' : [_ ||-v<l> e ≅ e' : _ | _ | VId]) 
-    (VPey : [_ ||-v<l> P[e .: y ..] | VΓ]) : 
-    [_ ||-v<l> P[e .: y ..] ≅ P[e' .: y' ..] | VΓ | VPey].
+  Lemma substExtIdElimMotive {wl Γ l A x P y y' e e'}
+    (VΓ : [||-v Γ]< wl >) 
+    (VA : [_ ||-v<l> A | VΓ]< wl >) 
+    (Vx : [_ ||-v<l> x : _ | _ | VA]< wl >)
+    (VΓext : [||-v (Γ ,, A) ,, tId A⟨@wk1 Γ A⟩ x⟨@wk1 Γ A⟩ (tRel 0)]< wl >)
+    (VP : [_ ||-v<l> P | VΓext]< wl >)
+    (Vy : [Γ ||-v<l> y : _ | _ | VA]< wl >)
+    (Vy' : [Γ ||-v<l> y' : _ | _ | VA]< wl >)
+    (Vyy' : [Γ ||-v<l> y ≅ y' : _ | _ | VA]< wl >)
+    (VId : [Γ ||-v<l> tId A x y | VΓ]< wl >)
+    (VId' : [Γ ||-v<l> tId A x y' | VΓ]< wl >)
+    (Ve : [_ ||-v<l> e : _ | _ | VId]< wl >) 
+    (Ve' : [_ ||-v<l> e' : _ | _ | VId']< wl >) 
+    (Vee' : [_ ||-v<l> e ≅ e' : _ | _ | VId]< wl >) 
+    (VPey : [_ ||-v<l> P[e .: y ..] | VΓ]< wl >) : 
+    [_ ||-v<l> P[e .: y ..] ≅ P[e' .: y' ..] | VΓ | VPey]< wl >.
   Proof.
     constructor; intros.
-    irrelevance0; rewrite subst_scons2; [reflexivity|]. 
+    Wirrelevance0; rewrite subst_scons2; [reflexivity|]. 
     unshelve eapply validTyExt.
-    5,6: eapply idElimMotiveScons2Valid; cycle 1; tea.
+    7,8: eapply idElimMotiveScons2Valid; cycle 1; tea.
     1: tea.
     instValid Vσ; unshelve eapply consSubstSEq''.
     4: now eapply idElimMotiveCtxIdValid.
-    2: eapply consSubstSEq'; [now eapply reflSubst|]; irrelevance.
-    all: irrelevance.
-    Unshelve. 1:tea. irrelevance.
+    2: eapply consSubstSEq'; [now eapply reflSubst|]; Wirrelevance.
+    all: Wirrelevance.
+    Unshelve. 1:tea. Wirrelevance.
   Qed.
 
-  Lemma substEqIdElimMotive {Γ l A A' x x' P P' y y' e e'}
-    (VΓ : [||-v Γ]) 
-    (VA : [_ ||-v<l> A | VΓ]) 
-    (VA' : [_ ||-v<l> A' | VΓ]) 
-    (VAA' : [_ ||-v<l> A ≅ A' | VΓ | VA]) 
-    (Vx : [_ ||-v<l> x : _ | _ | VA])
-    (Vx' : [_ ||-v<l> x' : _ | _ | VA])
-    (Vxx' : [_ ||-v<l> x ≅ x' : _ | _ | VA])
-    (VΓext : [||-v (Γ ,, A) ,, tId A⟨@wk1 Γ A⟩ x⟨@wk1 Γ A⟩ (tRel 0)])
-    (VP : [_ ||-v<l> P | VΓext])
-    (VP' : [_ ||-v<l> P | VΓext])
-    (VPP' : [_ ||-v<l> P ≅ P' | _ | VP])
-    (Vy : [Γ ||-v<l> y : _ | _ | VA])
-    (Vy' : [Γ ||-v<l> y' : _ | _ | VA])
-    (Vyy' : [Γ ||-v<l> y ≅ y' : _ | _ | VA])
-    (VId : [Γ ||-v<l> tId A x y | VΓ])
-    (Ve : [_ ||-v<l> e : _ | _ | VId]) 
-    (Ve' : [_ ||-v<l> e' : _ | _ | VId]) 
-    (Vee' : [_ ||-v<l> e ≅ e' : _ | _ | VId]) 
-    (VPey : [_ ||-v<l> P[e .: y ..] | VΓ]) : 
-    [_ ||-v<l> P[e .: y ..] ≅ P'[e' .: y' ..] | VΓ | VPey].
+  Lemma substEqIdElimMotive {wl Γ l A A' x x' P P' y y' e e'}
+    (VΓ : [||-v Γ]< wl >) 
+    (VA : [_ ||-v<l> A | VΓ]< wl >) 
+    (VA' : [_ ||-v<l> A' | VΓ]< wl >) 
+    (VAA' : [_ ||-v<l> A ≅ A' | VΓ | VA]< wl >) 
+    (Vx : [_ ||-v<l> x : _ | _ | VA]< wl >)
+    (Vx' : [_ ||-v<l> x' : _ | _ | VA]< wl >)
+    (Vxx' : [_ ||-v<l> x ≅ x' : _ | _ | VA]< wl >)
+    (VΓext : [||-v (Γ ,, A) ,, tId A⟨@wk1 Γ A⟩ x⟨@wk1 Γ A⟩ (tRel 0)]< wl >)
+    (VP : [_ ||-v<l> P | VΓext]< wl >)
+    (VP' : [_ ||-v<l> P | VΓext]< wl >)
+    (VPP' : [_ ||-v<l> P ≅ P' | _ | VP]< wl >)
+    (Vy : [Γ ||-v<l> y : _ | _ | VA]< wl >)
+    (Vy' : [Γ ||-v<l> y' : _ | _ | VA]< wl >)
+    (Vyy' : [Γ ||-v<l> y ≅ y' : _ | _ | VA]< wl >)
+    (VId : [Γ ||-v<l> tId A x y | VΓ]< wl >)
+    (Ve : [_ ||-v<l> e : _ | _ | VId]< wl >) 
+    (Ve' : [_ ||-v<l> e' : _ | _ | VId]< wl >) 
+    (Vee' : [_ ||-v<l> e ≅ e' : _ | _ | VId]< wl >) 
+    (VPey : [_ ||-v<l> P[e .: y ..] | VΓ]< wl >) : 
+    [_ ||-v<l> P[e .: y ..] ≅ P'[e' .: y' ..] | VΓ | VPey]< wl >.
   Proof.
-    assert (VId' : [Γ ||-v<l> tId A x y' | VΓ]) by now eapply IdValid.
-    assert [Γ ||-v< l > e' : tId A x y' | VΓ | VId'].
+    assert (VId' : [Γ ||-v<l> tId A x y' | VΓ]< wl >) by now eapply IdValid.
+    assert [Γ ||-v< l > e' : tId A x y' | VΓ | VId']< wl >.
     1:{
       eapply conv; tea.
       eapply IdCongValid; tea.
@@ -551,13 +550,13 @@ Context `{GenericTypingProperties}.
     - eapply substExtIdElimMotive.
       2: tea. all: tea.
       Unshelve. eapply substIdElimMotive; cycle 1; tea.
-    - constructor; intros; irrelevance0; rewrite subst_scons2; [reflexivity|].
+    - constructor; intros; Wirrelevance0; rewrite subst_scons2; [reflexivity|].
       unshelve eapply validTyEq.
-      6: tea. 1: tea.
+      8: tea. 1,2: tea.
       eapply idElimMotiveScons2Valid; tea.
   Qed.
     
-  (* Lemma liftSubstS' {Γ σ Δ lF F} 
+  (* Lemma liftSubstS' {wl Γ σ Δ lF F} 
     {VΓ : [||-v Γ]} 
     {wfΔ : [|- Δ]}
     (VF : [Γ ||-v<lF> F | VΓ])
@@ -571,88 +570,179 @@ Context `{GenericTypingProperties}.
   Qed. *)
 
 
-  Lemma IdElimValid {Γ l A x P hr y e}
-    (VΓ : [||-v Γ]) 
-    (VA : [_ ||-v<l> A | VΓ]) 
-    (Vx : [_ ||-v<l> x : _ | _ | VA])
-    (VΓext : [||-v (Γ ,, A) ,, tId A⟨@wk1 Γ A⟩ x⟨@wk1 Γ A⟩ (tRel 0)])
-    (VP : [_ ||-v<l> P | VΓext])
+  Lemma IdElimValid {wl Γ l A x P hr y e}
+    (VΓ : [||-v Γ]< wl >) 
+    (VA : [_ ||-v<l> A | VΓ]< wl >) 
+    (Vx : [_ ||-v<l> x : _ | _ | VA]< wl >)
+    (VΓext : [||-v (Γ ,, A) ,, tId A⟨@wk1 Γ A⟩ x⟨@wk1 Γ A⟩ (tRel 0)]< wl >)
+    (VP : [_ ||-v<l> P | VΓext]< wl >)
     (VPhr := substIdElimMotive VΓ VA Vx VΓext VP Vx (IdValid VΓ VA Vx Vx) (reflValid VΓ VA Vx _))
-    (Vhr : [_ ||-v<l> hr : _ | _ | VPhr ])
-    (Vy : [_ ||-v<l> y : _ | _ | VA]) 
-    (VId : [Γ ||-v<l> tId A x y | VΓ])
-    (Ve : [_ ||-v<l> e : _ | _ | VId])
+    (Vhr : [_ ||-v<l> hr : _ | _ | VPhr ]< wl >)
+    (Vy : [_ ||-v<l> y : _ | _ | VA]< wl >) 
+    (VId : [Γ ||-v<l> tId A x y | VΓ]< wl >)
+    (Ve : [_ ||-v<l> e : _ | _ | VId]< wl >)
     (VPye := substIdElimMotive VΓ VA Vx VΓext VP Vy VId Ve) :
-    [_ ||-v<l> tIdElim A x P hr y e : _ | _ | VPye].
+    [_ ||-v<l> tIdElim A x P hr y e : _ | _ | VPye]< wl >.
   Proof.
-    unshelve epose (h := _ : [||-v Γ,, A]). 1: now eapply validSnoc.
+    unshelve epose (h := _ : [||-v Γ,, A]< wl >). 1: now eapply validSnoc'.
     constructor; intros.
     - instValid Vσ.
-      irrelevance0.
-      2: unshelve eapply idElimRed; refold; tea.
-      1: refold; now rewrite subst_upup_scons2, subst_scons2.
-      2,5: irrelevance.
-      + intros; eapply subst_idElimMotive_substupup; cycle 1; tea.
-      + now eapply red_idElimMotive_substupup.
-      + intros; eapply substEq_idElimMotive_substupup; cycle 1; tea.
-        eapply LRTmRedConv; tea; now eapply LRTyEqSym.
+      eapply (TreeTmSplit (DTree_fusion _ _ _)).
+      intros wl'' Ho HA.
+      pose (f':= over_tree_le Ho).
+      pose (RIAxy := (WRed (tId A x y)[σ] RVId wl'' (over_tree_fusion_l Ho))).
+      assert (Re: [Δ ||-< l > e[σ] : (tId A x y)[σ] | LRId' (invLRId RIAxy)]< wl'' >).
+      { enough [Δ ||-< l > e[σ] : (tId A x y)[σ] | LRId' (invLRId RIAxy) ]< wl'' > by eauto.
+        refold.
+        irrelevanceRefl ; unshelve eapply RVe.
+        1: now eapply over_tree_fusion_l.
+        now eapply over_tree_fusion_r ; exact Ho.
+      }
+      pose proof (IdRedTy_inv (invLRId RIAxy)) as [eA ex ey] ; refold.
+      pose proof (hred := Re.(IdRedTm.red)); unfold_id_outTy; rewrite <-eA,<-ex,<-ey in hred.
+      unshelve epose proof (Hyp := red_idElimMotive_substupup _ _ _ _ _ _ _).
+      13,17: tea.
+      2: tea.
+      enough (X : W[ Δ ||-< l > tIdElim A[σ] x[σ] P[up_term_term (up_term_term σ)] hr[σ] y[σ] (IdRedTm.nf Re) : P[e .: y..][σ] | HA ]< wl'' >).
+      { cbn in * ; eapply WredSubstTerm.
+        1: exact X.
+        escape ; Wescape.
+        destruct hred.
+        rewrite subst_scons2, <-subst_upup_scons2.
+        eapply redtm_idElim ; tea.
+        1,3: now eapply wft_Ltrans.
+        1,3: now eapply ty_Ltrans.
+        rewrite subst_scons2 in RRVhr.
+        rewrite subst_upup_scons2 ; now eapply ty_Ltrans.
+      }
+      pose proof (redTmFwdConv Re hred (IdProp_whnf _ _ (IdRedTm.prop Re))) as [Rnf Rnfeq].
+      eapply WLRTmRedConv.
+      2: unshelve eapply WidElimPropRed ; refold; tea.
+      + eapply WLRTransEq.
+        1: eapply substEq_idElimMotive_substupup.  
+        6: now eapply TmLogtoW.
+        2: eassumption.
+        4: eapply WreflLRTmEq.
+        2,3,4,5 : eapply WTm_Ltrans' ; [ eassumption | eassumption].
+        1: eassumption.
+        1: now eapply WLRTmEqSym, TmEqLogtoW.
+        cbn ; Wirrelevance0 ; [ | now eapply WreflLRTyEq ] ; now bsimpl.
+      + now eapply WLtrans.
+      + intros.
+        eapply subst_idElimMotive_substupup ; cycle 1 ; tea.
+        cbn ; Wirrelevance0 ; [reflexivity | now eapply WTm_Ltrans].
+      + now eapply WTm_Ltrans'.
+      + now eapply WLtrans.
+      + now eapply TmLogtoW'.
+      + now eapply WTm_Ltrans'.
+      + eapply invLRId.
+        eapply RVId, over_tree_fusion_l ; exact Ho.
+      + unshelve eapply red_idElimMotive_substupup.
+        3: eassumption.
+        4: now eapply (Validity_Ltrans' f).
+        * now eapply wfc_Ltrans.
+        * now eapply WfC_Ltrans.
+        * eapply subst_Ltrans', subst_Ltrans ; eassumption.
+        * now eapply TmValidity_Ltrans.
+        * now eapply Validity_Ltrans'.
+      + intros ; cbn in *.
+        eapply substEq_idElimMotive_substupup ; cycle 1; tea.
+        1,3: Wirrelevance.
+        eapply WLRTmRedConv; tea; now eapply WLRTyEqSym.
+      + cbn ; Wirrelevance0 ; [ | now eapply WTm_Ltrans].
+        now bsimpl.
+      + exact (IdRedTm.prop Re).
+        Unshelve.
+        2: rewrite subst_upup_scons2, <- subst_scons2 ; now eapply WLtrans.
+        all: try now eapply wfc_Ltrans + now eapply wfLCon_le_id.
+        all: tea; try now eapply wfLCon_le_trans.
+        1,3,4: now eapply subst_Ltrans.
+        now eapply WLtrans.
     - instAllValid Vσ Vσ' Vσσ'.
-      irrelevance0.
-      2: unshelve eapply idElimCongRed; refold.
+      Wirrelevance0.
+      2: unshelve eapply WidElimCongRed; refold.
       1: refold; now rewrite subst_upup_scons2, subst_scons2.
-      all: try now eapply LRCumulative.
-      all: tea; try irrelevanceCum.
+      all: try now eapply WLRCumulative.
+      all: tea; try now eapply WLRTmRedIrrelevantCum'.
+      all: tea; try now eapply WLRTmEqIrrelevantCum'.
+      all: tea; try now eapply WLRTyEqIrrelevantCum'.
       2,4: now eapply red_idElimMotive_substupup.
-      + intros; eapply subst_idElimMotive_substupup; cycle 1; tea; irrelevanceCum.
-        Unshelve. all: tea. irrelevanceCum.
-      + intros; eapply subst_idElimMotive_substupup; cycle 1; tea; irrelevanceCum.
-        Unshelve. all: tea.
+      + intros wl'' f' ** ; eapply subst_idElimMotive_substupup; cycle 1; tea.
+        all: now eapply WLRTmRedIrrelevantCum'.
+        Unshelve.
+        * now eapply wfLCon_le_trans.
+        * now eapply wfc_Ltrans.
+        * now eapply subst_Ltrans.
+        * now eapply WLRCumulative.
+      + intros wl'' f' **; eapply subst_idElimMotive_substupup; cycle 1; tea.
+        all: now eapply WLRTmRedIrrelevantCum'.
+        Unshelve.
+        * now eapply wfLCon_le_trans.
+        * now eapply wfc_Ltrans.
+        * now eapply subst_Ltrans.
+        * now eapply WLRCumulative.
       + now eapply red_idElimMotive_substupup_cong.
-      + intros; eapply substEq_idElimMotive_substupupEq; cycle 2; tea; irrelevanceCum.
-        Unshelve. all: tea. now eapply LRCumulative.
-      + intros; eapply substEq_idElimMotive_substupup; cycle 1; tea.
-        1,3-6: irrelevanceCum.
-        eapply LRTmRedConv;[|irrelevanceCum]; eapply LRTyEqSym; irrelevanceCum.
-        Unshelve. all: tea; now eapply LRCumulative.
-      + Set Printing Primitive Projection Parameters.
-        intros; eapply substEq_idElimMotive_substupup; cycle 1; tea.
-        1,3: irrelevanceCum.
-        eapply LRTmRedConv; [|irrelevanceCum]; eapply LRTyEqSym; irrelevanceCum.
-        Unshelve. all: tea.
+      + intros wl'' f' **; eapply substEq_idElimMotive_substupupEq; cycle 2; tea.
+        all: try now eapply WLRTmRedIrrelevantCum' + now eapply WLRTmEqIrrelevantCum'.
+        now eapply eqsubst_Ltrans.
+        Unshelve. 3,4: now eapply WLRCumulative.
+        3: assumption.
+        * now eapply wfc_Ltrans.
+        * now eapply subst_Ltrans.
+      + cbn. intros wl'' f' **.
+        eapply substEq_idElimMotive_substupup; cycle 1.
+        1: eassumption.
+        all: try now eapply WLRTmRedIrrelevantCum' + now eapply WLRTmEqIrrelevantCum'.
+        2: eassumption.
+        eapply WLRTmRedConv ; [ now eapply WLRTyEqSym, WLRTyEqIrrelevantCum' | ].
+        now eapply WLRTmRedIrrelevantCum'.
+    +  Set Printing Primitive Projection Parameters.
+       intros; eapply substEq_idElimMotive_substupup; cycle 1; tea.
+       all: try now eapply WLRTmRedIrrelevantCum'.
+       all: try now eapply WLRTmEqIrrelevantCum'.
+       eapply WLRTmRedConv; [| now eapply WLRTmRedIrrelevantCum'].
+       eapply WLRTyEqSym ; now eapply WLRTyEqIrrelevantCum'.
+    + cbn ; Wirrelevance0 ; [ | eassumption] ; now rewrite subst_upup_scons2, subst_scons2.
+    + cbn ; Wirrelevance0 ; [ | eassumption] ; now rewrite subst_upup_scons2, subst_scons2.
+    + cbn ; Wirrelevance0 ; [ | eassumption] ; now rewrite subst_upup_scons2, subst_scons2.
+      Unshelve. all: tea.
+      all: try now eapply wfc_Ltrans + now eapply wfLCon_le_trans.
+      all: try now eapply WLtrans + now eapply subst_Ltrans.
+      all: try now eapply WLRCumulative.
   Qed.
 
-  Lemma IdElimCongValid {Γ l A A' x x' P P' hr hr' y y' e e'}
-    (VΓ : [||-v Γ]) 
-    (VA : [_ ||-v<l> A | VΓ]) 
-    (VA' : [_ ||-v<l> A' | VΓ]) 
-    (VAA' : [_ ||-v<l> A ≅ A' | _ | VA])
-    (Vx : [_ ||-v<l> x : _ | _ | VA])
-    (Vx' : [_ ||-v<l> x' : _ | _ | VA])
-    (Vxx' : [_ ||-v<l> x ≅ x' : _ | _ | VA])
-    (VΓext : [||-v (Γ ,, A) ,, tId A⟨@wk1 Γ A⟩ x⟨@wk1 Γ A⟩ (tRel 0)])
-    (VP : [_ ||-v<l> P | VΓext])
-    (VP' : [_ ||-v<l> P' | VΓext])
-    (VPP' : [_ ||-v<l> P ≅ P' | _ | VP])
+  Lemma IdElimCongValid {wl Γ l A A' x x' P P' hr hr' y y' e e'}
+    (VΓ : [||-v Γ]< wl >) 
+    (VA : [_ ||-v<l> A | VΓ]< wl >) 
+    (VA' : [_ ||-v<l> A' | VΓ]< wl >) 
+    (VAA' : [_ ||-v<l> A ≅ A' | _ | VA]< wl >)
+    (Vx : [_ ||-v<l> x : _ | _ | VA]< wl >)
+    (Vx' : [_ ||-v<l> x' : _ | _ | VA]< wl >)
+    (Vxx' : [_ ||-v<l> x ≅ x' : _ | _ | VA]< wl >)
+    (VΓext : [||-v (Γ ,, A) ,, tId A⟨@wk1 Γ A⟩ x⟨@wk1 Γ A⟩ (tRel 0)]< wl >)
+    (VP : [_ ||-v<l> P | VΓext]< wl >)
+    (VP' : [_ ||-v<l> P' | VΓext]< wl >)
+    (VPP' : [_ ||-v<l> P ≅ P' | _ | VP]< wl >)
     (VPhr := substIdElimMotive VΓ VA Vx VΓext VP Vx (IdValid VΓ VA Vx Vx) (reflValid VΓ VA Vx _))
-    (Vhr : [_ ||-v<l> hr : _ | _ | VPhr ])
-    (Vhr' : [_ ||-v<l> hr' : _ | _ | VPhr ])
-    (Vhrhr' : [_ ||-v<l> hr ≅ hr' : _ | _ | VPhr])
-    (Vy : [_ ||-v<l> y : _ | _ | VA]) 
-    (Vy' : [_ ||-v<l> y' : _ | _ | VA]) 
-    (Vyy' : [_ ||-v<l> y ≅ y' : _ | _ | VA]) 
-    (VId : [Γ ||-v<l> tId A x y | VΓ])
-    (Ve : [_ ||-v<l> e : _ | _ | VId])
-    (Ve' : [_ ||-v<l> e' : _ | _ | VId])
-    (Vee' : [_ ||-v<l> e ≅ e' : _ | _ | VId])
+    (Vhr : [_ ||-v<l> hr : _ | _ | VPhr ]< wl >)
+    (Vhr' : [_ ||-v<l> hr' : _ | _ | VPhr ]< wl >)
+    (Vhrhr' : [_ ||-v<l> hr ≅ hr' : _ | _ | VPhr]< wl >)
+    (Vy : [_ ||-v<l> y : _ | _ | VA]< wl >) 
+    (Vy' : [_ ||-v<l> y' : _ | _ | VA]< wl >) 
+    (Vyy' : [_ ||-v<l> y ≅ y' : _ | _ | VA]< wl >) 
+    (VId : [Γ ||-v<l> tId A x y | VΓ]< wl >)
+    (Ve : [_ ||-v<l> e : _ | _ | VId]< wl >)
+    (Ve' : [_ ||-v<l> e' : _ | _ | VId]< wl >)
+    (Vee' : [_ ||-v<l> e ≅ e' : _ | _ | VId]< wl >)
     (VPye := substIdElimMotive VΓ VA Vx VΓext VP Vy VId Ve) :
-    [_ ||-v<l> tIdElim A x P hr y e ≅ tIdElim A' x' P' hr' y' e' : _ | _ | VPye].
+    [_ ||-v<l> tIdElim A x P hr y e ≅ tIdElim A' x' P' hr' y' e' : _ | _ | VPye]< wl >.
   Proof.
-    assert [_ ||-v<l> x' : _ | _ | VA'] by now eapply conv.
-    assert [_ ||-v<l> y' : _ | _ | VA'] by now eapply conv.
-    assert (VΓext' : [||-v (Γ ,, A'),, tId A'⟨@wk1 Γ A'⟩ x'⟨@wk1 Γ A'⟩ (tRel 0)]).
-    1: eapply validSnoc; now eapply idElimMotiveCtxIdValid.
+    assert [_ ||-v<l> x' : _ | _ | VA']< wl > by now eapply conv.
+    assert [_ ||-v<l> y' : _ | _ | VA']< wl > by now eapply conv.
+    assert (VΓext' : [||-v (Γ ,, A'),, tId A'⟨@wk1 Γ A'⟩ x'⟨@wk1 Γ A'⟩ (tRel 0)]< wl >).
+    1: eapply validSnoc'; now eapply idElimMotiveCtxIdValid.
     assert (h : forall t, t⟨@wk1 Γ A'⟩ = t⟨@wk1 Γ A⟩) by reflexivity.
-    assert (VPalt' : [_ ||-v<l> P' | VΓext']).
+    assert (VPalt' : [_ ||-v<l> P' | VΓext']< wl >).
     1:{
       eapply convCtx2'; tea.
       1: eapply convCtx1; tea; [now eapply symValidTyEq| ].
@@ -662,34 +752,70 @@ Context `{GenericTypingProperties}.
     }
     constructor; intros.
     instValid Vσ.
-    irrelevance0.
-    2: unshelve eapply idElimCongRed; refold.
+    Wirrelevance0.
+    2: unshelve eapply WidElimCongRed; refold.
     1: refold; now rewrite subst_upup_scons2, subst_scons2.
-    all: first [now eapply LRCumulative | solve [irrelevance | irrelevanceCum] | now eapply LRTmRedConv | tea].
-    + intros ; eapply subst_idElimMotive_substupup; cycle 1; tea; irrelevanceCum.
-      Unshelve. all: tea. irrelevanceCum.
-    + intros; eapply red_idElimMotive_substupup; tea.
-    + intros; eapply subst_idElimMotive_substupup; cycle 1; tea.
-      irrelevance.
+    all: first [now eapply WLRCumulative | solve [Wirrelevance | WirrelevanceCum] | now eapply WLRTmRedConv | tea].
+
+    + intros ; eapply subst_idElimMotive_substupup; cycle 1; tea; WirrelevanceCum.
       Unshelve. all: tea.
-    + unshelve eapply IdRed; tea; eapply LRTmRedConv; tea.
+      * now eapply wfLCon_le_trans.
+      * now eapply wfc_Ltrans.
+      * now eapply subst_Ltrans.
+      * WirrelevanceCum.
+    + eapply WLRTmRedConv; [ | now WirrelevanceCum].
+      WirrelevanceCum.
+    + eapply red_idElimMotive_substupup ; tea.
+    + intros; eapply subst_idElimMotive_substupup; cycle 1; tea.
+      1,2: WirrelevanceCum.
+      Unshelve. all: tea.
+      1,5: WirrelevanceCum.
+      * now eapply wfLCon_le_trans.
+      * now eapply wfc_Ltrans.
+      * now eapply subst_Ltrans.
+    + unshelve eapply WIdRed; tea.
+      1,2: now WirrelevanceCum0.
+      eapply WLRTmRedConv; now WirrelevanceCum0.
     + eapply red_idElimMotive_substupup; tea.
     + eapply redEq_idElimMotive_substupup.
       6-8: tea. 3-5: tea. all: tea.
-    + intros.
-      assert [_ ||-<l> y'0 : _ | RVA] by (eapply LRTmRedConv; tea; now eapply LRTyEqSym).
+    + intros wl'' f' **.
+      assert W[_ ||-<l> y'0 : _ | (WLtrans f' RVA)]< wl'' >.
+      { eapply WLRTmRedConv; tea ; [ eapply WLRTyEqSym | ].
+        2: now WirrelevanceCum0.
+        now eapply WEq_Ltrans.
+      }
       eapply substExt_idElimMotive_substupup.
-      7: tea. 2,3,5,6: tea. all: tea; try solve [irrelevanceCum].
-      1: eapply LRTmRedConv; tea; eapply LRTyEqSym; tea.
-      eapply IdCongRed; tea; [now escape|  now eapply reflLRTmEq].
-      Unshelve. 1: now eapply LRCumulative. 1,2: now eapply IdRed.
-    + intros; eapply substEq_idElimMotive_substupup; cycle 1; tea; try solve [irrelevanceCum].
-      eapply LRTmRedConv. 2:irrelevanceCum. eapply LRTyEqSym; irrelevanceCum.
-      Unshelve. all: tea; now eapply LRCumulative.
-    + intros; eapply substEq_idElimMotive_substupup; cycle 1; tea; try solve [irrelevanceCum].
-      eapply LRTmRedConv. 2:irrelevanceCum. eapply LRTyEqSym; irrelevanceCum.
-      Unshelve. all: tea; now eapply LRCumulative.
-    + eapply LRTmRedConv; tea.
+      7: tea. 2,3,5,6: tea. all: tea; try solve [WirrelevanceCum].
+      1: eapply WLRTmRedConv; tea; [ eapply WLRTyEqSym | ] ; tea.
+      2: now WirrelevanceCum0.
+      eapply WIdCongRed; tea; [now Wescape|.. | now eapply WreflLRTmEq].
+      1: now eapply WEq_Ltrans.
+      now eapply WTmEq_Ltrans.
+      Unshelve. 2: now eapply WLRCumulative.
+      all: try now eapply WLtrans + now WirrelevanceCum0 + tea.
+      1: now eapply wfLCon_le_trans.
+      1: now eapply wfc_Ltrans.
+      1: now eapply subst_Ltrans.
+      1,2: eapply WIdRed ; eauto.
+      all: now eapply WTm_Ltrans.
+    + intros; eapply substEq_idElimMotive_substupup; cycle 1; tea;
+        try solve [WirrelevanceCum].
+      eapply WLRTmRedConv. 2:WirrelevanceCum.
+      eapply WLRTyEqSym; WirrelevanceCum.
+      Unshelve. all: tea ; try now eapply WLRCumulative.
+      1: now eapply wfLCon_le_trans.
+      1: now eapply wfc_Ltrans.
+      1: now eapply subst_Ltrans.
+    + intros; eapply substEq_idElimMotive_substupup; cycle 1; tea;
+        try solve [WirrelevanceCum].
+      eapply WLRTmRedConv. 2:WirrelevanceCum.
+      eapply WLRTyEqSym; WirrelevanceCum.
+      Unshelve. all: tea; try now eapply WLRCumulative.
+      1: now eapply wfLCon_le_trans.
+      1: now eapply wfc_Ltrans.
+      1: now eapply subst_Ltrans.
+    + eapply WLRTmRedConv; tea.
       rewrite subst_upup_scons2; change (tRefl A'[σ] x'[σ]) with (tRefl A' x')[σ].
       rewrite <- subst_scons2.
       eapply validTyEq. eapply substEqIdElimMotive.
@@ -699,32 +825,40 @@ Context `{GenericTypingProperties}.
       1: eapply symValidTyEq; now eapply IdCongValid.
       now eapply reflCongValid.
       Unshelve. all: now eapply IdValid.
-    + eapply LRTmRedConv; tea.
-      now eapply IdCongValid.
+    + eapply WLRTmRedConv; tea.
+      2: now WirrelevanceCum0.
+      now WirrelevanceCum.
+    + eapply WLRTmRedConv; tea.
+      2: now WirrelevanceCum0.
+      1: WirrelevanceCum0 ; [reflexivity | ].
+      now eapply IdCongValid ; tea.
+      Unshelve.
+      all: tea.
+      1,2: now WirrelevanceCum0.
   Qed.
 
 
-  Lemma IdElimReflValid {Γ l A x P hr y B z}
-    (VΓ : [||-v Γ]) 
-    (VA : [_ ||-v<l> A | VΓ]) 
-    (Vx : [_ ||-v<l> x : _ | _ | VA])
-    (VΓext : [||-v (Γ ,, A) ,, tId A⟨@wk1 Γ A⟩ x⟨@wk1 Γ A⟩ (tRel 0)])
-    (VP : [_ ||-v<l> P | VΓext])
+  Lemma IdElimReflValid {wl Γ l A x P hr y B z}
+    (VΓ : [||-v Γ]< wl >) 
+    (VA : [_ ||-v<l> A | VΓ]< wl >) 
+    (Vx : [_ ||-v<l> x : _ | _ | VA]< wl >)
+    (VΓext : [||-v (Γ ,, A) ,, tId A⟨@wk1 Γ A⟩ x⟨@wk1 Γ A⟩ (tRel 0)]< wl >)
+    (VP : [_ ||-v<l> P | VΓext]< wl >)
     (VPhr := substIdElimMotive VΓ VA Vx VΓext VP Vx (IdValid VΓ VA Vx Vx) (reflValid VΓ VA Vx _))
-    (Vhr : [_ ||-v<l> hr : _ | _ | VPhr ])
-    (Vy : [_ ||-v<l> y : _ | _ | VA]) 
-    (Vxy : [_ ||-v<l> x ≅ y : _ | _ | VA]) 
-    (VB : [_ ||-v<l> B | VΓ])
-    (VAB : [_ ||-v<l> _ ≅ B | VΓ | VA])
-    (Vz : [_ ||-v<l> z : _ | _ | VB]) 
-    (Vxz : [_ ||-v<l> x ≅ z : _ | _ | VA]) 
-    (VId : [Γ ||-v<l> tId A x y | VΓ]) 
-    (VRefl : [_ ||-v<l> tRefl B z : _ | _ | VId])
+    (Vhr : [_ ||-v<l> hr : _ | _ | VPhr ]< wl >)
+    (Vy : [_ ||-v<l> y : _ | _ | VA]< wl >) 
+    (Vxy : [_ ||-v<l> x ≅ y : _ | _ | VA]< wl >) 
+    (VB : [_ ||-v<l> B | VΓ]< wl >)
+    (VAB : [_ ||-v<l> _ ≅ B | VΓ | VA]< wl >)
+    (Vz : [_ ||-v<l> z : _ | _ | VB]< wl >) 
+    (Vxz : [_ ||-v<l> x ≅ z : _ | _ | VA]< wl >) 
+    (VId : [Γ ||-v<l> tId A x y | VΓ]< wl >) 
+    (VRefl : [_ ||-v<l> tRefl B z : _ | _ | VId]< wl >)
     (VPye := substIdElimMotive VΓ VA Vx VΓext VP Vy VId VRefl) :
-    [_ ||-v<l> tIdElim A x P hr y (tRefl B z) ≅ hr : _ | _ | VPye].
+    [_ ||-v<l> tIdElim A x P hr y (tRefl B z) ≅ hr : _ | _ | VPye]< wl >.
   Proof.
     constructor; intros.
-    assert [Γ ||-v< l > P[tRefl A x .: x..] ≅ P[tRefl B z .: y..] | VΓ | VPhr].
+    assert [Γ ||-v< l > P[tRefl A x .: x..] ≅ P[tRefl B z .: y..] | VΓ | VPhr]< wl >.
     1:{
       eapply substExtIdElimMotive; cycle 1; tea.
       1: now eapply reflValid.
@@ -736,12 +870,12 @@ Context `{GenericTypingProperties}.
     eapply redwfSubstValid; cycle 1.
     + eapply conv; tea.
     + constructor; intros.
-      instValid Vσ0; escape.
+      instValid Vσ0; Wescape.
       constructor.
-      - eapply ty_conv; tea.
+      - eapply ty_conv; now tea.
       - rewrite subst_scons2, <- subst_upup_scons2.
         eapply redtm_idElimRefl; refold; tea.
-        * eapply escape. now eapply red_idElimMotive_substupup.
+        * eapply Wescape. now eapply red_idElimMotive_substupup.
         * rewrite subst_upup_scons2; change (tRefl ?A[?σ] ?x[_]) with (tRefl A x)[σ].
           now rewrite <- subst_scons2.
         * now eapply ty_conv.
