theories/Substitution/Split.v
@@ -1,0 +1,360 @@
+From LogRel.AutoSubst Require Import core unscoped Ast Extra.
+From LogRel Require Import Utils BasicAst Notations LContexts Context NormalForms Weakening GenericTyping Monad LogicalRelation Validity.
+From LogRel.LogicalRelation Require Import Induction Irrelevance Reflexivity Transitivity Monotonicity Split.
+From LogRel.Substitution Require Import Irrelevance Properties Monotonicity.
+
+
+Set Universe Polymorphism.
+
+Section Split.
+Context `{GenericTypingProperties}.
+
+Lemma validTySplit {wl : wfLCon} {Γ l A} {n : nat} {ne : not_in_LCon wl n}
+  {VΓt : [||-v Γ ]< (wl ,,l (ne, true)) >}
+  {VΓf : [||-v Γ ]< (wl ,,l (ne, false)) >}
+  {VΓ : [||-v Γ]< wl >} :
+  [Γ ||-v<l> A | VΓt]< wl ,,l (ne, true) > ->
+  [Γ ||-v<l> A | VΓf]< wl ,,l (ne, false) > ->
+  [Γ ||-v<l> A | VΓ]< wl >.
+Proof.
+  intros [VAt VAextt] [VAf VAextf].
+  unshelve econstructor.
+  - intros ??????.
+    destruct (decidInLCon wl' n) as [ i | i | notin].
+    + pose (f' := LCon_le_in_LCon (ne := ne) f i).
+      pose (f'':= @LCon_le_step wl wl n true ne (wfLCon_le_id _)).
+      unshelve eapply VAt ; tea.
+      change f with (f' •ε f'') in vσ.
+      eapply subst_Ltrans' in vσ.
+      unshelve eapply irrelevanceSubst.
+      * exists (VPack_Ltrans f'' VΓ).
+        now eapply  WfC_Ltrans.
+      * assumption.
+      * exact vσ.
+    + pose (f' := LCon_le_in_LCon (ne := ne) f i).
+      pose (f'':= @LCon_le_step wl wl n false ne (wfLCon_le_id _)).
+      unshelve eapply VAf ; tea.
+      change f with (f' •ε f'') in vσ.
+      eapply subst_Ltrans' in vσ.
+      unshelve eapply irrelevanceSubst.
+      * exists (VPack_Ltrans f'' VΓ).
+        now eapply  WfC_Ltrans.
+      * assumption.
+      * exact vσ.
+    + unshelve eapply Split.
+      2: exact notin.
+      * pose (i := @in_here_l wl' n true).
+        pose (f' := @LCon_le_up wl wl' n true ne notin f). 
+        pose (f'':= @LCon_le_step wl wl n true ne (wfLCon_le_id _)).
+        pose (f''':= @LCon_le_step wl' wl' n true notin (wfLCon_le_id _)).
+        unshelve eapply VAt ; tea.
+        2: unshelve epose proof (X:= subst_Ltrans f''' _ vσ).
+        1,2: now eapply wfc_Ltrans.
+        change (f''' •ε f)  with (f' •ε f'') in X.
+        eapply subst_Ltrans' in vσ.
+        unshelve eapply irrelevanceSubst.
+        -- exists (VPack_Ltrans f'' VΓ).
+           now eapply  WfC_Ltrans.
+        -- now eapply wfc_Ltrans.
+        -- assumption.
+      * pose (i := @in_here_l wl' n false).
+        pose (f' := @LCon_le_up wl wl' n false ne notin f). 
+        pose (f'':= @LCon_le_step wl wl n false ne (wfLCon_le_id _)).
+        pose (f''':= @LCon_le_step wl' wl' n false notin (wfLCon_le_id _)).
+        unshelve eapply VAf ; tea.
+        2: unshelve epose proof (X:= subst_Ltrans f''' _ vσ).
+        1,2: now eapply wfc_Ltrans.
+        change (f''' •ε f)  with (f' •ε f'') in X.
+        eapply subst_Ltrans' in vσ.
+        unshelve eapply irrelevanceSubst.
+        -- exists (VPack_Ltrans f'' VΓ).
+           now eapply  WfC_Ltrans.
+        -- now eapply wfc_Ltrans.
+        -- assumption.
+  - cbn.
+    intros.
+    destruct (decidInLCon wl' n) as [ i | i | notin] ; cbn in *.
+    + pose (f' := LCon_le_in_LCon (ne := ne) f i).
+      pose (f'':= @LCon_le_step wl wl n true ne (wfLCon_le_id _)).
+      unshelve eapply VAextt.
+      * change f with (f' •ε f'') in vσ'.
+        eapply subst_Ltrans' in vσ'.
+        unshelve eapply irrelevanceSubst ; [ | assumption | ]. 
+        1: now eapply  WfC_Ltrans.
+        exact vσ'.
+      * change f with (f' •ε f'') in vσσ'.
+        unshelve eapply eqsubst_Ltrans' in vσσ'.
+        unshelve eapply irrelevanceSubstEq ; [ | assumption | | ]. 
+        1: now eapply  WfC_Ltrans.
+        2: exact vσσ'.
+    + pose (f' := LCon_le_in_LCon (ne := ne) f i).
+      pose (f'':= @LCon_le_step wl wl n false ne (wfLCon_le_id _)).
+      unshelve eapply VAextf.
+      * change f with (f' •ε f'') in vσ'.
+        eapply subst_Ltrans' in vσ'.
+        unshelve eapply irrelevanceSubst ; [ | assumption | ]. 
+        1: now eapply WfC_Ltrans.
+        exact vσ'.
+      * change f with (f' •ε f'') in vσσ'.
+        unshelve eapply eqsubst_Ltrans' in vσσ'.
+        unshelve eapply irrelevanceSubstEq ; [ | assumption | | ]. 
+        1: now eapply  WfC_Ltrans.
+        2: exact vσσ'.
+    + unshelve eapply EqSplit.
+      * pose (i := @in_here_l wl' n true).
+        pose (f' := @LCon_le_up wl wl' n true ne notin f). 
+        pose (f'':= @LCon_le_step wl wl n true ne (wfLCon_le_id _)).
+        pose (f''':= @LCon_le_step wl' wl' n true notin (wfLCon_le_id _)).
+        unshelve eapply VAextt ; tea.
+        -- unshelve epose proof (X:= subst_Ltrans f''' _ vσ').
+           1: now eapply wfc_Ltrans.
+           change (f''' •ε f)  with (f' •ε f'') in X.
+           eapply subst_Ltrans' in X.
+           unshelve eapply irrelevanceSubst.
+           ++ exists (VPack_Ltrans f'' VΓ).
+              now eapply  WfC_Ltrans.
+           ++ now eapply wfc_Ltrans.
+           ++ assumption.
+        -- unshelve epose proof (X:= eqsubst_Ltrans f''' _ _ vσσ').
+           1: now eapply wfc_Ltrans.
+           change (f''' •ε f)  with (f' •ε f'') in X.
+           eapply eqsubst_Ltrans' in X.
+           unshelve eapply irrelevanceSubstEq.
+           1: cbn ; exists (VPack_Ltrans f'' VΓ) ; now eapply  WfC_Ltrans.
+           1:  now eapply wfc_Ltrans.
+           2: eassumption.
+      * pose (i := @in_here_l wl' n false).
+        pose (f' := @LCon_le_up wl wl' n false ne notin f). 
+        pose (f'':= @LCon_le_step wl wl n false ne (wfLCon_le_id _)).
+        pose (f''':= @LCon_le_step wl' wl' n false notin (wfLCon_le_id _)).
+        unshelve eapply VAextf ; tea.
+        -- unshelve epose proof (X:= subst_Ltrans f''' _ vσ').
+           1: now eapply wfc_Ltrans.
+           change (f''' •ε f)  with (f' •ε f'') in X.
+           eapply subst_Ltrans' in X.
+           unshelve eapply irrelevanceSubst.
+           ++ exists (VPack_Ltrans f'' VΓ).
+              now eapply  WfC_Ltrans.
+           ++ now eapply wfc_Ltrans.
+           ++ assumption.
+        -- unshelve epose proof (X:= eqsubst_Ltrans f''' _ _ vσσ').
+           1: now eapply wfc_Ltrans.
+           change (f''' •ε f)  with (f' •ε f'') in X.
+           eapply eqsubst_Ltrans' in X.
+           unshelve eapply irrelevanceSubstEq.
+           1: cbn ; exists (VPack_Ltrans f'' VΓ) ; now eapply  WfC_Ltrans.
+           1:  now eapply wfc_Ltrans.
+           2: eassumption.
+Defined.
+
+
+Lemma validEqTySplit {wl : wfLCon} {Γ l A B} {n : nat} {ne : not_in_LCon wl n}
+  {VΓt : [||-v Γ ]< (wl ,,l (ne, true)) >}
+  {VΓf : [||-v Γ ]< (wl ,,l (ne, false)) >}
+  {VΓ : [||-v Γ]< wl >}
+  {VAt : [Γ ||-v<l> A | VΓt]< wl ,,l (ne, true) >}
+  {VAf : [Γ ||-v<l> A | VΓf]< wl ,,l (ne, false) >} :
+  [Γ ||-v<l> A ≅ B | VΓt | VAt]< _ > ->
+  [Γ ||-v<l> A ≅ B | VΓf | VAf]< _ > ->
+  [Γ ||-v<l> A ≅ B | VΓ | validTySplit VAt VAf]< wl >.
+Proof.
+  intros [VBt] [VBf].
+  unshelve econstructor.
+  - intros ?????? ; cbn.
+    destruct (decidInLCon wl' n) as [ i | i | notin].
+    + now eapply VBt.
+    + now eapply VBf.
+    + eapply EqSplit.
+      * now eapply VBt.
+      * now eapply VBf.
+Qed.
+
+Lemma validEqTySplit' {wl : wfLCon} {Γ l A B} {n : nat} {ne : not_in_LCon wl n}
+  {VΓt : [||-v Γ ]< (wl ,,l (ne, true)) >}
+  {VΓf : [||-v Γ ]< (wl ,,l (ne, false)) >}
+  {VΓ : [||-v Γ]< wl >}
+  {VAt : [Γ ||-v<l> A | VΓt]< wl ,,l (ne, true) >}
+  {VAf : [Γ ||-v<l> A | VΓf]< wl ,,l (ne, false) >}
+  {VA : [Γ ||-v<l> A | VΓ]< wl >}:
+  [Γ ||-v<l> A ≅ B | VΓt | VAt]< _ > ->
+  [Γ ||-v<l> A ≅ B | VΓf | VAf]< _ > ->
+  [Γ ||-v<l> A ≅ B | VΓ | VA ]< wl >.
+Proof.
+  intros.
+  unshelve eapply irrelevanceTyEq ; [eassumption | | ].
+  2: now eapply validEqTySplit.
+Qed.  
+
+Lemma validTmSplit {wl : wfLCon} {Γ l A t} {n : nat} {ne : not_in_LCon wl n}
+  {VΓt : [||-v Γ ]< (wl ,,l (ne, true)) >}
+  {VΓf : [||-v Γ ]< (wl ,,l (ne, false)) >}
+  {VΓ : [||-v Γ]< wl >}
+  {VAt : [Γ ||-v<l> A | VΓt]< wl ,,l (ne, true) >}
+  {VAf : [Γ ||-v<l> A | VΓf]< wl ,,l (ne, false) >} :
+  [Γ ||-v<l> t : A | VΓt | VAt]< _ > ->
+  [Γ ||-v<l> t : A | VΓf | VAf]< _ > ->
+  [Γ ||-v<l> t : A | VΓ | validTySplit VAt VAf]< wl >.
+Proof.
+  intros [Vtt Vtextt] [Vtf Vtextf].
+  unshelve econstructor.
+  - intros ?????? ; cbn.
+    destruct (decidInLCon wl' n) as [ i | i | notin].
+    + now eapply Vtt.
+    + now eapply Vtf.
+    + eapply TmSplit.
+      * now eapply Vtt.
+      * now eapply Vtf.
+  - intros ; cbn.
+    destruct (decidInLCon wl' n) as [ i | i | notin].
+    + pose (f' := LCon_le_in_LCon (ne := ne) f i).
+      pose (f'':= @LCon_le_step wl wl n true ne (wfLCon_le_id _)).
+      unshelve eapply Vtextt.
+      * change f with (f' •ε f'') in Vσ'.
+        eapply subst_Ltrans' in Vσ'.
+        unshelve eapply irrelevanceSubst ; [ | assumption | ]. 
+        1: now eapply  WfC_Ltrans.
+        exact Vσ'.
+      * change f with (f' •ε f'') in Vσσ'.
+        unshelve eapply eqsubst_Ltrans' in Vσσ'.
+        unshelve eapply irrelevanceSubstEq ; [ | assumption | | ]. 
+        1: now eapply  WfC_Ltrans.
+        2: exact Vσσ'.
+    + pose (f' := LCon_le_in_LCon (ne := ne) f i).
+      pose (f'':= @LCon_le_step wl wl n false ne (wfLCon_le_id _)).
+      unshelve eapply Vtextf.
+      * change f with (f' •ε f'') in Vσ'.
+        eapply subst_Ltrans' in Vσ'.
+        unshelve eapply irrelevanceSubst ; [ | assumption | ]. 
+        1: now eapply  WfC_Ltrans.
+        exact Vσ'.
+      * change f with (f' •ε f'') in Vσσ'.
+        unshelve eapply eqsubst_Ltrans' in Vσσ'.
+        unshelve eapply irrelevanceSubstEq ; [ | assumption | | ]. 
+        1: now eapply  WfC_Ltrans.
+        2: exact Vσσ'.
+    + unshelve eapply TmEqSplit.
+      * pose (i := @in_here_l wl' n true).
+        pose (f' := @LCon_le_up wl wl' n true ne notin f). 
+        pose (f'':= @LCon_le_step wl wl n true ne (wfLCon_le_id _)).
+        pose (f''':= @LCon_le_step wl' wl' n true notin (wfLCon_le_id _)).
+        unshelve eapply Vtextt ; tea.
+        -- unshelve epose proof (X:= subst_Ltrans f''' _ Vσ').
+           1: now eapply wfc_Ltrans.
+           change (f''' •ε f)  with (f' •ε f'') in X.
+           eapply subst_Ltrans' in X.
+           unshelve eapply irrelevanceSubst.
+           ++ exists (VPack_Ltrans f'' VΓ).
+              now eapply  WfC_Ltrans.
+           ++ now eapply wfc_Ltrans.
+           ++ assumption.
+        -- unshelve epose proof (X:= eqsubst_Ltrans f''' _ _ Vσσ').
+           1: now eapply wfc_Ltrans.
+           change (f''' •ε f)  with (f' •ε f'') in X.
+           eapply eqsubst_Ltrans' in X.
+           unshelve eapply irrelevanceSubstEq.
+           1: cbn ; exists (VPack_Ltrans f'' VΓ) ; now eapply  WfC_Ltrans.
+           1:  now eapply wfc_Ltrans.
+           2: eassumption.
+      * pose (i := @in_here_l wl' n false).
+        pose (f' := @LCon_le_up wl wl' n false ne notin f). 
+        pose (f'':= @LCon_le_step wl wl n false ne (wfLCon_le_id _)).
+        pose (f''':= @LCon_le_step wl' wl' n false notin (wfLCon_le_id _)).
+        unshelve eapply Vtextf ; tea.
+        -- unshelve epose proof (X:= subst_Ltrans f''' _ Vσ').
+           1: now eapply wfc_Ltrans.
+           change (f''' •ε f)  with (f' •ε f'') in X.
+           eapply subst_Ltrans' in X.
+           unshelve eapply irrelevanceSubst.
+           ++ exists (VPack_Ltrans f'' VΓ).
+              now eapply  WfC_Ltrans.
+           ++ now eapply wfc_Ltrans.
+           ++ assumption.
+        -- unshelve epose proof (X:= eqsubst_Ltrans f''' _ _ Vσσ').
+           1: now eapply wfc_Ltrans.
+           change (f''' •ε f)  with (f' •ε f'') in X.
+           eapply eqsubst_Ltrans' in X.
+           unshelve eapply irrelevanceSubstEq.
+           1: cbn ; exists (VPack_Ltrans f'' VΓ) ; now eapply  WfC_Ltrans.
+           1:  now eapply wfc_Ltrans.
+           2: eassumption.
+Qed.
+
+Lemma validTmSplit' {wl : wfLCon} {Γ l A t} {n : nat} {ne : not_in_LCon wl n}
+  {VΓt : [||-v Γ ]< (wl ,,l (ne, true)) >}
+  {VΓf : [||-v Γ ]< (wl ,,l (ne, false)) >}
+  {VΓ : [||-v Γ]< wl >}
+  {VAt : [Γ ||-v<l> A | VΓt]< wl ,,l (ne, true) >}
+  {VAf : [Γ ||-v<l> A | VΓf]< wl ,,l (ne, false) >}
+  {VA : [Γ ||-v<l> A | VΓ]< wl >}:
+  [Γ ||-v<l> t : A | VΓt | VAt]< _ > ->
+  [Γ ||-v<l> t : A | VΓf | VAf]< _ > ->
+  [Γ ||-v<l> t : A | VΓ | VA]< wl >.
+Proof.
+  intros.
+  unshelve eapply irrelevanceTm ; [eassumption | | ].
+  2: now eapply validTmSplit.
+Qed.  
+
+Lemma validEqTmSplit {wl : wfLCon} {Γ l t u A} {n : nat} {ne : not_in_LCon wl n}
+  {VΓt : [||-v Γ ]< (wl ,,l (ne, true)) >}
+  {VΓf : [||-v Γ ]< (wl ,,l (ne, false)) >}
+  {VΓ : [||-v Γ]< wl >}
+  {VAt : [Γ ||-v<l> A | VΓt]< wl ,,l (ne, true) >}
+  {VAf : [Γ ||-v<l> A | VΓf]< wl ,,l (ne, false) >} :
+  [Γ ||-v<l> t ≅ u : A | VΓt | VAt]< _ > ->
+  [Γ ||-v<l> t ≅ u : A | VΓf | VAf]< _ > ->
+  [Γ ||-v<l> t ≅ u : A | VΓ | validTySplit VAt VAf]< wl >.
+Proof.
+  intros [Vtut] [Vtuf].
+  unshelve econstructor.
+  - intros ; cbn.
+    destruct (decidInLCon wl' n) as [ i | i | notin].
+    + now eapply Vtut.
+    + now eapply Vtuf.
+    + eapply TmEqSplit.
+      * now eapply Vtut.
+      * now eapply Vtuf.
+Qed.
+        
+
+Lemma validEqTmSplit' {wl : wfLCon} {Γ l t u A} {n : nat} {ne : not_in_LCon wl n}
+  {VΓt : [||-v Γ ]< (wl ,,l (ne, true)) >}
+  {VΓf : [||-v Γ ]< (wl ,,l (ne, false)) >}
+  {VΓ : [||-v Γ]< wl >}
+  {VAt : [Γ ||-v<l> A | VΓt]< wl ,,l (ne, true) >}
+  {VAf : [Γ ||-v<l> A | VΓf]< wl ,,l (ne, false) >}
+  {VA : [Γ ||-v<l> A | VΓ]< wl >}:
+  [Γ ||-v<l> t ≅ u : A | VΓt | VAt]< _ > ->
+  [Γ ||-v<l> t ≅ u : A | VΓf | VAf]< _ > ->
+  [Γ ||-v<l> t ≅ u : A | VΓ | VA]< wl >.
+Proof.
+  intros.
+  unshelve eapply irrelevanceTmEq ; [eassumption | | ].
+  2: now eapply validEqTmSplit.
+Qed.  
+
+Lemma WfCSplit {wl : wfLCon} {Γ} {n : nat} {ne : not_in_LCon wl n} :
+  [||-v Γ ]< (wl ,,l (ne, true)) > ->
+  [||-v Γ ]< (wl ,,l (ne, false)) > ->
+  [||-v Γ ]< wl >.
+Proof.
+  intros VGt VGf.
+  epose (Ht := invValidity VGt).
+  epose (Hf := invValidity VGf).
+  induction Γ as [ | A ? ?] ; cbn in *.
+  - now eapply validEmpty'.
+  - cbn in *.
+    destruct Ht as [lt [VGt' [VAt [Hsubt [Hextt Heqt]]]]].
+    destruct Hf as [lf [VGf' [VAf [Hsubf [Hextf Heqf]]]]].
+    unshelve eapply validSnoc'.
+    1: destruct lt ; [destruct lf ; [exact zero | exact one] | exact one].
+    1: now eapply IHΓ.
+    all: cbn.
+    1:{ destruct lt, lf.
+        all: eapply validTySplit ; try eassumption.
+        1,2 : eapply embValidTy ; try eassumption.
+        all: now constructor.
+    }
+Qed.
+
+End Split.
